<?xml version="1.0"?>
<rdf:RDF xmlns="http://ontologies.ti-semantics.com/core#"
     xml:base="http://ontologies.ti-semantics.com/core"
     xmlns:dct="http://purl.org/dc/dcmitype/"
     xmlns:owl="http://www.w3.org/2002/07/owl#"
     xmlns:rdf="http://www.w3.org/1999/02/22-rdf-syntax-ns#"
     xmlns:uvo="http://ontologies.ti-semantics.com/uvo#"
     xmlns:xml="http://www.w3.org/XML/1998/namespace"
     xmlns:xsd="http://www.w3.org/2001/XMLSchema#"
     xmlns:rdfs="http://www.w3.org/2000/01/rdf-schema#"
     xmlns:terms="http://purl.org/dc/terms/">
    <owl:Ontology rdf:about="http://ontologies.ti-semantics.com/core">
        <owl:versionIRI rdf:resource="http://ontologies.ti-semantics.com/core-1.0.3"/>
        <terms:license rdf:resource="http://creativecommons.org/licenses/by-sa/4.0/"/>
        <rdfs:comment xml:lang="en">Core concepts for the ontology of computer security properties and classes for use in threat intelligence and incidence response.</rdfs:comment>
        <rdfs:label xml:lang="en">Core Computer Security Ontology</rdfs:label>
        <rdfs:seeAlso rdf:datatype="http://www.w3.org/2001/XMLSchema#anyURI">https://nvlpubs.nist.gov/nistpubs/SpecialPublications/NIST.SP.800-126r3.pdf</rdfs:seeAlso>
        <owl:versionInfo xml:lang="en">Be warned that this version is under heavy development</owl:versionInfo>
    </owl:Ontology>
    


    <!-- 
    ///////////////////////////////////////////////////////////////////////////////////////
    //
    // Annotation properties
    //
    ///////////////////////////////////////////////////////////////////////////////////////
     -->

    


    <!-- http://purl.org/dc/terms/license -->

    <owl:AnnotationProperty rdf:about="http://purl.org/dc/terms/license"/>
    


    <!-- 
    ///////////////////////////////////////////////////////////////////////////////////////
    //
    // Object Properties
    //
    ///////////////////////////////////////////////////////////////////////////////////////
     -->

    


    <!-- http://ontologies.ti-semantics.com/core#comprisedOf -->

    <owl:ObjectProperty rdf:about="http://ontologies.ti-semantics.com/core#comprisedOf">
        <rdfs:domain rdf:resource="http://ontologies.ti-semantics.com/core#Platform"/>
        <rdfs:range rdf:resource="http://ontologies.ti-semantics.com/core#Hardware"/>
        <rdfs:range rdf:resource="http://ontologies.ti-semantics.com/core#Software"/>
    </owl:ObjectProperty>
    


    <!-- http://ontologies.ti-semantics.com/core#reference -->

    <owl:ObjectProperty rdf:about="http://ontologies.ti-semantics.com/core#reference">
        <rdfs:range rdf:resource="http://ontologies.ti-semantics.com/core#Reference"/>
        <rdfs:comment xml:lang="en">Relates some entity to some external resource.</rdfs:comment>
    </owl:ObjectProperty>
    


    <!-- http://ontologies.ti-semantics.com/cti#implements -->

    <owl:ObjectProperty rdf:about="http://ontologies.ti-semantics.com/cti#implements"/>
    


    <!-- 
    ///////////////////////////////////////////////////////////////////////////////////////
    //
    // Data properties
    //
    ///////////////////////////////////////////////////////////////////////////////////////
     -->

    


    <!-- http://ontologies.ti-semantics.com/core#externalID -->

    <owl:DatatypeProperty rdf:about="http://ontologies.ti-semantics.com/core#externalID">
        <rdfs:subPropertyOf rdf:resource="http://ontologies.ti-semantics.com/core#id"/>
        <rdfs:domain rdf:resource="http://ontologies.ti-semantics.com/core#Reference"/>
        <rdfs:range rdf:resource="http://www.w3.org/2001/XMLSchema#token"/>
        <rdfs:comment xml:lang="en">This is an ID given by some other entity, not a part of the RDF model. For instance, &quot;CAPEC-158&quot; or &quot;S0049&quot;. It is not meaningful on it&apos;s own, but together with a referenceSource or some other qualifier, may be useful.</rdfs:comment>
    </owl:DatatypeProperty>
    


    <!-- http://ontologies.ti-semantics.com/core#id -->

    <owl:DatatypeProperty rdf:about="http://ontologies.ti-semantics.com/core#id">
        <rdfs:range rdf:resource="http://www.w3.org/2001/XMLSchema#token"/>
        <rdfs:comment xml:lang="en">General identifier as a token literal. For instance, CVE-2019-0002 for a CVE.</rdfs:comment>
        <rdfs:label xml:lang="en">id</rdfs:label>
    </owl:DatatypeProperty>
    


    <!-- http://ontologies.ti-semantics.com/core#referenceSource -->

    <owl:DatatypeProperty rdf:about="http://ontologies.ti-semantics.com/core#referenceSource">
        <rdfs:domain rdf:resource="http://ontologies.ti-semantics.com/core#Reference"/>
        <rdfs:range rdf:resource="http://www.w3.org/2001/XMLSchema#token"/>
        <rdfs:comment xml:lang="en">This is a token that represents the source of the reference. Values look like: BID, SECTRACK, CONFIRM, etc.</rdfs:comment>
        <rdfs:label xml:lang="en">reference source</rdfs:label>
    </owl:DatatypeProperty>
    


    <!-- http://ontologies.ti-semantics.com/core#referenceTitle -->

    <owl:DatatypeProperty rdf:about="http://ontologies.ti-semantics.com/core#referenceTitle">
        <rdfs:domain rdf:resource="http://ontologies.ti-semantics.com/core#Reference"/>
        <rdfs:range rdf:resource="http://www.w3.org/2000/01/rdf-schema#Literal"/>
        <rdfs:comment xml:lang="en">A human readable title for this reference.</rdfs:comment>
        <rdfs:label xml:lang="en">reference title</rdfs:label>
    </owl:DatatypeProperty>
    


    <!-- http://ontologies.ti-semantics.com/core#referenceURL -->

    <owl:DatatypeProperty rdf:about="http://ontologies.ti-semantics.com/core#referenceURL">
        <rdfs:domain rdf:resource="http://ontologies.ti-semantics.com/core#Reference"/>
        <rdfs:range rdf:resource="http://www.w3.org/2001/XMLSchema#anyURI"/>
        <rdfs:comment xml:lang="en">The URL the reference points to. This should be a human readable WWW resource. If the resource is RDF, it would be better to use rdfs:seeAlso.</rdfs:comment>
        <rdfs:label xml:lang="en">reference URL</rdfs:label>
    </owl:DatatypeProperty>
    


    <!-- 
    ///////////////////////////////////////////////////////////////////////////////////////
    //
    // Classes
    //
    ///////////////////////////////////////////////////////////////////////////////////////
     -->

    


    <!-- http://ontologies.ti-semantics.com/core#Activity -->

    <owl:Class rdf:about="http://ontologies.ti-semantics.com/core#Activity">
        <rdfs:comment xml:lang="en">An activity is some action executed by an actor or on behalf on an actor.</rdfs:comment>
    </owl:Class>
    


    <!-- http://ontologies.ti-semantics.com/core#AdversarialActivity -->

    <owl:Class rdf:about="http://ontologies.ti-semantics.com/core#AdversarialActivity">
        <rdfs:subClassOf rdf:resource="http://ontologies.ti-semantics.com/core#Activity"/>
    </owl:Class>
    


    <!-- http://ontologies.ti-semantics.com/core#Application -->

    <owl:Class rdf:about="http://ontologies.ti-semantics.com/core#Application">
        <rdfs:subClassOf rdf:resource="http://ontologies.ti-semantics.com/core#Software"/>
    </owl:Class>
    


    <!-- http://ontologies.ti-semantics.com/core#Attack -->

    <owl:Class rdf:about="http://ontologies.ti-semantics.com/core#Attack">
        <rdfs:subClassOf rdf:resource="http://ontologies.ti-semantics.com/core#AdversarialActivity"/>
    </owl:Class>
    


    <!-- http://ontologies.ti-semantics.com/core#Catalog -->

    <owl:Class rdf:about="http://ontologies.ti-semantics.com/core#Catalog">
        <rdfs:comment xml:lang="en">Characterizes a collection of software security issues (flaws, faults, bugs, vulnerabilities, weaknesses, etc).</rdfs:comment>
        <rdfs:label xml:lang="en">Catalog</rdfs:label>
    </owl:Class>
    


    <!-- http://ontologies.ti-semantics.com/core#CourseOfAction -->

    <owl:Class rdf:about="http://ontologies.ti-semantics.com/core#CourseOfAction">
        <rdfs:comment xml:lang="en">A Course of Action is an action taken either to prevent an attack or to respond to an attack that is in progress. It may describe technical, automatable responses (applying patches, reconfiguring firewalls) but can also describe higher level actions like employee training or policy changes. For example, a course of action to mitigate a vulnerability could describe applying the patch that fixes it.</rdfs:comment>
    </owl:Class>
    


    <!-- http://ontologies.ti-semantics.com/core#Firmware -->

    <owl:Class rdf:about="http://ontologies.ti-semantics.com/core#Firmware">
        <rdfs:subClassOf rdf:resource="http://ontologies.ti-semantics.com/core#Software"/>
    </owl:Class>
    


    <!-- http://ontologies.ti-semantics.com/core#Hardware -->

    <owl:Class rdf:about="http://ontologies.ti-semantics.com/core#Hardware"/>
    


    <!-- http://ontologies.ti-semantics.com/core#LocalUser -->

    <owl:Class rdf:about="http://ontologies.ti-semantics.com/core#LocalUser">
        <rdfs:subClassOf rdf:resource="http://xmlns.com/foaf/0.1/Agent"/>
    </owl:Class>
    


    <!-- http://ontologies.ti-semantics.com/core#Malware -->

    <owl:Class rdf:about="http://ontologies.ti-semantics.com/core#Malware">
        <owl:disjointWith rdf:resource="http://ontologies.ti-semantics.com/core#Tool"/>
        <rdfs:comment xml:lang="en">Malware is a type of TTP that is also known as malicious code and malicious software, and refers to a program that is inserted into a system, usually covertly, with the intent of compromising the confidentiality, integrity, or availability of the victim&apos;s data, applications, or operating system (OS) or of otherwise annoying or disrupting the victim. Malware such as viruses and worms are usually designed to perform these nefarious functions in such a way that users are unaware of them, at least initially.
 
A Malware individual characterizes, identifies, and categorizes malware samples and families via a text description property. This provides detailed information about how the malware works and what it does. Relationships from Malware can capture what the malware targets (Vulnerability and Identity) and link it to other Malware individuals that it is a variant of.</rdfs:comment>
        <rdfs:isDefinedBy xml:lang="en">http://docs.oasis-open.org/cti/stix/v2.0/cs01/part2-stix-objects/stix-v2.0-cs01-part2-stix-objects.html#_Toc496714319</rdfs:isDefinedBy>
    </owl:Class>
    


    <!-- http://ontologies.ti-semantics.com/core#Metric -->

    <owl:Class rdf:about="http://ontologies.ti-semantics.com/core#Metric">
        <rdfs:comment xml:lang="en">A security metric is a measurement of risk associated with some aspect of computer security. A standard of measure of a degree to which a software system or process possesses some property.</rdfs:comment>
        <rdfs:label xml:lang="en">Metric</rdfs:label>
    </owl:Class>
    


    <!-- http://ontologies.ti-semantics.com/core#OperatingSystem -->

    <owl:Class rdf:about="http://ontologies.ti-semantics.com/core#OperatingSystem">
        <rdfs:subClassOf rdf:resource="http://ontologies.ti-semantics.com/core#Software"/>
    </owl:Class>
    


    <!-- http://ontologies.ti-semantics.com/core#Platform -->

    <owl:Class rdf:about="http://ontologies.ti-semantics.com/core#Platform">
        <owl:equivalentClass>
            <owl:Class>
                <owl:intersectionOf rdf:parseType="Collection">
                    <owl:Restriction>
                        <owl:onProperty rdf:resource="http://ontologies.ti-semantics.com/core#comprisedOf"/>
                        <owl:someValuesFrom rdf:resource="http://ontologies.ti-semantics.com/core#Application"/>
                    </owl:Restriction>
                    <owl:Restriction>
                        <owl:onProperty rdf:resource="http://ontologies.ti-semantics.com/core#comprisedOf"/>
                        <owl:qualifiedCardinality rdf:datatype="http://www.w3.org/2001/XMLSchema#nonNegativeInteger">1</owl:qualifiedCardinality>
                        <owl:onClass rdf:resource="http://ontologies.ti-semantics.com/core#Hardware"/>
                    </owl:Restriction>
                    <owl:Restriction>
                        <owl:onProperty rdf:resource="http://ontologies.ti-semantics.com/core#comprisedOf"/>
                        <owl:qualifiedCardinality rdf:datatype="http://www.w3.org/2001/XMLSchema#nonNegativeInteger">1</owl:qualifiedCardinality>
                        <owl:onClass rdf:resource="http://ontologies.ti-semantics.com/core#OperatingSystem"/>
                    </owl:Restriction>
                </owl:intersectionOf>
            </owl:Class>
        </owl:equivalentClass>
        <rdfs:comment xml:lang="en">In this context, platform refers to applications, operating systems, and hardware devices present among an enterprise’s computing assets. A computer or hardware device and/or associated operating system, or a virtual environment, on which software can be installed or run. Examples of platforms include Linux™, Microsoft Windows Vista®, and Java™.</rdfs:comment>
        <rdfs:label xml:lang="en">Platform</rdfs:label>
    </owl:Class>
    


    <!-- http://ontologies.ti-semantics.com/core#Reference -->

    <owl:Class rdf:about="http://ontologies.ti-semantics.com/core#Reference">
        <rdfs:comment xml:lang="en">A reference is some identifiable external resource. Ideally, it would have a referenceURL, but in some cases we have to work with a referenceSource and an externalID to help locate this resource.
For references to other RDF resources, we could also use rdf:seeAlso.</rdfs:comment>
        <rdfs:label xml:lang="en">Reference</rdfs:label>
    </owl:Class>
    


    <!-- http://ontologies.ti-semantics.com/core#RemoteUser -->

    <owl:Class rdf:about="http://ontologies.ti-semantics.com/core#RemoteUser">
        <rdfs:subClassOf rdf:resource="http://xmlns.com/foaf/0.1/Agent"/>
    </owl:Class>
    


    <!-- http://ontologies.ti-semantics.com/core#Software -->

    <owl:Class rdf:about="http://ontologies.ti-semantics.com/core#Software">
        <owl:equivalentClass rdf:resource="http://purl.org/dc/dcmitype/Software"/>
    </owl:Class>
    


    <!-- http://ontologies.ti-semantics.com/core#Superuser -->

    <owl:Class rdf:about="http://ontologies.ti-semantics.com/core#Superuser">
        <rdfs:subClassOf rdf:resource="http://xmlns.com/foaf/0.1/Agent"/>
        <rdfs:isDefinedBy xml:lang="en">https://en.wikipedia.org/wiki/Superuser</rdfs:isDefinedBy>
    </owl:Class>
    


    <!-- http://ontologies.ti-semantics.com/core#System -->

    <owl:Class rdf:about="http://ontologies.ti-semantics.com/core#System">
        <rdfs:subClassOf rdf:resource="http://ontologies.ti-semantics.com/core#Platform"/>
    </owl:Class>
    


    <!-- http://ontologies.ti-semantics.com/core#ThreatActor -->

    <owl:Class rdf:about="http://ontologies.ti-semantics.com/core#ThreatActor">
        <rdfs:comment xml:lang="en">Threat Actors are actual individuals, groups, or organizations believed to be operating with malicious intent. A Threat Actor is not an Intrusion Set but may support or be affiliated with various Intrusion Sets, groups, or organizations over time.
 
Threat Actors leverage their resources, and possibly the resources of an Intrusion Set, to conduct attacks and run Campaigns against targets.
 
Threat Actors can be characterized by their motives, capabilities, goals, sophistication level, past activities, resources they have access to, and their role in the organization.</rdfs:comment>
        <rdfs:isDefinedBy xml:lang="en">http://docs.oasis-open.org/cti/stix/v2.0/cs01/part2-stix-objects/stix-v2.0-cs01-part2-stix-objects.html#_Toc496714328</rdfs:isDefinedBy>
    </owl:Class>
    


    <!-- http://ontologies.ti-semantics.com/core#Tool -->

    <owl:Class rdf:about="http://ontologies.ti-semantics.com/core#Tool">
        <rdfs:subClassOf>
            <owl:Class>
                <owl:intersectionOf rdf:parseType="Collection">
                    <rdf:Description rdf:about="http://ontologies.ti-semantics.com/core#Software"/>
                    <owl:Restriction>
                        <owl:onProperty rdf:resource="http://ontologies.ti-semantics.com/cti#implements"/>
                        <owl:someValuesFrom rdf:resource="http://ontologies.ti-semantics.com/cti#Technique"/>
                    </owl:Restriction>
                </owl:intersectionOf>
            </owl:Class>
        </rdfs:subClassOf>
        <rdfs:comment xml:lang="en">Tools are legitimate software that can be used by threat actors to perform attacks. Knowing how and when threat actors use such tools can be important for understanding how campaigns are executed. Unlike malware, these tools or software packages are often found on a system and have legitimate purposes for power users, system administrators, network administrators, or even normal users. Remote access tools (e.g., RDP) and network scanning tools (e.g., Nmap) are examples of Tools that may be used by a Threat Actor during an attack.
 
The Tool individual characterizes the properties of these software tools and can be used as a basis for making an assertion about how a Threat Actor uses them during an attack. It contains properties to name and describe the tool, a list of Kill Chain Phases the tool can be used to carry out, and the version of the tool.
 
A Tool individual must not be used to characterize malware. Further, a Tool must not be used to characterise tools used as part of a course of action in response to an attack. Tools used during response activities can be included directly as part of a course of action.</rdfs:comment>
        <rdfs:isDefinedBy xml:lang="en">http://docs.oasis-open.org/cti/stix/v2.0/cs01/part2-stix-objects/stix-v2.0-cs01-part2-stix-objects.html#_Toc496714331</rdfs:isDefinedBy>
    </owl:Class>
    


    <!-- http://ontologies.ti-semantics.com/core#UnixRoot -->

    <owl:Class rdf:about="http://ontologies.ti-semantics.com/core#UnixRoot">
        <rdfs:subClassOf rdf:resource="http://ontologies.ti-semantics.com/core#Superuser"/>
        <rdfs:comment xml:lang="en">In Unix-like computer OSes (such as Linux), root is the conventional name of the user who has all rights or permissions (to all files and programs) in all modes (single- or multi-user). Alternative names include baron in BeOS and avatar on some Unix variants. BSD often provides a toor (&quot;root&quot; written backward) account in addition to a root account. Regardless of the name, the superuser always has a user ID of 0. The root user can do many things an ordinary user cannot, such as changing the ownership of files and binding to network ports numbered below 1024.</rdfs:comment>
        <rdfs:isDefinedBy xml:lang="en">https://en.wikipedia.org/wiki/Superuser#Unix_and_Unix-like</rdfs:isDefinedBy>
    </owl:Class>
    


    <!-- http://ontologies.ti-semantics.com/core#Vulnerability -->

    <owl:Class rdf:about="http://ontologies.ti-semantics.com/core#Vulnerability">
        <rdfs:comment xml:lang="en">A Vulnerability is any weakness in the computational logic found in products or devices that could be exploited by a threat source.

A Vulnerability is &quot;a mistake in software that can be directly used by a hacker to gain access to a system or network&quot;. For example, if a piece of malware exploits CVE-2015-12345, a Malware individal could be linked to a Vulnerability individual that references CVE-2015-12345.
 
A Vulnerability individual is primarily used to link to external definitions of vulnerabilities or to describe 0-day vulnerabilities that do not yet have an external definition. Typically, other individuals assert relationships to Vulnerability objects when a specific vulnerability is targeted and exploited as part of malicious cyber activity. As such, Vulnerability objects can be used as a linkage to the asset management and compliance process.</rdfs:comment>
        <rdfs:isDefinedBy xml:lang="en">https://csrc.nist.gov/CSRC/media/Publications/nistir/8138/draft/documents/nistir_8138_draft.pdf</rdfs:isDefinedBy>
    </owl:Class>
    


    <!-- http://ontologies.ti-semantics.com/core#Weakness -->

    <owl:Class rdf:about="http://ontologies.ti-semantics.com/core#Weakness">
        <rdfs:comment xml:lang="en">This describes a fault in a system or software that may be exploited by an Threat Actor.</rdfs:comment>
        <rdfs:label xml:lang="en">Weakness</rdfs:label>
    </owl:Class>
    


    <!-- http://ontologies.ti-semantics.com/core#WindowsAdministrator -->

    <owl:Class rdf:about="http://ontologies.ti-semantics.com/core#WindowsAdministrator">
        <rdfs:subClassOf rdf:resource="http://ontologies.ti-semantics.com/core#Superuser"/>
        <rdfs:comment xml:lang="en">An administrator is someone who can make changes on a computer that will affect other users of the computer. Administrators can change security settings, install software and hardware, access all files on the computer, and make changes to other user accounts. To log on as an administrator, you need to have a user account on the computer with an Administrator account type.</rdfs:comment>
    </owl:Class>
    


    <!-- http://ontologies.ti-semantics.com/core#WindowsSystemUser -->

    <owl:Class rdf:about="http://ontologies.ti-semantics.com/core#WindowsSystemUser">
        <rdfs:subClassOf rdf:resource="http://ontologies.ti-semantics.com/core#Superuser"/>
        <rdfs:comment xml:lang="en">The system account and the administrator account (Administrators group) have the same file privileges, but they have different functions. The system account is used by the operating system and by services that run under Windows. There are many services and processes within Windows that need the capability to log on internally (for example during a Windows installation). The system account was designed for that purpose; it is an internal account, does not show up in User Manager, cannot be added to any groups, and cannot have user rights assigned to it. On the other hand, the system account does show up on an NTFS volume in File Manager in the Permissions portion of the Security menu. By default, the system account is granted full control to all files on an NTFS volume. Here the system account has the same functional privileges as the administrator account.</rdfs:comment>
        <rdfs:isDefinedBy xml:lang="en">https://support.microsoft.com/en-sg/help/120929/how-the-system-account-is-used-in-windows</rdfs:isDefinedBy>
    </owl:Class>
    


    <!-- http://ontologies.ti-semantics.com/cti#Technique -->

    <owl:Class rdf:about="http://ontologies.ti-semantics.com/cti#Technique"/>
    


    <!-- http://purl.org/dc/dcmitype/Software -->

    <owl:Class rdf:about="http://purl.org/dc/dcmitype/Software"/>
    


    <!-- http://xmlns.com/foaf/0.1/Agent -->

    <owl:Class rdf:about="http://xmlns.com/foaf/0.1/Agent"/>
</rdf:RDF>



<!-- Generated by the OWL API (version 4.5.9.2019-02-01T07:24:44Z) https://github.com/owlcs/owlapi -->

