<?xml version="1.0"?>
<rdf:RDF xmlns="http://ontologies.ti-semantics.com/score#"
     xml:base="http://ontologies.ti-semantics.com/score"
     xmlns:owl="http://www.w3.org/2002/07/owl#"
     xmlns:rdf="http://www.w3.org/1999/02/22-rdf-syntax-ns#"
     xmlns:xml="http://www.w3.org/XML/1998/namespace"
     xmlns:xsd="http://www.w3.org/2001/XMLSchema#"
     xmlns:core="http://ontologies.ti-semantics.com/core#"
     xmlns:rdfs="http://www.w3.org/2000/01/rdf-schema#"
     xmlns:score="http://ontologies.ti-semantics.com/score#"
     xmlns:terms="http://purl.org/dc/terms/">
    <owl:Ontology rdf:about="http://ontologies.ti-semantics.com/score">
        <owl:versionIRI rdf:resource="http://ontologies.ti-semantics.com/score-3.0-1.7-0.1"/>
        <owl:imports rdf:resource="http://ontologies.ti-semantics.com/core-1.0.0"/>
        <terms:license rdf:resource="http://creativecommons.org/licenses/by-sa/4.0/"/>
        <rdfs:comment xml:lang="en">This ontology provides a vocabulary and representation for a unified form of the Common Vulnerability Scoring System (CVSS) which provides an open framework for communicating the characteristics and impacts of IT vulnerabilities.</rdfs:comment>
        <rdfs:seeAlso rdf:datatype="http://www.w3.org/2001/XMLSchema#anyURI">https://csrc.nist.gov/CSRC/media/Publications/nistir/8138/draft/documents/nistir_8138_draft.pdf</rdfs:seeAlso>
        <rdfs:seeAlso rdf:datatype="http://www.w3.org/2001/XMLSchema#anyURI">https://www.first.org/cvss/specification-document</rdfs:seeAlso>
        <rdfs:seeAlso rdf:datatype="http://www.w3.org/2001/XMLSchema#anyURI">https://www.first.org/cvss/v2/guide</rdfs:seeAlso>
    </owl:Ontology>
    


    <!-- 
    ///////////////////////////////////////////////////////////////////////////////////////
    //
    // Annotation properties
    //
    ///////////////////////////////////////////////////////////////////////////////////////
     -->

    


    <!-- http://ontologies.ti-semantics.com/score#code -->

    <owl:AnnotationProperty rdf:about="http://ontologies.ti-semantics.com/score#code">
        <rdfs:comment xml:lang="en">Short code for describing score entities, usually used in string vectors to be less wordy.</rdfs:comment>
        <rdfs:range rdf:resource="http://www.w3.org/2001/XMLSchema#token"/>
        <rdfs:domain rdf:resource="http://ontologies.ti-semantics.com/score#Metric"/>
    </owl:AnnotationProperty>
    


    <!-- http://ontologies.ti-semantics.com/score#cvss_v2_code -->

    <owl:AnnotationProperty rdf:about="http://ontologies.ti-semantics.com/score#cvss_v2_code">
        <rdfs:comment xml:lang="en">Short code used for describing the entity, like AV or PR</rdfs:comment>
        <rdfs:subPropertyOf rdf:resource="http://ontologies.ti-semantics.com/score#code"/>
        <rdfs:range rdf:resource="http://www.w3.org/2001/XMLSchema#token"/>
        <rdfs:domain rdf:resource="http://ontologies.ti-semantics.com/score#CVSSv2Metric"/>
    </owl:AnnotationProperty>
    


    <!-- http://ontologies.ti-semantics.com/score#cvss_v3_code -->

    <owl:AnnotationProperty rdf:about="http://ontologies.ti-semantics.com/score#cvss_v3_code">
        <rdfs:comment xml:lang="en">Short code used for describing the entity, like AV or PR</rdfs:comment>
        <rdfs:subPropertyOf rdf:resource="http://ontologies.ti-semantics.com/score#code"/>
        <rdfs:range rdf:resource="http://www.w3.org/2001/XMLSchema#token"/>
        <rdfs:domain rdf:resource="http://ontologies.ti-semantics.com/score#CVSSv3Metric"/>
    </owl:AnnotationProperty>
    


    <!-- http://purl.org/dc/terms/license -->

    <owl:AnnotationProperty rdf:about="http://purl.org/dc/terms/license"/>
    


    <!-- 
    ///////////////////////////////////////////////////////////////////////////////////////
    //
    // Object Properties
    //
    ///////////////////////////////////////////////////////////////////////////////////////
     -->

    


    <!-- http://ontologies.ti-semantics.com/score#baseMetrics -->

    <owl:ObjectProperty rdf:about="http://ontologies.ti-semantics.com/score#baseMetrics">
        <rdfs:range rdf:resource="http://ontologies.ti-semantics.com/score#CVSSv2BaseMetricGroup"/>
        <rdfs:comment rdf:datatype="http://www.w3.org/2001/XMLSchema#string">Specifies a reference to the details for the base metrics</rdfs:comment>
        <rdfs:isDefinedBy rdf:datatype="http://www.w3.org/2001/XMLSchema#anyURI">https://www.first.org/cvss/cvss-v30-specification-v1.7.pdf</rdfs:isDefinedBy>
        <rdfs:label>Based Metrics Details</rdfs:label>
    </owl:ObjectProperty>
    


    <!-- http://ontologies.ti-semantics.com/score#environmentalMetrics -->

    <owl:ObjectProperty rdf:about="http://ontologies.ti-semantics.com/score#environmentalMetrics">
        <rdfs:range rdf:resource="http://ontologies.ti-semantics.com/score#EnvironmentalMetric"/>
        <rdfs:comment rdf:datatype="http://www.w3.org/2001/XMLSchema#string">Specifies a reference to the details for environmental metrics</rdfs:comment>
        <rdfs:isDefinedBy rdf:datatype="http://www.w3.org/2001/XMLSchema#anyURI">https://www.first.org/cvss/cvss-v30-specification-v1.7.pdf</rdfs:isDefinedBy>
        <rdfs:label>Environmental Metrics Details</rdfs:label>
    </owl:ObjectProperty>
    


    <!-- http://ontologies.ti-semantics.com/score#greaterScoreThan -->

    <owl:ObjectProperty rdf:about="http://ontologies.ti-semantics.com/score#greaterScoreThan">
        <owl:inverseOf rdf:resource="http://ontologies.ti-semantics.com/score#lesserScoreThan"/>
        <rdf:type rdf:resource="http://www.w3.org/2002/07/owl#TransitiveProperty"/>
        <rdfs:domain rdf:resource="http://ontologies.ti-semantics.com/score#Metric"/>
        <rdfs:range rdf:resource="http://ontologies.ti-semantics.com/score#Metric"/>
        <rdfs:comment xml:lang="en">A given score for a metric is greater than the subject metric score by some arbitrary amount.</rdfs:comment>
    </owl:ObjectProperty>
    


    <!-- http://ontologies.ti-semantics.com/score#hasAttackComplexity -->

    <owl:ObjectProperty rdf:about="http://ontologies.ti-semantics.com/score#hasAttackComplexity">
        <rdfs:subPropertyOf rdf:resource="http://ontologies.ti-semantics.com/score#hasExploitabilityMetric"/>
        <rdfs:range rdf:resource="http://ontologies.ti-semantics.com/score#CVSSv2AccessComplexity"/>
        <rdfs:isDefinedBy rdf:datatype="http://www.w3.org/2001/XMLSchema#anyURI">https://www.first.org/cvss/cvss-v30-specification-v1.7.pdf</rdfs:isDefinedBy>
    </owl:ObjectProperty>
    


    <!-- http://ontologies.ti-semantics.com/score#hasAttackVector -->

    <owl:ObjectProperty rdf:about="http://ontologies.ti-semantics.com/score#hasAttackVector">
        <rdfs:subPropertyOf rdf:resource="http://ontologies.ti-semantics.com/score#hasExploitabilityMetric"/>
        <rdfs:range rdf:resource="http://ontologies.ti-semantics.com/score#CVSSv3AttackVector"/>
        <rdfs:isDefinedBy rdf:datatype="http://www.w3.org/2001/XMLSchema#anyURI">https://www.first.org/cvss/cvss-v30-specification-v1.7.pdf</rdfs:isDefinedBy>
    </owl:ObjectProperty>
    


    <!-- http://ontologies.ti-semantics.com/score#hasAvailabilityImpact -->

    <owl:ObjectProperty rdf:about="http://ontologies.ti-semantics.com/score#hasAvailabilityImpact">
        <rdfs:subPropertyOf rdf:resource="http://ontologies.ti-semantics.com/score#hasImpactMetric"/>
        <rdfs:range rdf:resource="http://ontologies.ti-semantics.com/score#CVSSv2AvailabilityImpact"/>
        <rdfs:isDefinedBy rdf:datatype="http://www.w3.org/2001/XMLSchema#anyURI">https://www.first.org/cvss/cvss-v30-specification-v1.7.pdf</rdfs:isDefinedBy>
    </owl:ObjectProperty>
    


    <!-- http://ontologies.ti-semantics.com/score#hasConfidentialityImpact -->

    <owl:ObjectProperty rdf:about="http://ontologies.ti-semantics.com/score#hasConfidentialityImpact">
        <rdfs:subPropertyOf rdf:resource="http://ontologies.ti-semantics.com/score#hasImpactMetric"/>
        <rdfs:range rdf:resource="http://ontologies.ti-semantics.com/score#CVSSv2ConfidentialityImpact"/>
        <rdfs:isDefinedBy rdf:datatype="http://www.w3.org/2001/XMLSchema#anyURI">https://www.first.org/cvss/cvss-v30-specification-v1.7.pdf</rdfs:isDefinedBy>
    </owl:ObjectProperty>
    


    <!-- http://ontologies.ti-semantics.com/score#hasExploitabilityMetric -->

    <owl:ObjectProperty rdf:about="http://ontologies.ti-semantics.com/score#hasExploitabilityMetric">
        <rdfs:subPropertyOf rdf:resource="http://www.w3.org/2002/07/owl#topObjectProperty"/>
        <rdfs:domain rdf:resource="http://ontologies.ti-semantics.com/score#EnvironmentalMetric"/>
        <rdfs:isDefinedBy rdf:datatype="http://www.w3.org/2001/XMLSchema#anyURI">https://www.first.org/cvss/cvss-v30-specification-v1.7.pdf</rdfs:isDefinedBy>
    </owl:ObjectProperty>
    


    <!-- http://ontologies.ti-semantics.com/score#hasImpactMetric -->

    <owl:ObjectProperty rdf:about="http://ontologies.ti-semantics.com/score#hasImpactMetric">
        <rdfs:isDefinedBy rdf:datatype="http://www.w3.org/2001/XMLSchema#anyURI">https://www.first.org/cvss/cvss-v30-specification-v1.7.pdf</rdfs:isDefinedBy>
    </owl:ObjectProperty>
    


    <!-- http://ontologies.ti-semantics.com/score#hasIntegrityImpact -->

    <owl:ObjectProperty rdf:about="http://ontologies.ti-semantics.com/score#hasIntegrityImpact">
        <rdfs:subPropertyOf rdf:resource="http://ontologies.ti-semantics.com/score#hasImpactMetric"/>
        <rdfs:range rdf:resource="http://ontologies.ti-semantics.com/score#CVSSv3IntegrityImpact"/>
        <rdfs:isDefinedBy rdf:datatype="http://www.w3.org/2001/XMLSchema#anyURI">https://www.first.org/cvss/cvss-v30-specification-v1.7.pdf</rdfs:isDefinedBy>
    </owl:ObjectProperty>
    


    <!-- http://ontologies.ti-semantics.com/score#hasPrivilegesRequired -->

    <owl:ObjectProperty rdf:about="http://ontologies.ti-semantics.com/score#hasPrivilegesRequired">
        <rdfs:subPropertyOf rdf:resource="http://ontologies.ti-semantics.com/score#hasExploitabilityMetric"/>
        <rdfs:range rdf:resource="http://ontologies.ti-semantics.com/score#CVSSv3PrivilegesRequired"/>
        <rdfs:isDefinedBy rdf:datatype="http://www.w3.org/2001/XMLSchema#anyURI">https://www.first.org/cvss/cvss-v30-specification-v1.7.pdf</rdfs:isDefinedBy>
    </owl:ObjectProperty>
    


    <!-- http://ontologies.ti-semantics.com/score#hasScope -->

    <owl:ObjectProperty rdf:about="http://ontologies.ti-semantics.com/score#hasScope">
        <rdfs:subPropertyOf rdf:resource="http://www.w3.org/2002/07/owl#topObjectProperty"/>
        <rdfs:range rdf:resource="http://ontologies.ti-semantics.com/score#CVSSv3Scope"/>
        <rdfs:isDefinedBy rdf:datatype="http://www.w3.org/2001/XMLSchema#anyURI">https://www.first.org/cvss/cvss-v30-specification-v1.7.pdf</rdfs:isDefinedBy>
    </owl:ObjectProperty>
    


    <!-- http://ontologies.ti-semantics.com/score#hasUserInteraction -->

    <owl:ObjectProperty rdf:about="http://ontologies.ti-semantics.com/score#hasUserInteraction">
        <rdfs:subPropertyOf rdf:resource="http://ontologies.ti-semantics.com/score#hasExploitabilityMetric"/>
        <rdfs:range rdf:resource="http://ontologies.ti-semantics.com/score#CVSSv3UserInteraction"/>
        <rdfs:isDefinedBy rdf:datatype="http://www.w3.org/2001/XMLSchema#anyURI">https://www.first.org/cvss/cvss-v30-specification-v1.7.pdf</rdfs:isDefinedBy>
    </owl:ObjectProperty>
    


    <!-- http://ontologies.ti-semantics.com/score#lesserScoreThan -->

    <owl:ObjectProperty rdf:about="http://ontologies.ti-semantics.com/score#lesserScoreThan">
        <rdf:type rdf:resource="http://www.w3.org/2002/07/owl#TransitiveProperty"/>
        <rdfs:domain rdf:resource="http://ontologies.ti-semantics.com/score#Metric"/>
        <rdfs:range rdf:resource="http://ontologies.ti-semantics.com/score#Metric"/>
        <rdfs:comment xml:lang="en">A given metric score is less than the subject metric score by some arbitrary amount.</rdfs:comment>
    </owl:ObjectProperty>
    


    <!-- http://ontologies.ti-semantics.com/score#termporalMetrics -->

    <owl:ObjectProperty rdf:about="http://ontologies.ti-semantics.com/score#termporalMetrics">
        <rdfs:range rdf:resource="http://ontologies.ti-semantics.com/score#TemporalMetric"/>
        <rdfs:comment rdf:datatype="http://www.w3.org/2001/XMLSchema#string">Specifies a reference to the details for the Temporal Metrics</rdfs:comment>
        <rdfs:isDefinedBy rdf:datatype="http://www.w3.org/2001/XMLSchema#anyURI">https://www.first.org/cvss/cvss-v30-specification-v1.7.pdf</rdfs:isDefinedBy>
        <rdfs:label>Temporal Metrics Details</rdfs:label>
    </owl:ObjectProperty>
    


    <!-- 
    ///////////////////////////////////////////////////////////////////////////////////////
    //
    // Data properties
    //
    ///////////////////////////////////////////////////////////////////////////////////////
     -->

    


    <!-- http://ontologies.ti-semantics.com/score#cvss_score -->

    <owl:DatatypeProperty rdf:about="http://ontologies.ti-semantics.com/score#cvss_score">
        <rdfs:range rdf:resource="http://www.w3.org/2001/XMLSchema#decimal"/>
        <rdfs:label xml:lang="en">CVSS score</rdfs:label>
    </owl:DatatypeProperty>
    


    <!-- http://ontologies.ti-semantics.com/score#cvss_v2_baseScore -->

    <owl:DatatypeProperty rdf:about="http://ontologies.ti-semantics.com/score#cvss_v2_baseScore">
        <rdfs:subPropertyOf rdf:resource="http://ontologies.ti-semantics.com/score#cvss_v2_score"/>
        <rdfs:domain rdf:resource="http://ontologies.ti-semantics.com/score#CVSSv2BaseMetricGroup"/>
        <rdfs:range rdf:resource="http://www.w3.org/2001/XMLSchema#decimal"/>
        <rdfs:comment xml:lang="en">The base equation is the foundation of CVSS scoring. The base equation (formula version 2.10) is:

BaseScore = round_to_1_decimal(((0.6*Impact)+(0.4*Exploitability)-1.5)*f(Impact))

Impact = 10.41*(1-(1-ConfImpact)*(1-IntegImpact)*(1-AvailImpact))

Exploitability = 20* AccessVector*AccessComplexity*Authentication

f(impact)= 0 if Impact=0, 1.176 otherwise</rdfs:comment>
        <rdfs:isDefinedBy rdf:datatype="http://www.w3.org/2001/XMLSchema#anyURI">https://www.first.org/cvss/v2/guide</rdfs:isDefinedBy>
        <rdfs:label>Base Metric Score</rdfs:label>
    </owl:DatatypeProperty>
    


    <!-- http://ontologies.ti-semantics.com/score#cvss_v2_environmentalScore -->

    <owl:DatatypeProperty rdf:about="http://ontologies.ti-semantics.com/score#cvss_v2_environmentalScore">
        <rdfs:subPropertyOf rdf:resource="http://ontologies.ti-semantics.com/score#cvss_v2_score"/>
        <rdfs:domain rdf:resource="http://ontologies.ti-semantics.com/score#CVSSv2EnvironmentalMetricGroup"/>
        <rdfs:range rdf:resource="http://www.w3.org/2001/XMLSchema#decimal"/>
        <rdfs:comment xml:lang="en">If employed, the environmental equation will combine the environmental metrics with the temporal score to produce an environmental score ranging from 0 to 10. Further, this equation will produce a score no higher than the temporal score. The environmental equation is:

EnvironmentalScore = round_to_1_decimal((AdjustedTemporal+
(10-AdjustedTemporal)*CollateralDamagePotential)*TargetDistribution)

AdjustedTemporal = TemporalScore recomputed with the BaseScore&apos;s Impact sub-equation replaced with the AdjustedImpact equation

AdjustedImpact = min(10,10.41*(1-(1-ConfImpact*ConfReq)*(1-IntegImpact*IntegReq)
                     *(1-AvailImpact*AvailReq)))</rdfs:comment>
        <rdfs:isDefinedBy rdf:datatype="http://www.w3.org/2001/XMLSchema#anyURI">https://www.first.org/cvss/v2/guide</rdfs:isDefinedBy>
        <rdfs:label>Environment Score</rdfs:label>
    </owl:DatatypeProperty>
    


    <!-- http://ontologies.ti-semantics.com/score#cvss_v2_exploitSubscore -->

    <owl:DatatypeProperty rdf:about="http://ontologies.ti-semantics.com/score#cvss_v2_exploitSubscore">
        <rdfs:subPropertyOf rdf:resource="http://ontologies.ti-semantics.com/score#cvss_v2_score"/>
        <rdfs:range rdf:resource="http://www.w3.org/2001/XMLSchema#decimal"/>
        <rdfs:comment xml:lang="en">Specifies the base exploit sub-score asisgned to a vulnerability by a source

Exploitability = 20* AccessVector*AccessComplexity*Authentication</rdfs:comment>
        <rdfs:isDefinedBy rdf:datatype="http://www.w3.org/2001/XMLSchema#anyURI">https://www.first.org/cvss/v2/guide</rdfs:isDefinedBy>
        <rdfs:label>Exploit Subscore</rdfs:label>
    </owl:DatatypeProperty>
    


    <!-- http://ontologies.ti-semantics.com/score#cvss_v2_impactSubscore -->

    <owl:DatatypeProperty rdf:about="http://ontologies.ti-semantics.com/score#cvss_v2_impactSubscore">
        <rdfs:subPropertyOf rdf:resource="http://ontologies.ti-semantics.com/score#cvss_v2_score"/>
        <rdfs:range rdf:resource="http://www.w3.org/2001/XMLSchema#decimal"/>
        <rdfs:comment xml:lang="en">Specifies the base impact sub-score assigned to a vulnerability by a source

Impact = 10.41*(1-(1-ConfImpact)*(1-IntegImpact)*(1-AvailImpact))</rdfs:comment>
        <rdfs:isDefinedBy rdf:datatype="http://www.w3.org/2001/XMLSchema#anyURI">https://www.first.org/cvss/v2/guide</rdfs:isDefinedBy>
        <rdfs:label>Impact Sub-score</rdfs:label>
    </owl:DatatypeProperty>
    


    <!-- http://ontologies.ti-semantics.com/score#cvss_v2_overallScore -->

    <owl:DatatypeProperty rdf:about="http://ontologies.ti-semantics.com/score#cvss_v2_overallScore">
        <rdfs:subPropertyOf rdf:resource="http://ontologies.ti-semantics.com/score#cvss_v2_score"/>
        <rdfs:range rdf:resource="http://www.w3.org/2001/XMLSchema#decimal"/>
        <rdfs:comment rdf:datatype="http://www.w3.org/2001/XMLSchema#string">Specifies the overall score.</rdfs:comment>
        <rdfs:isDefinedBy rdf:datatype="http://www.w3.org/2001/XMLSchema#anyURI">https://www.first.org/cvss/v2/guide</rdfs:isDefinedBy>
        <rdfs:label>Overall Score</rdfs:label>
    </owl:DatatypeProperty>
    


    <!-- http://ontologies.ti-semantics.com/score#cvss_v2_score -->

    <owl:DatatypeProperty rdf:about="http://ontologies.ti-semantics.com/score#cvss_v2_score">
        <rdfs:subPropertyOf rdf:resource="http://ontologies.ti-semantics.com/score#cvss_score"/>
        <rdfs:range rdf:resource="http://www.w3.org/2001/XMLSchema#decimal"/>
        <rdfs:comment xml:lang="en">Specifies the CVSS v2 score</rdfs:comment>
        <rdfs:label xml:lang="en">CVSS v2 score</rdfs:label>
    </owl:DatatypeProperty>
    


    <!-- http://ontologies.ti-semantics.com/score#cvss_v2_temporalScore -->

    <owl:DatatypeProperty rdf:about="http://ontologies.ti-semantics.com/score#cvss_v2_temporalScore">
        <rdfs:subPropertyOf rdf:resource="http://ontologies.ti-semantics.com/score#cvss_v2_score"/>
        <rdfs:domain rdf:resource="http://ontologies.ti-semantics.com/score#CVSSv2TemporalMetricGroup"/>
        <rdfs:range rdf:resource="http://www.w3.org/2001/XMLSchema#decimal"/>
        <rdfs:comment xml:lang="en">If employed, the temporal equation will combine the temporal metrics with the base score to produce a temporal score ranging from 0 to 10. Further, the temporal score will produce a temporal score no higher than the base score, and no greater than 33% lower than the base score. The temporal equation is:

TemporalScore = round_to_1_decimal(BaseScore*Exploitability
                *RemediationLevel*ReportConfidence)</rdfs:comment>
        <rdfs:isDefinedBy rdf:datatype="http://www.w3.org/2001/XMLSchema#anyURI">https://www.first.org/cvss/v2/guide</rdfs:isDefinedBy>
        <rdfs:label>Temporal Score</rdfs:label>
    </owl:DatatypeProperty>
    


    <!-- http://ontologies.ti-semantics.com/score#cvss_v3_baseScore -->

    <owl:DatatypeProperty rdf:about="http://ontologies.ti-semantics.com/score#cvss_v3_baseScore">
        <rdfs:subPropertyOf rdf:resource="http://ontologies.ti-semantics.com/score#cvss_v3_score"/>
        <rdfs:range rdf:resource="http://www.w3.org/2001/XMLSchema#decimal"/>
        <rdfs:comment rdf:datatype="http://www.w3.org/2001/XMLSchema#string">Specifies a score, between 0 and 10, that represents the intrinsic and fundamental characteristics of a vulnerability that are consistent over time and user environments.</rdfs:comment>
        <rdfs:isDefinedBy rdf:datatype="http://www.w3.org/2001/XMLSchema#anyURI">https://www.first.org/cvss/cvss-v30-specification-v1.7.pdf</rdfs:isDefinedBy>
        <rdfs:label>Base Metric Score</rdfs:label>
    </owl:DatatypeProperty>
    


    <!-- http://ontologies.ti-semantics.com/score#cvss_v3_environmentalScore -->

    <owl:DatatypeProperty rdf:about="http://ontologies.ti-semantics.com/score#cvss_v3_environmentalScore">
        <rdfs:subPropertyOf rdf:resource="http://ontologies.ti-semantics.com/score#cvss_v3_score"/>
        <rdfs:range rdf:resource="http://www.w3.org/2001/XMLSchema#decimal"/>
        <rdfs:comment rdf:datatype="http://www.w3.org/2001/XMLSchema#string">Specifies a score, between 0 and 10, that represents the characteristics of a vulnerability that change over time but not among user environments.</rdfs:comment>
        <rdfs:isDefinedBy rdf:datatype="http://www.w3.org/2001/XMLSchema#anyURI">https://www.first.org/cvss/cvss-v30-specification-v1.7.pdf</rdfs:isDefinedBy>
        <rdfs:label>Environment Score</rdfs:label>
    </owl:DatatypeProperty>
    


    <!-- http://ontologies.ti-semantics.com/score#cvss_v3_exploitSubscore -->

    <owl:DatatypeProperty rdf:about="http://ontologies.ti-semantics.com/score#cvss_v3_exploitSubscore">
        <rdfs:subPropertyOf rdf:resource="http://ontologies.ti-semantics.com/score#cvss_v3_score"/>
        <rdfs:range rdf:resource="http://www.w3.org/2001/XMLSchema#decimal"/>
        <rdfs:comment rdf:datatype="http://www.w3.org/2001/XMLSchema#string">Specifies the base exploit sub-score asisgned to a vulnerability by a source</rdfs:comment>
        <rdfs:isDefinedBy rdf:datatype="http://www.w3.org/2001/XMLSchema#anyURI">https://www.first.org/cvss/cvss-v30-specification-v1.7.pdf</rdfs:isDefinedBy>
        <rdfs:label>Exploit Subscore</rdfs:label>
    </owl:DatatypeProperty>
    


    <!-- http://ontologies.ti-semantics.com/score#cvss_v3_impactSubscore -->

    <owl:DatatypeProperty rdf:about="http://ontologies.ti-semantics.com/score#cvss_v3_impactSubscore">
        <rdfs:subPropertyOf rdf:resource="http://ontologies.ti-semantics.com/score#cvss_v3_score"/>
        <rdfs:range rdf:resource="http://www.w3.org/2001/XMLSchema#decimal"/>
        <rdfs:comment rdf:datatype="http://www.w3.org/2001/XMLSchema#string">Specifies the base impact sub-score assigned to a vulnerability by a source</rdfs:comment>
        <rdfs:isDefinedBy rdf:datatype="http://www.w3.org/2001/XMLSchema#anyURI">https://www.first.org/cvss/cvss-v30-specification-v1.7.pdf</rdfs:isDefinedBy>
        <rdfs:label>Impact Sub-score</rdfs:label>
    </owl:DatatypeProperty>
    


    <!-- http://ontologies.ti-semantics.com/score#cvss_v3_overallScore -->

    <owl:DatatypeProperty rdf:about="http://ontologies.ti-semantics.com/score#cvss_v3_overallScore">
        <rdfs:subPropertyOf rdf:resource="http://ontologies.ti-semantics.com/score#cvss_v3_score"/>
        <rdfs:range rdf:resource="http://www.w3.org/2001/XMLSchema#decimal"/>
        <rdfs:comment rdf:datatype="http://www.w3.org/2001/XMLSchema#string">Specifies the overall score.</rdfs:comment>
        <rdfs:isDefinedBy rdf:datatype="http://www.w3.org/2001/XMLSchema#anyURI">https://www.first.org/cvss/cvss-v30-specification-v1.7.pdf</rdfs:isDefinedBy>
        <rdfs:label>Overall Score</rdfs:label>
    </owl:DatatypeProperty>
    


    <!-- http://ontologies.ti-semantics.com/score#cvss_v3_score -->

    <owl:DatatypeProperty rdf:about="http://ontologies.ti-semantics.com/score#cvss_v3_score">
        <rdfs:subPropertyOf rdf:resource="http://ontologies.ti-semantics.com/score#cvss_score"/>
        <rdfs:range rdf:resource="http://www.w3.org/2001/XMLSchema#decimal"/>
        <rdfs:comment xml:lang="en">Specifies the CVSS v3 Score</rdfs:comment>
        <rdfs:isDefinedBy rdf:datatype="http://www.w3.org/2001/XMLSchema#anyURI">https://www.first.org/cvss/cvss-v30-specification-v1.7.pdf</rdfs:isDefinedBy>
        <rdfs:label xml:lang="en">CVSS v3 score</rdfs:label>
    </owl:DatatypeProperty>
    


    <!-- http://ontologies.ti-semantics.com/score#cvss_v3_temporalScore -->

    <owl:DatatypeProperty rdf:about="http://ontologies.ti-semantics.com/score#cvss_v3_temporalScore">
        <rdfs:subPropertyOf rdf:resource="http://ontologies.ti-semantics.com/score#cvss_v3_score"/>
        <rdfs:range rdf:resource="http://www.w3.org/2001/XMLSchema#decimal"/>
        <rdfs:comment rdf:datatype="http://www.w3.org/2001/XMLSchema#string">Specifies a score, between 0 and 10, that represents the characteristics of a vulnerability that are relevant and unique to a particular user&apos;s environments.</rdfs:comment>
        <rdfs:isDefinedBy rdf:datatype="http://www.w3.org/2001/XMLSchema#anyURI">https://www.first.org/cvss/cvss-v30-specification-v1.7.pdf</rdfs:isDefinedBy>
        <rdfs:label>Temporal Score</rdfs:label>
    </owl:DatatypeProperty>
    


    <!-- http://ontologies.ti-semantics.com/score#generationTime -->

    <owl:DatatypeProperty rdf:about="http://ontologies.ti-semantics.com/score#generationTime">
        <rdfs:range rdf:resource="http://www.w3.org/2001/XMLSchema#dateTime"/>
        <rdfs:comment rdf:datatype="http://www.w3.org/2001/XMLSchema#string">Specifies the time and date when the CVSS base metrics were determined</rdfs:comment>
        <rdfs:isDefinedBy rdf:datatype="http://www.w3.org/2001/XMLSchema#anyURI">https://www.first.org/cvss/cvss-v30-specification-v1.7.pdf</rdfs:isDefinedBy>
        <rdfs:label>Generation Time</rdfs:label>
    </owl:DatatypeProperty>
    


    <!-- http://ontologies.ti-semantics.com/score#source -->

    <owl:DatatypeProperty rdf:about="http://ontologies.ti-semantics.com/score#source">
        <rdfs:range rdf:resource="http://www.w3.org/2001/XMLSchema#anyURI"/>
        <rdfs:comment rdf:datatype="http://www.w3.org/2001/XMLSchema#string">Specifies the source of the CVSS metric in the form of a URL</rdfs:comment>
        <rdfs:isDefinedBy rdf:datatype="http://www.w3.org/2001/XMLSchema#anyURI">https://www.first.org/cvss/cvss-v30-specification-v1.7.pdf</rdfs:isDefinedBy>
        <rdfs:label>CVSS Source</rdfs:label>
    </owl:DatatypeProperty>
    


    <!-- http://ontologies.ti-semantics.com/score#vector -->

    <owl:DatatypeProperty rdf:about="http://ontologies.ti-semantics.com/score#vector">
        <rdfs:range rdf:resource="http://www.w3.org/2001/XMLSchema#string"/>
        <rdfs:comment xml:lang="en">A CVSS score is also represented as a vector string, a compressed textual representation of the values used to derive the score.</rdfs:comment>
        <rdfs:comment rdf:datatype="http://www.w3.org/2001/XMLSchema#string">Specifies a compressed textual representation that reflects the values used to drive the CVSS score</rdfs:comment>
        <rdfs:isDefinedBy rdf:datatype="http://www.w3.org/2001/XMLSchema#anyURI">https://www.first.org/cvss/cvss-v30-specification-v1.7.pdf</rdfs:isDefinedBy>
        <rdfs:label>CVSS v2 Vector</rdfs:label>
    </owl:DatatypeProperty>
    


    <!-- 
    ///////////////////////////////////////////////////////////////////////////////////////
    //
    // Classes
    //
    ///////////////////////////////////////////////////////////////////////////////////////
     -->

    


    <!-- http://ontologies.ti-semantics.com/score#CVSSMetric -->

    <owl:Class rdf:about="http://ontologies.ti-semantics.com/score#CVSSMetric">
        <rdfs:subClassOf rdf:resource="http://ontologies.ti-semantics.com/score#Metric"/>
    </owl:Class>
    


    <!-- http://ontologies.ti-semantics.com/score#CVSSMetricGroup -->

    <owl:Class rdf:about="http://ontologies.ti-semantics.com/score#CVSSMetricGroup">
        <rdfs:subClassOf rdf:resource="http://ontologies.ti-semantics.com/score#MetricGroup"/>
        <rdfs:subClassOf>
            <owl:Restriction>
                <owl:onProperty rdf:resource="http://ontologies.ti-semantics.com/score#vector"/>
                <owl:qualifiedCardinality rdf:datatype="http://www.w3.org/2001/XMLSchema#nonNegativeInteger">1</owl:qualifiedCardinality>
                <owl:onDataRange rdf:resource="http://www.w3.org/2001/XMLSchema#token"/>
            </owl:Restriction>
        </rdfs:subClassOf>
    </owl:Class>
    


    <!-- http://ontologies.ti-semantics.com/score#CVSSv2AccessComplexity -->

    <owl:Class rdf:about="http://ontologies.ti-semantics.com/score#CVSSv2AccessComplexity">
        <rdfs:subClassOf rdf:resource="http://ontologies.ti-semantics.com/score#CVSSv2Metric"/>
        <rdfs:subClassOf rdf:resource="http://ontologies.ti-semantics.com/score#ExploitabilityMetric"/>
        <cvss_v2_code xml:lang="en">AC</cvss_v2_code>
        <rdfs:comment xml:lang="en">This metric measures the complexity of the attack required to exploit the vulnerability once an attacker has gained access to the target system. For example, consider a buffer overflow in an Internet service: once the target system is located, the attacker can launch an exploit at will.

Other vulnerabilities, however, may require additional steps in order to be exploited. For example, a vulnerability in an email client is only exploited after the user downloads and opens a tainted attachment. The lower the required complexity, the higher the vulnerability score.</rdfs:comment>
        <rdfs:isDefinedBy xml:lang="en">https://www.first.org/cvss/v2/guide#2-1-2-Access-Complexity-AC</rdfs:isDefinedBy>
        <rdfs:label xml:lang="en">Access Complexity</rdfs:label>
    </owl:Class>
    


    <!-- http://ontologies.ti-semantics.com/score#CVSSv2AccessVector -->

    <owl:Class rdf:about="http://ontologies.ti-semantics.com/score#CVSSv2AccessVector">
        <rdfs:subClassOf rdf:resource="http://ontologies.ti-semantics.com/score#CVSSv2Metric"/>
        <cvss_v2_code rdf:datatype="http://www.w3.org/2001/XMLSchema#token">AV</cvss_v2_code>
        <rdfs:comment xml:lang="en">This metric reflects how the vulnerability is exploited.</rdfs:comment>
        <rdfs:isDefinedBy rdf:datatype="http://www.w3.org/2001/XMLSchema#anyURI">https://www.first.org/cvss/v2/guide</rdfs:isDefinedBy>
    </owl:Class>
    


    <!-- http://ontologies.ti-semantics.com/score#CVSSv2AdjacentAccessVector -->

    <owl:Class rdf:about="http://ontologies.ti-semantics.com/score#CVSSv2AdjacentAccessVector">
        <rdfs:subClassOf rdf:resource="http://ontologies.ti-semantics.com/score#CVSSv2AccessVector"/>
    </owl:Class>
    


    <!-- http://ontologies.ti-semantics.com/score#CVSSv2Authentication -->

    <owl:Class rdf:about="http://ontologies.ti-semantics.com/score#CVSSv2Authentication">
        <rdfs:subClassOf rdf:resource="http://ontologies.ti-semantics.com/score#CVSSv2Metric"/>
        <cvss_v2_code rdf:datatype="http://www.w3.org/2001/XMLSchema#token">Au</cvss_v2_code>
        <rdfs:comment xml:lang="en">This metric measures the number of times an attacker must authenticate to a target in order to exploit a vulnerability. This metric does not gauge the strength or complexity of the authentication process, only that an attacker is required to provide credentials before an exploit may occur.</rdfs:comment>
        <rdfs:isDefinedBy rdf:datatype="http://www.w3.org/2001/XMLSchema#anyURI">https://www.first.org/cvss/v2/guide#2-1-3-Authentication-Au</rdfs:isDefinedBy>
    </owl:Class>
    


    <!-- http://ontologies.ti-semantics.com/score#CVSSv2AvailabilityImpact -->

    <owl:Class rdf:about="http://ontologies.ti-semantics.com/score#CVSSv2AvailabilityImpact">
        <rdfs:subClassOf rdf:resource="http://ontologies.ti-semantics.com/score#CVSSv2Metric"/>
        <rdfs:subClassOf rdf:resource="http://ontologies.ti-semantics.com/score#ImpactMetric"/>
        <cvss_v3_code>AI</cvss_v3_code>
        <rdfs:comment xml:lang="en">This metric measures the impact to the availability of the impacted component resulting from a successfully exploited vulnerability. While the Confidentiality and Integrity impact metrics apply to the loss of confidentiality or integrity of data (e.g., information, files) used by the impacted component, this metric refers to the loss of availability of the impacted component itself, such as a networked service (e.g., web, database, email). Since availability refers to the accessibility of information resources, attacks that consume network bandwidth, processor cycles, or disk space all impact the availability of an impacted component. This metric value increases with the consequence to the impacted component.</rdfs:comment>
        <rdfs:isDefinedBy rdf:datatype="http://www.w3.org/2001/XMLSchema#anyURI">https://www.first.org/cvss/cvss-v30-specification-v1.7.pdf</rdfs:isDefinedBy>
        <rdfs:label xml:lang="en">Availability Impact</rdfs:label>
    </owl:Class>
    


    <!-- http://ontologies.ti-semantics.com/score#CVSSv2AvailabilityRequirement -->

    <owl:Class rdf:about="http://ontologies.ti-semantics.com/score#CVSSv2AvailabilityRequirement">
        <rdfs:subClassOf rdf:resource="http://ontologies.ti-semantics.com/score#CVSSv2Metric"/>
        <rdfs:subClassOf rdf:resource="http://ontologies.ti-semantics.com/score#SecurityRequirement"/>
        <cvss_v2_code xml:lang="en">AR</cvss_v2_code>
        <rdfs:comment xml:lang="en">These metrics enable the analyst to customize the CVSS score depending on the importance of the affected IT asset to a user&apos;s organization, measured in terms of Availability. That is, if an IT asset supports a business function for which Availability is most important, the analyst can assign a greater value to Availability relative to Confidentiality and Integrity. Each security requirement has three possible values: Low, Medium, or High.</rdfs:comment>
        <rdfs:isDefinedBy xml:lang="en">https://www.first.org/cvss/v2/guide#2-3-3-Security-Requirements-CR-IR-AR</rdfs:isDefinedBy>
    </owl:Class>
    


    <!-- http://ontologies.ti-semantics.com/score#CVSSv2BaseMetricGroup -->

    <owl:Class rdf:about="http://ontologies.ti-semantics.com/score#CVSSv2BaseMetricGroup">
        <rdfs:subClassOf rdf:resource="http://ontologies.ti-semantics.com/score#CVSSv2MetricGroup"/>
        <rdfs:subClassOf>
            <owl:Restriction>
                <owl:onProperty rdf:resource="http://ontologies.ti-semantics.com/score#generationTime"/>
                <owl:someValuesFrom rdf:resource="http://www.w3.org/2000/01/rdf-schema#Literal"/>
            </owl:Restriction>
        </rdfs:subClassOf>
        <rdfs:subClassOf>
            <owl:Restriction>
                <owl:onProperty rdf:resource="http://ontologies.ti-semantics.com/score#vector"/>
                <owl:someValuesFrom rdf:resource="http://www.w3.org/2000/01/rdf-schema#Literal"/>
            </owl:Restriction>
        </rdfs:subClassOf>
        <rdfs:comment rdf:datatype="http://www.w3.org/2001/XMLSchema#string">Defines the intrinsic and fundamental characteristics of a vulnerability that are constant with time and across user environments</rdfs:comment>
        <rdfs:isDefinedBy rdf:datatype="http://www.w3.org/2001/XMLSchema#anyURI">https://www.first.org/cvss/cvss-v30-specification-v1.7.pdf</rdfs:isDefinedBy>
        <rdfs:label>CVSS Base Metrics</rdfs:label>
    </owl:Class>
    


    <!-- http://ontologies.ti-semantics.com/score#CVSSv2CollateralDamagePotential -->

    <owl:Class rdf:about="http://ontologies.ti-semantics.com/score#CVSSv2CollateralDamagePotential">
        <rdfs:subClassOf rdf:resource="http://ontologies.ti-semantics.com/score#CVSSv2Metric"/>
        <rdfs:subClassOf rdf:resource="http://ontologies.ti-semantics.com/score#EnvironmentalMetric"/>
        <cvss_v2_code xml:lang="en">CDP</cvss_v2_code>
        <rdfs:comment xml:lang="en">This metric measures the potential for loss of life or physical assets through damage or theft of property or equipment.  The metric may also measure economic loss of productivity or revenue.</rdfs:comment>
        <rdfs:isDefinedBy xml:lang="en">https://www.first.org/cvss/v2/guide#2-3-1-Collateral-Damage-Potential-CDP</rdfs:isDefinedBy>
    </owl:Class>
    


    <!-- http://ontologies.ti-semantics.com/score#CVSSv2CompleteAvailabilityImpact -->

    <owl:Class rdf:about="http://ontologies.ti-semantics.com/score#CVSSv2CompleteAvailabilityImpact">
        <rdfs:subClassOf rdf:resource="http://ontologies.ti-semantics.com/score#CVSSv2AvailabilityImpact"/>
    </owl:Class>
    


    <!-- http://ontologies.ti-semantics.com/score#CVSSv2CompleteConfidentialityImpact -->

    <owl:Class rdf:about="http://ontologies.ti-semantics.com/score#CVSSv2CompleteConfidentialityImpact">
        <rdfs:subClassOf rdf:resource="http://ontologies.ti-semantics.com/score#CVSSv2ConfidentialityImpact"/>
    </owl:Class>
    


    <!-- http://ontologies.ti-semantics.com/score#CVSSv2CompleteIntegrityImpact -->

    <owl:Class rdf:about="http://ontologies.ti-semantics.com/score#CVSSv2CompleteIntegrityImpact">
        <owl:equivalentClass rdf:resource="http://ontologies.ti-semantics.com/score#CVSSv3HighIntegrityImpact"/>
        <rdfs:subClassOf rdf:resource="http://ontologies.ti-semantics.com/score#CVSSv2IntegrityImpact"/>
    </owl:Class>
    


    <!-- http://ontologies.ti-semantics.com/score#CVSSv2ConfidentialityImpact -->

    <owl:Class rdf:about="http://ontologies.ti-semantics.com/score#CVSSv2ConfidentialityImpact">
        <rdfs:subClassOf rdf:resource="http://ontologies.ti-semantics.com/score#CVSSv2Metric"/>
        <rdfs:subClassOf rdf:resource="http://ontologies.ti-semantics.com/score#ImpactMetric"/>
        <cvss_v2_code xml:lang="en">C</cvss_v2_code>
        <rdfs:comment xml:lang="en">This metric measures the impact on confidentiality of a successfully exploited vulnerability. Confidentiality refers to limiting information access and disclosure to only authorized users, as well as preventing access by, or disclosure to, unauthorized ones. The possible values for this metric are listed in Table 4. Increased confidentiality impact increases the vulnerability score.</rdfs:comment>
        <rdfs:isDefinedBy xml:lang="en">https://www.first.org/cvss/v2/guide</rdfs:isDefinedBy>
        <rdfs:label xml:lang="en">Confidentiality Impact</rdfs:label>
    </owl:Class>
    


    <!-- http://ontologies.ti-semantics.com/score#CVSSv2ConfidentialityRequirement -->

    <owl:Class rdf:about="http://ontologies.ti-semantics.com/score#CVSSv2ConfidentialityRequirement">
        <rdfs:subClassOf rdf:resource="http://ontologies.ti-semantics.com/score#SecurityRequirement"/>
        <cvss_v2_code xml:lang="en">CR</cvss_v2_code>
        <cvss_v3_code xml:lang="en">CR</cvss_v3_code>
        <rdfs:comment xml:lang="en">These metrics enable the analyst to customize the CVSS score depending on the importance of the affected IT asset to a user&apos;s organization, measured in terms of Confidentiality. That is, if an IT asset supports a business function for which Confidentiality is most important, the analyst can assign a greater value to Confidentiality relative to Availability and Integrity. This security requirement has three possible values: Low, Medium, or High.

Note that the Confidentiality Requirement will not affect the Environmental score if the (Modified Base) confidentiality impact is set to None. Also, increasing the Confidentiality Requirement from Medium to High will not change the Environmental score when the (Modified Base) impact metrics are set to High. This is because the modified impact sub score (part of the Modified Base score that calculates impact) is already at a maximum value of 10.</rdfs:comment>
        <rdfs:isDefinedBy rdf:datatype="http://www.w3.org/2001/XMLSchema#anyURI">https://www.first.org/cvss/specification-document#4-1-Security-Requirements-CR-IR-AR</rdfs:isDefinedBy>
        <rdfs:isDefinedBy xml:lang="en">https://www.first.org/cvss/v2/guide#2-3-3-Security-Requirements-CR-IR-AR</rdfs:isDefinedBy>
    </owl:Class>
    


    <!-- http://ontologies.ti-semantics.com/score#CVSSv2ConfirmedReportConfidence -->

    <owl:Class rdf:about="http://ontologies.ti-semantics.com/score#CVSSv2ConfirmedReportConfidence">
        <rdfs:subClassOf rdf:resource="http://ontologies.ti-semantics.com/score#CVSSv2ReportConfidence"/>
    </owl:Class>
    


    <!-- http://ontologies.ti-semantics.com/score#CVSSv2EnvironmentalMetricGroup -->

    <owl:Class rdf:about="http://ontologies.ti-semantics.com/score#CVSSv2EnvironmentalMetricGroup">
        <rdfs:subClassOf rdf:resource="http://ontologies.ti-semantics.com/score#CVSSv2MetricGroup"/>
    </owl:Class>
    


    <!-- http://ontologies.ti-semantics.com/score#CVSSv2Exploitability -->

    <owl:Class rdf:about="http://ontologies.ti-semantics.com/score#CVSSv2Exploitability">
        <rdfs:subClassOf rdf:resource="http://ontologies.ti-semantics.com/score#CVSSv2Metric"/>
        <rdfs:subClassOf rdf:resource="http://ontologies.ti-semantics.com/score#TemporalMetric"/>
        <cvss_v2_code xml:lang="en">E</cvss_v2_code>
        <rdfs:comment xml:lang="en">The Exploitability metrics reflect the characteristics of the thing that is vulnerable, which we refer to formally as the vulnerable component. Therefore, each of the Exploitability metrics listed below should be scored relative to the vulnerable component, and reflect the properties of the vulnerability that lead to a successful attack.</rdfs:comment>
        <rdfs:isDefinedBy xml:lang="en">https://www.first.org/cvss/specification-document#2-1-Exploitability-Metrics</rdfs:isDefinedBy>
    </owl:Class>
    


    <!-- http://ontologies.ti-semantics.com/score#CVSSv2FunctionalExploitability -->

    <owl:Class rdf:about="http://ontologies.ti-semantics.com/score#CVSSv2FunctionalExploitability">
        <owl:equivalentClass rdf:resource="http://ontologies.ti-semantics.com/score#CVSSv3FunctionalExploitCodeMaturity"/>
        <rdfs:subClassOf rdf:resource="http://ontologies.ti-semantics.com/score#CVSSv2Exploitability"/>
    </owl:Class>
    


    <!-- http://ontologies.ti-semantics.com/score#CVSSv2HighAccessComplexity -->

    <owl:Class rdf:about="http://ontologies.ti-semantics.com/score#CVSSv2HighAccessComplexity">
        <rdfs:subClassOf rdf:resource="http://ontologies.ti-semantics.com/score#CVSSv2AccessComplexity"/>
    </owl:Class>
    


    <!-- http://ontologies.ti-semantics.com/score#CVSSv2HighAvailabilityRequirement -->

    <owl:Class rdf:about="http://ontologies.ti-semantics.com/score#CVSSv2HighAvailabilityRequirement">
        <owl:equivalentClass rdf:resource="http://ontologies.ti-semantics.com/score#CVSSv3HighAvailabilityRequirement"/>
        <rdfs:subClassOf rdf:resource="http://ontologies.ti-semantics.com/score#CVSSv2AvailabilityRequirement"/>
    </owl:Class>
    


    <!-- http://ontologies.ti-semantics.com/score#CVSSv2HighCollateralDamagePotential -->

    <owl:Class rdf:about="http://ontologies.ti-semantics.com/score#CVSSv2HighCollateralDamagePotential">
        <rdfs:subClassOf rdf:resource="http://ontologies.ti-semantics.com/score#CVSSv2CollateralDamagePotential"/>
    </owl:Class>
    


    <!-- http://ontologies.ti-semantics.com/score#CVSSv2HighConfidentialityRequirement -->

    <owl:Class rdf:about="http://ontologies.ti-semantics.com/score#CVSSv2HighConfidentialityRequirement">
        <owl:equivalentClass rdf:resource="http://ontologies.ti-semantics.com/score#CVSSv3HighConfidentialityRequirement"/>
        <rdfs:subClassOf rdf:resource="http://ontologies.ti-semantics.com/score#CVSSv2ConfidentialityRequirement"/>
    </owl:Class>
    


    <!-- http://ontologies.ti-semantics.com/score#CVSSv2HighExploitability -->

    <owl:Class rdf:about="http://ontologies.ti-semantics.com/score#CVSSv2HighExploitability">
        <owl:equivalentClass rdf:resource="http://ontologies.ti-semantics.com/score#CVSSv3HighExploitCodeMaturity"/>
        <rdfs:subClassOf rdf:resource="http://ontologies.ti-semantics.com/score#CVSSv2Exploitability"/>
    </owl:Class>
    


    <!-- http://ontologies.ti-semantics.com/score#CVSSv2HighIntegrityRequirement -->

    <owl:Class rdf:about="http://ontologies.ti-semantics.com/score#CVSSv2HighIntegrityRequirement">
        <owl:equivalentClass rdf:resource="http://ontologies.ti-semantics.com/score#CVSSv3HighIntegrityRequirement"/>
        <rdfs:subClassOf rdf:resource="http://ontologies.ti-semantics.com/score#CVSSv2IntegrityRequirement"/>
    </owl:Class>
    


    <!-- http://ontologies.ti-semantics.com/score#CVSSv2HighTargetCount -->

    <owl:Class rdf:about="http://ontologies.ti-semantics.com/score#CVSSv2HighTargetCount">
        <rdfs:subClassOf rdf:resource="http://ontologies.ti-semantics.com/score#CVSSv2TargetDistribution"/>
    </owl:Class>
    


    <!-- http://ontologies.ti-semantics.com/score#CVSSv2IntegrityImpact -->

    <owl:Class rdf:about="http://ontologies.ti-semantics.com/score#CVSSv2IntegrityImpact">
        <rdfs:subClassOf rdf:resource="http://ontologies.ti-semantics.com/score#CVSSv2Metric"/>
        <rdfs:subClassOf rdf:resource="http://ontologies.ti-semantics.com/score#ImpactMetric"/>
        <cvss_v3_code>I</cvss_v3_code>
        <rdfs:comment xml:lang="en">This metric measures the impact to integrity of a successfully exploited vulnerability. Integrity refers to the trustworthiness and veracity of information. This metric value increases with the consequence to the impacted component.</rdfs:comment>
        <rdfs:isDefinedBy rdf:datatype="http://www.w3.org/2001/XMLSchema#anyURI">https://www.first.org/cvss/specification-document#2-3-2-Integrity-Impact-I</rdfs:isDefinedBy>
        <rdfs:label xml:lang="en">Integrity Impact</rdfs:label>
    </owl:Class>
    


    <!-- http://ontologies.ti-semantics.com/score#CVSSv2IntegrityRequirement -->

    <owl:Class rdf:about="http://ontologies.ti-semantics.com/score#CVSSv2IntegrityRequirement">
        <rdfs:subClassOf rdf:resource="http://ontologies.ti-semantics.com/score#SecurityRequirement"/>
        <cvss_v2_code xml:lang="en">CR</cvss_v2_code>
        <rdfs:comment xml:lang="en">This metric enables the analyst to customize the CVSS score depending on the importance of the affected IT asset to a user&apos;s organization, measured in terms of Integrity. That is, if an IT asset supports a business function for which Integrityis most important, the analyst can assign a greater value to Integrity relative to Confidentiality and Availability. Each security requirement has three possible values: Low, Medium, or High.</rdfs:comment>
        <rdfs:isDefinedBy xml:lang="en">https://www.first.org/cvss/specification-document#4-1-Security-Requirements-CR-IR-AR</rdfs:isDefinedBy>
        <rdfs:isDefinedBy xml:lang="en">https://www.first.org/cvss/v2/guide#2-3-3-Security-Requirements-CR-IR-AR</rdfs:isDefinedBy>
    </owl:Class>
    


    <!-- http://ontologies.ti-semantics.com/score#CVSSv2LocalAccessVector -->

    <owl:Class rdf:about="http://ontologies.ti-semantics.com/score#CVSSv2LocalAccessVector">
        <rdfs:subClassOf rdf:resource="http://ontologies.ti-semantics.com/score#CVSSv2AccessVector"/>
    </owl:Class>
    


    <!-- http://ontologies.ti-semantics.com/score#CVSSv2LowAccessComplexity -->

    <owl:Class rdf:about="http://ontologies.ti-semantics.com/score#CVSSv2LowAccessComplexity">
        <rdfs:subClassOf rdf:resource="http://ontologies.ti-semantics.com/score#CVSSv2AccessComplexity"/>
    </owl:Class>
    


    <!-- http://ontologies.ti-semantics.com/score#CVSSv2LowAvailabilityRequirement -->

    <owl:Class rdf:about="http://ontologies.ti-semantics.com/score#CVSSv2LowAvailabilityRequirement">
        <owl:equivalentClass rdf:resource="http://ontologies.ti-semantics.com/score#CVSSv3LowAvailabilityRequirement"/>
        <rdfs:subClassOf rdf:resource="http://ontologies.ti-semantics.com/score#CVSSv2AvailabilityRequirement"/>
    </owl:Class>
    


    <!-- http://ontologies.ti-semantics.com/score#CVSSv2LowCollateralDamagePotential -->

    <owl:Class rdf:about="http://ontologies.ti-semantics.com/score#CVSSv2LowCollateralDamagePotential">
        <rdfs:subClassOf rdf:resource="http://ontologies.ti-semantics.com/score#CVSSv2CollateralDamagePotential"/>
    </owl:Class>
    


    <!-- http://ontologies.ti-semantics.com/score#CVSSv2LowConfidentialityRequirement -->

    <owl:Class rdf:about="http://ontologies.ti-semantics.com/score#CVSSv2LowConfidentialityRequirement">
        <owl:equivalentClass rdf:resource="http://ontologies.ti-semantics.com/score#CVSSv3LowConfidentialityRequirement"/>
        <rdfs:subClassOf rdf:resource="http://ontologies.ti-semantics.com/score#CVSSv2ConfidentialityRequirement"/>
    </owl:Class>
    


    <!-- http://ontologies.ti-semantics.com/score#CVSSv2LowIntegrityRequirement -->

    <owl:Class rdf:about="http://ontologies.ti-semantics.com/score#CVSSv2LowIntegrityRequirement">
        <owl:equivalentClass rdf:resource="http://ontologies.ti-semantics.com/score#CVSSv3LowIntegrityRequirement"/>
        <rdfs:subClassOf rdf:resource="http://ontologies.ti-semantics.com/score#CVSSv2IntegrityRequirement"/>
    </owl:Class>
    


    <!-- http://ontologies.ti-semantics.com/score#CVSSv2LowMediumCollateralDamagePotential -->

    <owl:Class rdf:about="http://ontologies.ti-semantics.com/score#CVSSv2LowMediumCollateralDamagePotential">
        <rdfs:subClassOf rdf:resource="http://ontologies.ti-semantics.com/score#CVSSv2CollateralDamagePotential"/>
    </owl:Class>
    


    <!-- http://ontologies.ti-semantics.com/score#CVSSv2LowTargetCount -->

    <owl:Class rdf:about="http://ontologies.ti-semantics.com/score#CVSSv2LowTargetCount">
        <rdfs:subClassOf rdf:resource="http://ontologies.ti-semantics.com/score#CVSSv2TargetDistribution"/>
    </owl:Class>
    


    <!-- http://ontologies.ti-semantics.com/score#CVSSv2MediumAccessComplexity -->

    <owl:Class rdf:about="http://ontologies.ti-semantics.com/score#CVSSv2MediumAccessComplexity">
        <rdfs:subClassOf rdf:resource="http://ontologies.ti-semantics.com/score#CVSSv2AccessComplexity"/>
        <cvss_v2_code>M</cvss_v2_code>
        <rdfs:comment xml:lang="en">The access conditions are somewhat specialized; the following are examples:
- The attacking party is limited to a group of systems or users at some level of authorization, possibly untrusted.
- Some information must be gathered before a successful attack can be launched.
- The affected configuration is non-default, and is not commonly configured (e.g., a vulnerability present when a server performs user account authentication via a specific scheme, but not present for another authentication scheme).
- The attack requires a small amount of social engineering that might occasionally fool cautious users (e.g., phishing attacks that modify a web browsers status bar to show a false link, having to be on someones buddy list before sending an IM exploit).</rdfs:comment>
        <rdfs:isDefinedBy xml:lang="en">https://www.first.org/cvss/v2/guide#2-1-2-Access-Complexity-AC</rdfs:isDefinedBy>
        <rdfs:label xml:lang="en">Medium</rdfs:label>
    </owl:Class>
    


    <!-- http://ontologies.ti-semantics.com/score#CVSSv2MediumAvailabilityRequirement -->

    <owl:Class rdf:about="http://ontologies.ti-semantics.com/score#CVSSv2MediumAvailabilityRequirement">
        <owl:equivalentClass rdf:resource="http://ontologies.ti-semantics.com/score#CVSSv3MediumAvailabilityRequirement"/>
        <rdfs:subClassOf rdf:resource="http://ontologies.ti-semantics.com/score#CVSSv2AvailabilityRequirement"/>
    </owl:Class>
    


    <!-- http://ontologies.ti-semantics.com/score#CVSSv2MediumConfidentialityRequirement -->

    <owl:Class rdf:about="http://ontologies.ti-semantics.com/score#CVSSv2MediumConfidentialityRequirement">
        <owl:equivalentClass rdf:resource="http://ontologies.ti-semantics.com/score#CVSSv3MediumConfidentialityRequirement"/>
        <rdfs:subClassOf rdf:resource="http://ontologies.ti-semantics.com/score#CVSSv2ConfidentialityRequirement"/>
    </owl:Class>
    


    <!-- http://ontologies.ti-semantics.com/score#CVSSv2MediumHighCollateralDamagePotential -->

    <owl:Class rdf:about="http://ontologies.ti-semantics.com/score#CVSSv2MediumHighCollateralDamagePotential">
        <rdfs:subClassOf rdf:resource="http://ontologies.ti-semantics.com/score#CVSSv2CollateralDamagePotential"/>
    </owl:Class>
    


    <!-- http://ontologies.ti-semantics.com/score#CVSSv2MediumIntegrityRequirement -->

    <owl:Class rdf:about="http://ontologies.ti-semantics.com/score#CVSSv2MediumIntegrityRequirement">
        <owl:equivalentClass rdf:resource="http://ontologies.ti-semantics.com/score#CVSSv3MediumIntegrityRequirement"/>
        <rdfs:subClassOf rdf:resource="http://ontologies.ti-semantics.com/score#CVSSv2IntegrityRequirement"/>
    </owl:Class>
    


    <!-- http://ontologies.ti-semantics.com/score#CVSSv2MediumTargetCount -->

    <owl:Class rdf:about="http://ontologies.ti-semantics.com/score#CVSSv2MediumTargetCount">
        <rdfs:subClassOf rdf:resource="http://ontologies.ti-semantics.com/score#CVSSv2TargetDistribution"/>
    </owl:Class>
    


    <!-- http://ontologies.ti-semantics.com/score#CVSSv2Metric -->

    <owl:Class rdf:about="http://ontologies.ti-semantics.com/score#CVSSv2Metric">
        <rdfs:subClassOf rdf:resource="http://ontologies.ti-semantics.com/score#CVSSMetric"/>
        <rdfs:comment xml:lang="en">The Common Vulnerability Scoring System (CVSS) provides an open framework for communicating the characteristics and impacts of IT vulnerabilities. CVSS consists of 3 groups: Base, Temporal and Environmental. Each group produces a numeric score ranging from 0 to 10, and a Vector, a compressed textual representation that reflects the values used to derive the score. The Base group represents the intrinsic qualities of a vulnerability. The Temporal group reflects the characteristics of a vulnerability that change over time. The Environmental group represents the characteristics of a vulnerability that are unique to any user&apos;s environment. CVSS enables IT managers, vulnerability bulletin providers, security vendors, application vendors and researchers to all benefit by adopting this common language of scoring IT vulnerabilities.</rdfs:comment>
    </owl:Class>
    


    <!-- http://ontologies.ti-semantics.com/score#CVSSv2MetricGroup -->

    <owl:Class rdf:about="http://ontologies.ti-semantics.com/score#CVSSv2MetricGroup">
        <rdfs:subClassOf rdf:resource="http://ontologies.ti-semantics.com/score#CVSSMetricGroup"/>
    </owl:Class>
    


    <!-- http://ontologies.ti-semantics.com/score#CVSSv2MultipleAuthentications -->

    <owl:Class rdf:about="http://ontologies.ti-semantics.com/score#CVSSv2MultipleAuthentications">
        <rdfs:subClassOf rdf:resource="http://ontologies.ti-semantics.com/score#CVSSv2Authentication"/>
    </owl:Class>
    


    <!-- http://ontologies.ti-semantics.com/score#CVSSv2NetworkAccessVector -->

    <owl:Class rdf:about="http://ontologies.ti-semantics.com/score#CVSSv2NetworkAccessVector">
        <rdfs:subClassOf rdf:resource="http://ontologies.ti-semantics.com/score#CVSSv2AccessVector"/>
    </owl:Class>
    


    <!-- http://ontologies.ti-semantics.com/score#CVSSv2NilTargetCount -->

    <owl:Class rdf:about="http://ontologies.ti-semantics.com/score#CVSSv2NilTargetCount">
        <rdfs:subClassOf rdf:resource="http://ontologies.ti-semantics.com/score#CVSSv2TargetDistribution"/>
    </owl:Class>
    


    <!-- http://ontologies.ti-semantics.com/score#CVSSv2NoAuthentication -->

    <owl:Class rdf:about="http://ontologies.ti-semantics.com/score#CVSSv2NoAuthentication">
        <rdfs:subClassOf rdf:resource="http://ontologies.ti-semantics.com/score#CVSSv2Authentication"/>
    </owl:Class>
    


    <!-- http://ontologies.ti-semantics.com/score#CVSSv2NoAvailabilityImpact -->

    <owl:Class rdf:about="http://ontologies.ti-semantics.com/score#CVSSv2NoAvailabilityImpact">
        <rdfs:subClassOf rdf:resource="http://ontologies.ti-semantics.com/score#CVSSv2AvailabilityImpact"/>
    </owl:Class>
    


    <!-- http://ontologies.ti-semantics.com/score#CVSSv2NoCollateralDamagePotential -->

    <owl:Class rdf:about="http://ontologies.ti-semantics.com/score#CVSSv2NoCollateralDamagePotential">
        <rdfs:subClassOf rdf:resource="http://ontologies.ti-semantics.com/score#CVSSv2CollateralDamagePotential"/>
    </owl:Class>
    


    <!-- http://ontologies.ti-semantics.com/score#CVSSv2NoConfidentialityImpact -->

    <owl:Class rdf:about="http://ontologies.ti-semantics.com/score#CVSSv2NoConfidentialityImpact">
        <rdfs:subClassOf rdf:resource="http://ontologies.ti-semantics.com/score#CVSSv2ConfidentialityImpact"/>
    </owl:Class>
    


    <!-- http://ontologies.ti-semantics.com/score#CVSSv2NoIntegrityImpact -->

    <owl:Class rdf:about="http://ontologies.ti-semantics.com/score#CVSSv2NoIntegrityImpact">
        <owl:equivalentClass rdf:resource="http://ontologies.ti-semantics.com/score#CVSSv3NoIntegrityImpact"/>
        <rdfs:subClassOf rdf:resource="http://ontologies.ti-semantics.com/score#CVSSv2IntegrityImpact"/>
    </owl:Class>
    


    <!-- http://ontologies.ti-semantics.com/score#CVSSv2NotDefinedAvailabilityRequirement -->

    <owl:Class rdf:about="http://ontologies.ti-semantics.com/score#CVSSv2NotDefinedAvailabilityRequirement">
        <owl:equivalentClass rdf:resource="http://ontologies.ti-semantics.com/score#CVSSv3NotDefinedAvailabilityRequirement"/>
        <rdfs:subClassOf rdf:resource="http://ontologies.ti-semantics.com/score#CVSSv2AvailabilityRequirement"/>
    </owl:Class>
    


    <!-- http://ontologies.ti-semantics.com/score#CVSSv2NotDefinedCollateralDamagePotential -->

    <owl:Class rdf:about="http://ontologies.ti-semantics.com/score#CVSSv2NotDefinedCollateralDamagePotential">
        <rdfs:subClassOf rdf:resource="http://ontologies.ti-semantics.com/score#CVSSv2CollateralDamagePotential"/>
    </owl:Class>
    


    <!-- http://ontologies.ti-semantics.com/score#CVSSv2NotDefinedConfidentialityRequirement -->

    <owl:Class rdf:about="http://ontologies.ti-semantics.com/score#CVSSv2NotDefinedConfidentialityRequirement">
        <owl:equivalentClass rdf:resource="http://ontologies.ti-semantics.com/score#CVSSv3NotDefinedConfidentialityRequirement"/>
        <rdfs:subClassOf rdf:resource="http://ontologies.ti-semantics.com/score#CVSSv2ConfidentialityRequirement"/>
    </owl:Class>
    


    <!-- http://ontologies.ti-semantics.com/score#CVSSv2NotDefinedExploitability -->

    <owl:Class rdf:about="http://ontologies.ti-semantics.com/score#CVSSv2NotDefinedExploitability">
        <owl:equivalentClass rdf:resource="http://ontologies.ti-semantics.com/score#CVSSv3NotDefinedExploitCodeMaturity"/>
        <rdfs:subClassOf rdf:resource="http://ontologies.ti-semantics.com/score#CVSSv2Exploitability"/>
    </owl:Class>
    


    <!-- http://ontologies.ti-semantics.com/score#CVSSv2NotDefinedIntegrityRequirement -->

    <owl:Class rdf:about="http://ontologies.ti-semantics.com/score#CVSSv2NotDefinedIntegrityRequirement">
        <owl:equivalentClass rdf:resource="http://ontologies.ti-semantics.com/score#CVSSv3NotDefinedIntegrityRequirement"/>
        <rdfs:subClassOf rdf:resource="http://ontologies.ti-semantics.com/score#CVSSv2IntegrityRequirement"/>
    </owl:Class>
    


    <!-- http://ontologies.ti-semantics.com/score#CVSSv2NotDefinedRemediation -->

    <owl:Class rdf:about="http://ontologies.ti-semantics.com/score#CVSSv2NotDefinedRemediation">
        <rdfs:subClassOf rdf:resource="http://ontologies.ti-semantics.com/score#CVSSv2RemediationLevel"/>
    </owl:Class>
    


    <!-- http://ontologies.ti-semantics.com/score#CVSSv2NotDefinedReportConfidence -->

    <owl:Class rdf:about="http://ontologies.ti-semantics.com/score#CVSSv2NotDefinedReportConfidence">
        <rdfs:subClassOf rdf:resource="http://ontologies.ti-semantics.com/score#CVSSv2ReportConfidence"/>
        <cvss_v2_code>ND</cvss_v2_code>
        <rdfs:comment xml:lang="en">Assigning this value to the metric will not influence the score. It is a signal to a scoring equation to skip this metric.</rdfs:comment>
        <rdfs:isDefinedBy rdf:datatype="http://www.w3.org/2001/XMLSchema#anyURI">https://www.first.org/cvss/v2/guide#2-2-2-Remediation-Level-RL</rdfs:isDefinedBy>
        <rdfs:label xml:lang="en">Not Defined</rdfs:label>
    </owl:Class>
    


    <!-- http://ontologies.ti-semantics.com/score#CVSSv2NotDefinedTargetCount -->

    <owl:Class rdf:about="http://ontologies.ti-semantics.com/score#CVSSv2NotDefinedTargetCount">
        <rdfs:subClassOf rdf:resource="http://ontologies.ti-semantics.com/score#CVSSv2TargetDistribution"/>
    </owl:Class>
    


    <!-- http://ontologies.ti-semantics.com/score#CVSSv2OfficialFixRemediation -->

    <owl:Class rdf:about="http://ontologies.ti-semantics.com/score#CVSSv2OfficialFixRemediation">
        <rdfs:subClassOf rdf:resource="http://ontologies.ti-semantics.com/score#CVSSv2RemediationLevel"/>
    </owl:Class>
    


    <!-- http://ontologies.ti-semantics.com/score#CVSSv2PartialAvailabilityImpact -->

    <owl:Class rdf:about="http://ontologies.ti-semantics.com/score#CVSSv2PartialAvailabilityImpact">
        <rdfs:subClassOf rdf:resource="http://ontologies.ti-semantics.com/score#CVSSv2AvailabilityImpact"/>
    </owl:Class>
    


    <!-- http://ontologies.ti-semantics.com/score#CVSSv2PartialConfidentialityImpact -->

    <owl:Class rdf:about="http://ontologies.ti-semantics.com/score#CVSSv2PartialConfidentialityImpact">
        <rdfs:subClassOf rdf:resource="http://ontologies.ti-semantics.com/score#CVSSv2ConfidentialityImpact"/>
    </owl:Class>
    


    <!-- http://ontologies.ti-semantics.com/score#CVSSv2PartialIntegrityImpact -->

    <owl:Class rdf:about="http://ontologies.ti-semantics.com/score#CVSSv2PartialIntegrityImpact">
        <owl:equivalentClass rdf:resource="http://ontologies.ti-semantics.com/score#CVSSv3LowIntegrityImpact"/>
        <rdfs:subClassOf rdf:resource="http://ontologies.ti-semantics.com/score#CVSSv2IntegrityImpact"/>
    </owl:Class>
    


    <!-- http://ontologies.ti-semantics.com/score#CVSSv2ProofOfConceptExploitability -->

    <owl:Class rdf:about="http://ontologies.ti-semantics.com/score#CVSSv2ProofOfConceptExploitability">
        <owl:equivalentClass rdf:resource="http://ontologies.ti-semantics.com/score#CVSSv3ProofOfConceptExploitCodeMaturity"/>
        <rdfs:subClassOf rdf:resource="http://ontologies.ti-semantics.com/score#CVSSv2Exploitability"/>
    </owl:Class>
    


    <!-- http://ontologies.ti-semantics.com/score#CVSSv2RemediationLevel -->

    <owl:Class rdf:about="http://ontologies.ti-semantics.com/score#CVSSv2RemediationLevel">
        <rdfs:subClassOf rdf:resource="http://ontologies.ti-semantics.com/score#CVSSv2Metric"/>
        <rdfs:subClassOf rdf:resource="http://ontologies.ti-semantics.com/score#TemporalMetric"/>
        <cvss_v2_code xml:lang="en">RL</cvss_v2_code>
        <cvss_v3_code xml:lang="en">RL</cvss_v3_code>
        <rdfs:comment xml:lang="en">The Remediation Level of a vulnerability is an important factor for prioritization. The typical vulnerability is unpatched when initially published. Workarounds or hotfixes may offer interim remediation until an official patch or upgrade is issued. Each of these respective stages adjusts the temporal score downwards, reflecting the decreasing urgency as remediation becomes final. The less official and permanent a fix, the higher the vulnerability score.</rdfs:comment>
        <rdfs:isDefinedBy rdf:datatype="http://www.w3.org/2001/XMLSchema#anyURI">https://www.first.org/cvss/specification-document#3-2-Remediation-Level-RL</rdfs:isDefinedBy>
        <rdfs:isDefinedBy xml:lang="en">https://www.first.org/cvss/v2/guide#2-2-2-Remediation-Level-RL</rdfs:isDefinedBy>
        <rdfs:label xml:lang="en">Remediation Level</rdfs:label>
    </owl:Class>
    


    <!-- http://ontologies.ti-semantics.com/score#CVSSv2ReportConfidence -->

    <owl:Class rdf:about="http://ontologies.ti-semantics.com/score#CVSSv2ReportConfidence">
        <rdfs:subClassOf rdf:resource="http://ontologies.ti-semantics.com/score#CVSSv2Metric"/>
        <rdfs:subClassOf rdf:resource="http://ontologies.ti-semantics.com/score#TemporalMetric"/>
        <cvss_v2_code xml:lang="en">RC</cvss_v2_code>
        <rdfs:comment xml:lang="en">This metric measures the degree of confidence in the existence of the vulnerability and the credibility of the known technical details. Sometimes only the existence of vulnerabilities are publicized, but without specific details. For example, an impact may be recognized as undesirable, but the root cause may not be known. The vulnerability may later be corroborated by research which suggests where the vulnerability may lie, though the research may not be certain. Finally, a vulnerability may be confirmed through acknowledgement by the author or vendor of the affected technology. The urgency of a vulnerability is higher when a vulnerability is known to exist with certainty. This metric also suggests the level of technical knowledge available to would-be attackers. The more a vulnerability is validated by the vendor or other reputable sources, the higher the score.</rdfs:comment>
        <rdfs:isDefinedBy xml:lang="en">https://www.first.org/cvss/v2/guide#2-2-3-Report-Confidence-RC</rdfs:isDefinedBy>
        <rdfs:label xml:lang="en">Report Confidence</rdfs:label>
    </owl:Class>
    


    <!-- http://ontologies.ti-semantics.com/score#CVSSv2SingleAuthentication -->

    <owl:Class rdf:about="http://ontologies.ti-semantics.com/score#CVSSv2SingleAuthentication">
        <rdfs:subClassOf rdf:resource="http://ontologies.ti-semantics.com/score#CVSSv2Authentication"/>
    </owl:Class>
    


    <!-- http://ontologies.ti-semantics.com/score#CVSSv2TargetDistribution -->

    <owl:Class rdf:about="http://ontologies.ti-semantics.com/score#CVSSv2TargetDistribution">
        <rdfs:subClassOf rdf:resource="http://ontologies.ti-semantics.com/score#CVSSv2Metric"/>
        <rdfs:subClassOf rdf:resource="http://ontologies.ti-semantics.com/score#EnvironmentalMetric"/>
        <cvss_v2_code xml:lang="en">TD</cvss_v2_code>
        <rdfs:comment xml:lang="en">This metric measures the proportion of vulnerable systems. It is meant as an environment-specific indicator in order to approximate the percentage of systems that could be affected by the vulnerability.</rdfs:comment>
        <rdfs:isDefinedBy xml:lang="en">https://www.first.org/cvss/v2/guide#2-3-2-Target-Distribution-TD</rdfs:isDefinedBy>
    </owl:Class>
    


    <!-- http://ontologies.ti-semantics.com/score#CVSSv2TemporalMetricGroup -->

    <owl:Class rdf:about="http://ontologies.ti-semantics.com/score#CVSSv2TemporalMetricGroup">
        <rdfs:subClassOf rdf:resource="http://ontologies.ti-semantics.com/score#CVSSv2MetricGroup"/>
    </owl:Class>
    


    <!-- http://ontologies.ti-semantics.com/score#CVSSv2TemporaryFixRemediation -->

    <owl:Class rdf:about="http://ontologies.ti-semantics.com/score#CVSSv2TemporaryFixRemediation">
        <rdfs:subClassOf rdf:resource="http://ontologies.ti-semantics.com/score#CVSSv2RemediationLevel"/>
    </owl:Class>
    


    <!-- http://ontologies.ti-semantics.com/score#CVSSv2UnavailableRemediation -->

    <owl:Class rdf:about="http://ontologies.ti-semantics.com/score#CVSSv2UnavailableRemediation">
        <rdfs:subClassOf rdf:resource="http://ontologies.ti-semantics.com/score#CVSSv2RemediationLevel"/>
    </owl:Class>
    


    <!-- http://ontologies.ti-semantics.com/score#CVSSv2UnconfirmedReportConfidence -->

    <owl:Class rdf:about="http://ontologies.ti-semantics.com/score#CVSSv2UnconfirmedReportConfidence">
        <owl:equivalentClass rdf:resource="http://ontologies.ti-semantics.com/score#CVSSv3UnknownReportConfidence"/>
        <rdfs:subClassOf rdf:resource="http://ontologies.ti-semantics.com/score#CVSSv2ReportConfidence"/>
    </owl:Class>
    


    <!-- http://ontologies.ti-semantics.com/score#CVSSv2UncorroboratedReportConfidence -->

    <owl:Class rdf:about="http://ontologies.ti-semantics.com/score#CVSSv2UncorroboratedReportConfidence">
        <rdfs:subClassOf rdf:resource="http://ontologies.ti-semantics.com/score#CVSSv2ReportConfidence"/>
    </owl:Class>
    


    <!-- http://ontologies.ti-semantics.com/score#CVSSv2UnprovenExploitability -->

    <owl:Class rdf:about="http://ontologies.ti-semantics.com/score#CVSSv2UnprovenExploitability">
        <owl:equivalentClass rdf:resource="http://ontologies.ti-semantics.com/score#CVSSv3UnprovenExploitCodeMaturity"/>
        <rdfs:subClassOf rdf:resource="http://ontologies.ti-semantics.com/score#CVSSv2Exploitability"/>
    </owl:Class>
    


    <!-- http://ontologies.ti-semantics.com/score#CVSSv2WorkaroundRemediation -->

    <owl:Class rdf:about="http://ontologies.ti-semantics.com/score#CVSSv2WorkaroundRemediation">
        <rdfs:subClassOf rdf:resource="http://ontologies.ti-semantics.com/score#CVSSv2RemediationLevel"/>
    </owl:Class>
    


    <!-- http://ontologies.ti-semantics.com/score#CVSSv3AdjacentAttackVector -->

    <owl:Class rdf:about="http://ontologies.ti-semantics.com/score#CVSSv3AdjacentAttackVector">
        <rdfs:subClassOf rdf:resource="http://ontologies.ti-semantics.com/score#CVSSv3AttackVector"/>
    </owl:Class>
    


    <!-- http://ontologies.ti-semantics.com/score#CVSSv3AttackComplexity -->

    <owl:Class rdf:about="http://ontologies.ti-semantics.com/score#CVSSv3AttackComplexity">
        <rdfs:subClassOf rdf:resource="http://ontologies.ti-semantics.com/score#CVSSv3Metric"/>
        <rdfs:subClassOf rdf:resource="http://ontologies.ti-semantics.com/score#ExploitabilityMetric"/>
        <cvss_v2_code xml:lang="en">AC</cvss_v2_code>
        <cvss_v3_code>AC</cvss_v3_code>
        <rdfs:comment xml:lang="en">This metric describes the conditions beyond the attacker’s control that must exist in order to exploit the vulnerability. As described below, such conditions may require the collection of more information about the target, the presence of certain system configuration settings, or computational exceptions. Importantly, the assessment of this metric excludes any requirements for user interaction in order to exploit the vulnerability (such conditions are captured in the User Interaction metric). This metric value is largest for the least complex attacks.</rdfs:comment>
        <rdfs:isDefinedBy rdf:datatype="http://www.w3.org/2001/XMLSchema#anyURI">https://www.first.org/cvss/specification-document#2-1-2-Attack-Complexity-AC</rdfs:isDefinedBy>
        <rdfs:isDefinedBy xml:lang="en">https://www.first.org/cvss/v2/guide#2-1-2-Access-Complexity-AC</rdfs:isDefinedBy>
        <rdfs:label xml:lang="en">Attack Complexity</rdfs:label>
    </owl:Class>
    


    <!-- http://ontologies.ti-semantics.com/score#CVSSv3AttackVector -->

    <owl:Class rdf:about="http://ontologies.ti-semantics.com/score#CVSSv3AttackVector">
        <rdfs:subClassOf rdf:resource="http://ontologies.ti-semantics.com/score#CVSSv3Metric"/>
        <rdfs:subClassOf rdf:resource="http://ontologies.ti-semantics.com/score#ExploitabilityMetric"/>
        <cvss_v3_code>AV</cvss_v3_code>
        <rdfs:comment xml:lang="en">This metric reflects the context by which vulnerability exploitation is possible. This metric value (and consequently the Base score) will be larger the more remote (logically, and physically) an attacker can be in order to exploit the vulnerable component. The assumption is that the number of potential attackers for a vulnerability that could be exploited from across the Internet is larger than the number of potential attackers that could exploit a vulnerability requiring physical access to a device, and therefore warrants a greater score.</rdfs:comment>
        <rdfs:isDefinedBy rdf:datatype="http://www.w3.org/2001/XMLSchema#anyURI">https://www.first.org/cvss/specification-document#2-1-1-Attack-Vector-AV</rdfs:isDefinedBy>
        <rdfs:label xml:lang="en">Attack Vector</rdfs:label>
    </owl:Class>
    


    <!-- http://ontologies.ti-semantics.com/score#CVSSv3AvailabilityImpact -->

    <owl:Class rdf:about="http://ontologies.ti-semantics.com/score#CVSSv3AvailabilityImpact">
        <rdfs:subClassOf rdf:resource="http://ontologies.ti-semantics.com/score#CVSSv3Metric"/>
        <rdfs:subClassOf rdf:resource="http://ontologies.ti-semantics.com/score#ImpactMetric"/>
        <cvss_v3_code>AI</cvss_v3_code>
        <rdfs:comment xml:lang="en">This metric measures the impact to the availability of the impacted component resulting from a successfully exploited vulnerability. While the Confidentiality and Integrity impact metrics apply to the loss of confidentiality or integrity of data (e.g., information, files) used by the impacted component, this metric refers to the loss of availability of the impacted component itself, such as a networked service (e.g., web, database, email). Since availability refers to the accessibility of information resources, attacks that consume network bandwidth, processor cycles, or disk space all impact the availability of an impacted component. This metric value increases with the consequence to the impacted component.</rdfs:comment>
        <rdfs:isDefinedBy rdf:datatype="http://www.w3.org/2001/XMLSchema#anyURI">https://www.first.org/cvss/cvss-v30-specification-v1.7.pdf</rdfs:isDefinedBy>
        <rdfs:label xml:lang="en">Availability Impact</rdfs:label>
    </owl:Class>
    


    <!-- http://ontologies.ti-semantics.com/score#CVSSv3AvailabilityRequirement -->

    <owl:Class rdf:about="http://ontologies.ti-semantics.com/score#CVSSv3AvailabilityRequirement">
        <rdfs:subClassOf rdf:resource="http://ontologies.ti-semantics.com/score#CVSSv3Metric"/>
        <rdfs:subClassOf rdf:resource="http://ontologies.ti-semantics.com/score#SecurityRequirement"/>
        <cvss_v3_code xml:lang="en">AR</cvss_v3_code>
        <rdfs:comment xml:lang="en">These metrics enable the analyst to customize the CVSS score depending on the importance of the affected IT asset to a user&apos;s organization, measured in terms of Availability. That is, if an IT asset supports a business function for which Availability is most important, the analyst can assign a greater value to Availability relative to Confidentiality and Integrity. Each security requirement has three possible values: Low, Medium, or High.</rdfs:comment>
        <rdfs:isDefinedBy xml:lang="en">https://www.first.org/cvss/specification-document#4-1-Security-Requirements-CR-IR-AR</rdfs:isDefinedBy>
    </owl:Class>
    


    <!-- http://ontologies.ti-semantics.com/score#CVSSv3BaseMetricGroup -->

    <owl:Class rdf:about="http://ontologies.ti-semantics.com/score#CVSSv3BaseMetricGroup">
        <rdfs:subClassOf rdf:resource="http://ontologies.ti-semantics.com/score#CVSSv3MetricGroup"/>
    </owl:Class>
    


    <!-- http://ontologies.ti-semantics.com/score#CVSSv3ChangedScope -->

    <owl:Class rdf:about="http://ontologies.ti-semantics.com/score#CVSSv3ChangedScope">
        <rdfs:subClassOf rdf:resource="http://ontologies.ti-semantics.com/score#CVSSv3Scope"/>
    </owl:Class>
    


    <!-- http://ontologies.ti-semantics.com/score#CVSSv3ConfidentialityImpact -->

    <owl:Class rdf:about="http://ontologies.ti-semantics.com/score#CVSSv3ConfidentialityImpact">
        <rdfs:subClassOf rdf:resource="http://ontologies.ti-semantics.com/score#CVSSv3Metric"/>
        <rdfs:subClassOf rdf:resource="http://ontologies.ti-semantics.com/score#ImpactMetric"/>
        <cvss_v3_code>C</cvss_v3_code>
        <rdfs:comment xml:lang="en">This metric measures the impact to the confidentiality of the information resources managed by a software component due to a successfully exploited vulnerability. Confidentiality refers to limiting information access and disclosure to only authorized users, as well as preventing access by, or disclosure to, unauthorized ones. This metric value increases with the degree of loss to the impacted component.</rdfs:comment>
        <rdfs:isDefinedBy rdf:datatype="http://www.w3.org/2001/XMLSchema#anyURI">https://www.first.org/cvss/cvss-v30-specification-v1.7.pdf</rdfs:isDefinedBy>
        <rdfs:label xml:lang="en">Confidentiality Impact</rdfs:label>
    </owl:Class>
    


    <!-- http://ontologies.ti-semantics.com/score#CVSSv3ConfidentialityRequirement -->

    <owl:Class rdf:about="http://ontologies.ti-semantics.com/score#CVSSv3ConfidentialityRequirement">
        <rdfs:subClassOf rdf:resource="http://ontologies.ti-semantics.com/score#SecurityRequirement"/>
        <cvss_v2_code xml:lang="en">CR</cvss_v2_code>
        <cvss_v3_code xml:lang="en">CR</cvss_v3_code>
        <rdfs:comment xml:lang="en">These metrics enable the analyst to customize the CVSS score depending on the importance of the affected IT asset to a user&apos;s organization, measured in terms of Confidentiality. That is, if an IT asset supports a business function for which Confidentiality is most important, the analyst can assign a greater value to Confidentiality relative to Availability and Integrity. This security requirement has three possible values: Low, Medium, or High.

Note that the Confidentiality Requirement will not affect the Environmental score if the (Modified Base) confidentiality impact is set to None. Also, increasing the Confidentiality Requirement from Medium to High will not change the Environmental score when the (Modified Base) impact metrics are set to High. This is because the modified impact sub score (part of the Modified Base score that calculates impact) is already at a maximum value of 10.</rdfs:comment>
        <rdfs:isDefinedBy rdf:datatype="http://www.w3.org/2001/XMLSchema#anyURI">https://www.first.org/cvss/specification-document#4-1-Security-Requirements-CR-IR-AR</rdfs:isDefinedBy>
        <rdfs:isDefinedBy xml:lang="en">https://www.first.org/cvss/v2/guide#2-3-3-Security-Requirements-CR-IR-AR</rdfs:isDefinedBy>
    </owl:Class>
    


    <!-- http://ontologies.ti-semantics.com/score#CVSSv3ConfirmedReportConfidence -->

    <owl:Class rdf:about="http://ontologies.ti-semantics.com/score#CVSSv3ConfirmedReportConfidence">
        <rdfs:subClassOf rdf:resource="http://ontologies.ti-semantics.com/score#CVSSv3ReportConfidence"/>
    </owl:Class>
    


    <!-- http://ontologies.ti-semantics.com/score#CVSSv3EnvironmentalMetricGroup -->

    <owl:Class rdf:about="http://ontologies.ti-semantics.com/score#CVSSv3EnvironmentalMetricGroup">
        <rdfs:subClassOf rdf:resource="http://ontologies.ti-semantics.com/score#CVSSv3MetricGroup"/>
    </owl:Class>
    


    <!-- http://ontologies.ti-semantics.com/score#CVSSv3ExploitCodeMaturity -->

    <owl:Class rdf:about="http://ontologies.ti-semantics.com/score#CVSSv3ExploitCodeMaturity">
        <rdfs:subClassOf rdf:resource="http://ontologies.ti-semantics.com/score#CVSSv3Metric"/>
        <rdfs:subClassOf rdf:resource="http://ontologies.ti-semantics.com/score#TemporalMetric"/>
        <cvss_v3_code xml:lang="en">E</cvss_v3_code>
        <rdfs:comment xml:lang="en">This metric measures the likelihood of the vulnerability being attacked, and is typically based on the current state of exploit techniques, exploit code availability, or active, &quot;in-the-wild&quot; exploitation. Public availability of easy-to-use exploit code increases the number of potential attackers by including those who are unskilled, thereby increasing the severity of the vulnerability. Initially, real-world exploitation may only be theoretical. Publication of proof-of-concept code, functional exploit code, or sufficient technical details necessary to exploit the vulnerability may follow. Furthermore, the exploit code available may progress from a proof-of-concept demonstration to exploit code that is successful in exploiting the vulnerability consistently. In severe cases, it may be delivered as the payload of a network-based worm or virus or other automated attack tools.</rdfs:comment>
        <rdfs:isDefinedBy rdf:datatype="http://www.w3.org/2001/XMLSchema#anyURI">https://www.first.org/cvss/specification-document#3-1-Exploit-Code-Maturity-E</rdfs:isDefinedBy>
        <rdfs:label xml:lang="en">Exploit Code Maturity</rdfs:label>
    </owl:Class>
    


    <!-- http://ontologies.ti-semantics.com/score#CVSSv3FunctionalExploitCodeMaturity -->

    <owl:Class rdf:about="http://ontologies.ti-semantics.com/score#CVSSv3FunctionalExploitCodeMaturity">
        <rdfs:subClassOf rdf:resource="http://ontologies.ti-semantics.com/score#CVSSv3ExploitCodeMaturity"/>
    </owl:Class>
    


    <!-- http://ontologies.ti-semantics.com/score#CVSSv3HighAttackComplexity -->

    <owl:Class rdf:about="http://ontologies.ti-semantics.com/score#CVSSv3HighAttackComplexity">
        <rdfs:subClassOf rdf:resource="http://ontologies.ti-semantics.com/score#CVSSv3AttackComplexity"/>
    </owl:Class>
    


    <!-- http://ontologies.ti-semantics.com/score#CVSSv3HighAvailabilityImpact -->

    <owl:Class rdf:about="http://ontologies.ti-semantics.com/score#CVSSv3HighAvailabilityImpact">
        <rdfs:subClassOf rdf:resource="http://ontologies.ti-semantics.com/score#CVSSv3AvailabilityImpact"/>
    </owl:Class>
    


    <!-- http://ontologies.ti-semantics.com/score#CVSSv3HighAvailabilityRequirement -->

    <owl:Class rdf:about="http://ontologies.ti-semantics.com/score#CVSSv3HighAvailabilityRequirement">
        <rdfs:subClassOf rdf:resource="http://ontologies.ti-semantics.com/score#CVSSv3AvailabilityRequirement"/>
    </owl:Class>
    


    <!-- http://ontologies.ti-semantics.com/score#CVSSv3HighConfidentialityImpact -->

    <owl:Class rdf:about="http://ontologies.ti-semantics.com/score#CVSSv3HighConfidentialityImpact">
        <rdfs:subClassOf rdf:resource="http://ontologies.ti-semantics.com/score#CVSSv3ConfidentialityImpact"/>
    </owl:Class>
    


    <!-- http://ontologies.ti-semantics.com/score#CVSSv3HighConfidentialityRequirement -->

    <owl:Class rdf:about="http://ontologies.ti-semantics.com/score#CVSSv3HighConfidentialityRequirement">
        <rdfs:subClassOf rdf:resource="http://ontologies.ti-semantics.com/score#CVSSv3ConfidentialityRequirement"/>
        <cvss_v3_code xml:lang="en">H</cvss_v3_code>
        <rdfs:comment xml:lang="en">Loss of Confidentiality is likely to have a catastrophic adverse effect on the organization or individuals associated with the organization (e.g., employees, customers).</rdfs:comment>
        <rdfs:isDefinedBy rdf:datatype="http://www.w3.org/2001/XMLSchema#anyURI">https://www.first.org/cvss/specification-document#4-1-Security-Requirements-CR-IR-AR</rdfs:isDefinedBy>
    </owl:Class>
    


    <!-- http://ontologies.ti-semantics.com/score#CVSSv3HighExploitCodeMaturity -->

    <owl:Class rdf:about="http://ontologies.ti-semantics.com/score#CVSSv3HighExploitCodeMaturity">
        <rdfs:subClassOf rdf:resource="http://ontologies.ti-semantics.com/score#CVSSv3ExploitCodeMaturity"/>
    </owl:Class>
    


    <!-- http://ontologies.ti-semantics.com/score#CVSSv3HighIntegrityImpact -->

    <owl:Class rdf:about="http://ontologies.ti-semantics.com/score#CVSSv3HighIntegrityImpact">
        <rdfs:subClassOf rdf:resource="http://ontologies.ti-semantics.com/score#CVSSv3IntegrityImpact"/>
    </owl:Class>
    


    <!-- http://ontologies.ti-semantics.com/score#CVSSv3HighIntegrityRequirement -->

    <owl:Class rdf:about="http://ontologies.ti-semantics.com/score#CVSSv3HighIntegrityRequirement">
        <rdfs:subClassOf rdf:resource="http://ontologies.ti-semantics.com/score#CVSSv3IntegrityRequirement"/>
        <cvss_v3_code xml:lang="en">H</cvss_v3_code>
        <rdfs:comment xml:lang="en">Loss of Integrity is likely to have a catastrophic adverse effect on the organization or individuals associated with the organization (e.g., employees, customers).</rdfs:comment>
        <rdfs:isDefinedBy rdf:datatype="http://www.w3.org/2001/XMLSchema#anyURI">https://www.first.org/cvss/specification-document#4-1-Security-Requirements-CR-IR-AR</rdfs:isDefinedBy>
    </owl:Class>
    


    <!-- http://ontologies.ti-semantics.com/score#CVSSv3HighPrivilegesRequired -->

    <owl:Class rdf:about="http://ontologies.ti-semantics.com/score#CVSSv3HighPrivilegesRequired">
        <rdfs:subClassOf rdf:resource="http://ontologies.ti-semantics.com/score#CVSSv3PrivilegesRequired"/>
    </owl:Class>
    


    <!-- http://ontologies.ti-semantics.com/score#CVSSv3IntegrityImpact -->

    <owl:Class rdf:about="http://ontologies.ti-semantics.com/score#CVSSv3IntegrityImpact">
        <rdfs:subClassOf rdf:resource="http://ontologies.ti-semantics.com/score#CVSSv3Metric"/>
        <rdfs:subClassOf rdf:resource="http://ontologies.ti-semantics.com/score#ImpactMetric"/>
        <cvss_v3_code>I</cvss_v3_code>
        <rdfs:comment xml:lang="en">This metric measures the impact to integrity of a successfully exploited vulnerability. Integrity refers to the trustworthiness and veracity of information. This metric value increases with the consequence to the impacted component.</rdfs:comment>
        <rdfs:isDefinedBy rdf:datatype="http://www.w3.org/2001/XMLSchema#anyURI">https://www.first.org/cvss/specification-document#2-3-2-Integrity-Impact-I</rdfs:isDefinedBy>
        <rdfs:label xml:lang="en">Integrity Impact</rdfs:label>
    </owl:Class>
    


    <!-- http://ontologies.ti-semantics.com/score#CVSSv3IntegrityRequirement -->

    <owl:Class rdf:about="http://ontologies.ti-semantics.com/score#CVSSv3IntegrityRequirement">
        <rdfs:subClassOf rdf:resource="http://ontologies.ti-semantics.com/score#SecurityRequirement"/>
        <cvss_v2_code xml:lang="en">CR</cvss_v2_code>
        <rdfs:comment xml:lang="en">This metric enables the analyst to customize the CVSS score depending on the importance of the affected IT asset to a user&apos;s organization, measured in terms of Integrity. That is, if an IT asset supports a business function for which Integrityis most important, the analyst can assign a greater value to Integrity relative to Confidentiality and Availability. Each security requirement has three possible values: Low, Medium, or High.</rdfs:comment>
        <rdfs:isDefinedBy xml:lang="en">https://www.first.org/cvss/specification-document#4-1-Security-Requirements-CR-IR-AR</rdfs:isDefinedBy>
        <rdfs:isDefinedBy xml:lang="en">https://www.first.org/cvss/v2/guide#2-3-3-Security-Requirements-CR-IR-AR</rdfs:isDefinedBy>
    </owl:Class>
    


    <!-- http://ontologies.ti-semantics.com/score#CVSSv3LocalAttackVector -->

    <owl:Class rdf:about="http://ontologies.ti-semantics.com/score#CVSSv3LocalAttackVector">
        <rdfs:subClassOf rdf:resource="http://ontologies.ti-semantics.com/score#CVSSv3AttackVector"/>
    </owl:Class>
    


    <!-- http://ontologies.ti-semantics.com/score#CVSSv3LowAttackComplexity -->

    <owl:Class rdf:about="http://ontologies.ti-semantics.com/score#CVSSv3LowAttackComplexity">
        <rdfs:subClassOf rdf:resource="http://ontologies.ti-semantics.com/score#CVSSv3AttackComplexity"/>
    </owl:Class>
    


    <!-- http://ontologies.ti-semantics.com/score#CVSSv3LowAvailabilityImpact -->

    <owl:Class rdf:about="http://ontologies.ti-semantics.com/score#CVSSv3LowAvailabilityImpact">
        <rdfs:subClassOf rdf:resource="http://ontologies.ti-semantics.com/score#CVSSv3AvailabilityImpact"/>
    </owl:Class>
    


    <!-- http://ontologies.ti-semantics.com/score#CVSSv3LowAvailabilityRequirement -->

    <owl:Class rdf:about="http://ontologies.ti-semantics.com/score#CVSSv3LowAvailabilityRequirement">
        <rdfs:subClassOf rdf:resource="http://ontologies.ti-semantics.com/score#CVSSv3AvailabilityRequirement"/>
    </owl:Class>
    


    <!-- http://ontologies.ti-semantics.com/score#CVSSv3LowConfidentialityImpact -->

    <owl:Class rdf:about="http://ontologies.ti-semantics.com/score#CVSSv3LowConfidentialityImpact">
        <rdfs:subClassOf rdf:resource="http://ontologies.ti-semantics.com/score#CVSSv3ConfidentialityImpact"/>
    </owl:Class>
    


    <!-- http://ontologies.ti-semantics.com/score#CVSSv3LowConfidentialityRequirement -->

    <owl:Class rdf:about="http://ontologies.ti-semantics.com/score#CVSSv3LowConfidentialityRequirement">
        <rdfs:subClassOf rdf:resource="http://ontologies.ti-semantics.com/score#CVSSv3ConfidentialityRequirement"/>
        <cvss_v3_code xml:lang="en">L</cvss_v3_code>
        <rdfs:comment xml:lang="en">Loss of Confidentiality is likely to have only a limited adverse effect on the organization or individuals associated with the organization (e.g., employees, customers).</rdfs:comment>
        <rdfs:isDefinedBy rdf:datatype="http://www.w3.org/2001/XMLSchema#anyURI">https://www.first.org/cvss/specification-document#4-1-Security-Requirements-CR-IR-AR</rdfs:isDefinedBy>
    </owl:Class>
    


    <!-- http://ontologies.ti-semantics.com/score#CVSSv3LowIntegrityImpact -->

    <owl:Class rdf:about="http://ontologies.ti-semantics.com/score#CVSSv3LowIntegrityImpact">
        <rdfs:subClassOf rdf:resource="http://ontologies.ti-semantics.com/score#CVSSv3IntegrityImpact"/>
    </owl:Class>
    


    <!-- http://ontologies.ti-semantics.com/score#CVSSv3LowIntegrityRequirement -->

    <owl:Class rdf:about="http://ontologies.ti-semantics.com/score#CVSSv3LowIntegrityRequirement">
        <rdfs:subClassOf rdf:resource="http://ontologies.ti-semantics.com/score#CVSSv3IntegrityRequirement"/>
        <cvss_v3_code xml:lang="en">L</cvss_v3_code>
        <rdfs:comment xml:lang="en">Loss of Integrity is likely to have only a limited adverse effect on the organization or individuals associated with the organization (e.g., employees, customers).</rdfs:comment>
        <rdfs:isDefinedBy rdf:datatype="http://www.w3.org/2001/XMLSchema#anyURI">https://www.first.org/cvss/specification-document#4-1-Security-Requirements-CR-IR-AR</rdfs:isDefinedBy>
    </owl:Class>
    


    <!-- http://ontologies.ti-semantics.com/score#CVSSv3LowPrivilegesRequired -->

    <owl:Class rdf:about="http://ontologies.ti-semantics.com/score#CVSSv3LowPrivilegesRequired">
        <rdfs:subClassOf rdf:resource="http://ontologies.ti-semantics.com/score#CVSSv3PrivilegesRequired"/>
    </owl:Class>
    


    <!-- http://ontologies.ti-semantics.com/score#CVSSv3MediumAvailabilityRequirement -->

    <owl:Class rdf:about="http://ontologies.ti-semantics.com/score#CVSSv3MediumAvailabilityRequirement">
        <rdfs:subClassOf rdf:resource="http://ontologies.ti-semantics.com/score#CVSSv3AvailabilityRequirement"/>
    </owl:Class>
    


    <!-- http://ontologies.ti-semantics.com/score#CVSSv3MediumConfidentialityRequirement -->

    <owl:Class rdf:about="http://ontologies.ti-semantics.com/score#CVSSv3MediumConfidentialityRequirement">
        <rdfs:subClassOf rdf:resource="http://ontologies.ti-semantics.com/score#CVSSv3ConfidentialityRequirement"/>
        <cvss_v3_code xml:lang="en">M</cvss_v3_code>
        <rdfs:comment xml:lang="en">Loss of Confidentiality is likely to have a serious adverse effect on the organization or individuals associated with the organization (e.g., employees, customers).</rdfs:comment>
        <rdfs:isDefinedBy rdf:datatype="http://www.w3.org/2001/XMLSchema#anyURI">https://www.first.org/cvss/specification-document#4-1-Security-Requirements-CR-IR-AR</rdfs:isDefinedBy>
    </owl:Class>
    


    <!-- http://ontologies.ti-semantics.com/score#CVSSv3MediumIntegrityRequirement -->

    <owl:Class rdf:about="http://ontologies.ti-semantics.com/score#CVSSv3MediumIntegrityRequirement">
        <rdfs:subClassOf rdf:resource="http://ontologies.ti-semantics.com/score#CVSSv3IntegrityRequirement"/>
        <cvss_v3_code xml:lang="en">M</cvss_v3_code>
        <rdfs:comment xml:lang="en">Loss of Integrity is likely to have a serious adverse effect on the organization or individuals associated with the organization (e.g., employees, customers).</rdfs:comment>
        <rdfs:isDefinedBy rdf:datatype="http://www.w3.org/2001/XMLSchema#anyURI">https://www.first.org/cvss/specification-document#4-1-Security-Requirements-CR-IR-AR</rdfs:isDefinedBy>
    </owl:Class>
    


    <!-- http://ontologies.ti-semantics.com/score#CVSSv3Metric -->

    <owl:Class rdf:about="http://ontologies.ti-semantics.com/score#CVSSv3Metric">
        <rdfs:subClassOf rdf:resource="http://ontologies.ti-semantics.com/score#CVSSMetric"/>
        <rdfs:subClassOf rdf:resource="http://ontologies.ti-semantics.com/score#CVSSv2Metric"/>
    </owl:Class>
    


    <!-- http://ontologies.ti-semantics.com/score#CVSSv3MetricGroup -->

    <owl:Class rdf:about="http://ontologies.ti-semantics.com/score#CVSSv3MetricGroup">
        <rdfs:subClassOf rdf:resource="http://ontologies.ti-semantics.com/score#CVSSMetricGroup"/>
    </owl:Class>
    


    <!-- http://ontologies.ti-semantics.com/score#CVSSv3ModifiedBaseMetric -->

    <owl:Class rdf:about="http://ontologies.ti-semantics.com/score#CVSSv3ModifiedBaseMetric">
        <rdfs:subClassOf rdf:resource="http://ontologies.ti-semantics.com/score#EnvironmentalMetric"/>
        <rdfs:comment xml:lang="en">These metrics enable the analyst to adjust the Base metrics according to modifications that exist within the analyst’s environment. That is, if an environment has made general changes for the affected software that differs in a way which would affect its Exploitability, Scope, or Impact, then the environment can reflect this via an appropriately-modified, Environmental score.

The full effect on the Environmental score is determined by the corresponding Base metrics. That is, these metrics modify the Environmental score by reassigning the (Base) metrics values, prior to applying the (Environmental) Security Requirements. For example, the default configuration for a vulnerable component may be to run a listening service with administrator privileges, for which a compromise might grant an attacker Confidentiality, Integrity, and Availability impacts that are all High. Yet, in the analyst’s environment, that same Internet service might be running with reduced privileges; in that case, the Modified Confidentiality, Modified Integrity, and Modified Availability might each be set to Low.

For brevity, only the names of the Modified Base metrics are mentioned. Each Modified Environmental metric has the same values as its corresponding Base metric, plus a value of Not Defined.

The intent of this metric is to define the mitigations in place for a given environment. It is acceptable to use the Modified metrics to describe situations that increase the Base score. For example, the default configuration of a component may be to require high privileges (PR: High) in order to access a particular function, but in the analyst’s environment, there may be no privileges required (PR: None). The analyst can set MPR: None to reflect this more serious condition for their environment.</rdfs:comment>
        <rdfs:isDefinedBy rdf:datatype="http://www.w3.org/2001/XMLSchema#anyURI">https://www.first.org/cvss/specification-document#4-2-Modified-Base-Metrics</rdfs:isDefinedBy>
    </owl:Class>
    


    <!-- http://ontologies.ti-semantics.com/score#CVSSv3NetworkAttackVector -->

    <owl:Class rdf:about="http://ontologies.ti-semantics.com/score#CVSSv3NetworkAttackVector">
        <rdfs:subClassOf rdf:resource="http://ontologies.ti-semantics.com/score#CVSSv3AttackVector"/>
    </owl:Class>
    


    <!-- http://ontologies.ti-semantics.com/score#CVSSv3NoAvailabilityImpact -->

    <owl:Class rdf:about="http://ontologies.ti-semantics.com/score#CVSSv3NoAvailabilityImpact">
        <rdfs:subClassOf rdf:resource="http://ontologies.ti-semantics.com/score#CVSSv3AvailabilityImpact"/>
    </owl:Class>
    


    <!-- http://ontologies.ti-semantics.com/score#CVSSv3NoConfidentialityImpact -->

    <owl:Class rdf:about="http://ontologies.ti-semantics.com/score#CVSSv3NoConfidentialityImpact">
        <rdfs:subClassOf rdf:resource="http://ontologies.ti-semantics.com/score#CVSSv3ConfidentialityImpact"/>
    </owl:Class>
    


    <!-- http://ontologies.ti-semantics.com/score#CVSSv3NoIntegrityImpact -->

    <owl:Class rdf:about="http://ontologies.ti-semantics.com/score#CVSSv3NoIntegrityImpact">
        <rdfs:subClassOf rdf:resource="http://ontologies.ti-semantics.com/score#CVSSv3IntegrityImpact"/>
    </owl:Class>
    


    <!-- http://ontologies.ti-semantics.com/score#CVSSv3NoPrivilegesRequired -->

    <owl:Class rdf:about="http://ontologies.ti-semantics.com/score#CVSSv3NoPrivilegesRequired">
        <rdfs:subClassOf rdf:resource="http://ontologies.ti-semantics.com/score#CVSSv3PrivilegesRequired"/>
    </owl:Class>
    


    <!-- http://ontologies.ti-semantics.com/score#CVSSv3NoUserInteraction -->

    <owl:Class rdf:about="http://ontologies.ti-semantics.com/score#CVSSv3NoUserInteraction">
        <rdfs:subClassOf rdf:resource="http://ontologies.ti-semantics.com/score#CVSSv3UserInteraction"/>
    </owl:Class>
    


    <!-- http://ontologies.ti-semantics.com/score#CVSSv3NotDefinedAvailabilityRequirement -->

    <owl:Class rdf:about="http://ontologies.ti-semantics.com/score#CVSSv3NotDefinedAvailabilityRequirement">
        <rdfs:subClassOf rdf:resource="http://ontologies.ti-semantics.com/score#CVSSv3AvailabilityRequirement"/>
    </owl:Class>
    


    <!-- http://ontologies.ti-semantics.com/score#CVSSv3NotDefinedConfidentialityRequirement -->

    <owl:Class rdf:about="http://ontologies.ti-semantics.com/score#CVSSv3NotDefinedConfidentialityRequirement">
        <rdfs:subClassOf rdf:resource="http://ontologies.ti-semantics.com/score#CVSSv3ConfidentialityRequirement"/>
        <cvss_v3_code xml:lang="en">X</cvss_v3_code>
        <rdfs:comment xml:lang="en">Assigning this value to the metric will not influence the score. It is a signal to the equation to skip this metric.</rdfs:comment>
        <rdfs:isDefinedBy rdf:datatype="http://www.w3.org/2001/XMLSchema#anyURI">https://www.first.org/cvss/specification-document#4-1-Security-Requirements-CR-IR-AR</rdfs:isDefinedBy>
    </owl:Class>
    


    <!-- http://ontologies.ti-semantics.com/score#CVSSv3NotDefinedExploitCodeMaturity -->

    <owl:Class rdf:about="http://ontologies.ti-semantics.com/score#CVSSv3NotDefinedExploitCodeMaturity">
        <rdfs:subClassOf rdf:resource="http://ontologies.ti-semantics.com/score#CVSSv3ExploitCodeMaturity"/>
    </owl:Class>
    


    <!-- http://ontologies.ti-semantics.com/score#CVSSv3NotDefinedIntegrityRequirement -->

    <owl:Class rdf:about="http://ontologies.ti-semantics.com/score#CVSSv3NotDefinedIntegrityRequirement">
        <rdfs:subClassOf rdf:resource="http://ontologies.ti-semantics.com/score#CVSSv3IntegrityRequirement"/>
        <cvss_v3_code xml:lang="en">X</cvss_v3_code>
        <rdfs:comment xml:lang="en">Assigning this value to the metric will not influence the score. It is a signal to the equation to skip this metric.</rdfs:comment>
        <rdfs:isDefinedBy rdf:datatype="http://www.w3.org/2001/XMLSchema#anyURI">https://www.first.org/cvss/specification-document#4-1-Security-Requirements-CR-IR-AR</rdfs:isDefinedBy>
    </owl:Class>
    


    <!-- http://ontologies.ti-semantics.com/score#CVSSv3NotDefinedRemediation -->

    <owl:Class rdf:about="http://ontologies.ti-semantics.com/score#CVSSv3NotDefinedRemediation">
        <rdfs:subClassOf rdf:resource="http://ontologies.ti-semantics.com/score#CVSSv3RemediationLevel"/>
    </owl:Class>
    


    <!-- http://ontologies.ti-semantics.com/score#CVSSv3NotDefinedReportConfidence -->

    <owl:Class rdf:about="http://ontologies.ti-semantics.com/score#CVSSv3NotDefinedReportConfidence">
        <rdfs:subClassOf rdf:resource="http://ontologies.ti-semantics.com/score#CVSSv3ReportConfidence"/>
    </owl:Class>
    


    <!-- http://ontologies.ti-semantics.com/score#CVSSv3OfficialFixRemediation -->

    <owl:Class rdf:about="http://ontologies.ti-semantics.com/score#CVSSv3OfficialFixRemediation">
        <rdfs:subClassOf rdf:resource="http://ontologies.ti-semantics.com/score#CVSSv3RemediationLevel"/>
    </owl:Class>
    


    <!-- http://ontologies.ti-semantics.com/score#CVSSv3PhysicalAttackVector -->

    <owl:Class rdf:about="http://ontologies.ti-semantics.com/score#CVSSv3PhysicalAttackVector">
        <rdfs:subClassOf rdf:resource="http://ontologies.ti-semantics.com/score#CVSSv3AttackVector"/>
    </owl:Class>
    


    <!-- http://ontologies.ti-semantics.com/score#CVSSv3PrivilegesRequired -->

    <owl:Class rdf:about="http://ontologies.ti-semantics.com/score#CVSSv3PrivilegesRequired">
        <rdfs:subClassOf rdf:resource="http://ontologies.ti-semantics.com/score#CVSSv3Metric"/>
        <rdfs:subClassOf rdf:resource="http://ontologies.ti-semantics.com/score#ExploitabilityMetric"/>
        <cvss_v3_code>PR</cvss_v3_code>
        <rdfs:comment xml:lang="en">This metric describes the level of privileges an attacker must possess before successfully exploiting the vulnerability. This metric if greatest if no privileges are required.</rdfs:comment>
        <rdfs:isDefinedBy rdf:datatype="http://www.w3.org/2001/XMLSchema#anyURI">https://www.first.org/cvss/specification-document#2-1-3-Privileges-Required-PR</rdfs:isDefinedBy>
    </owl:Class>
    


    <!-- http://ontologies.ti-semantics.com/score#CVSSv3ProofOfConceptExploitCodeMaturity -->

    <owl:Class rdf:about="http://ontologies.ti-semantics.com/score#CVSSv3ProofOfConceptExploitCodeMaturity">
        <rdfs:subClassOf rdf:resource="http://ontologies.ti-semantics.com/score#CVSSv3ExploitCodeMaturity"/>
    </owl:Class>
    


    <!-- http://ontologies.ti-semantics.com/score#CVSSv3ReasonableReportConfidence -->

    <owl:Class rdf:about="http://ontologies.ti-semantics.com/score#CVSSv3ReasonableReportConfidence">
        <rdfs:subClassOf rdf:resource="http://ontologies.ti-semantics.com/score#CVSSv3ReportConfidence"/>
    </owl:Class>
    


    <!-- http://ontologies.ti-semantics.com/score#CVSSv3RemediationLevel -->

    <owl:Class rdf:about="http://ontologies.ti-semantics.com/score#CVSSv3RemediationLevel">
        <rdfs:subClassOf rdf:resource="http://ontologies.ti-semantics.com/score#CVSSv3Metric"/>
        <rdfs:subClassOf rdf:resource="http://ontologies.ti-semantics.com/score#TemporalMetric"/>
        <cvss_v2_code xml:lang="en">RL</cvss_v2_code>
        <cvss_v3_code xml:lang="en">RL</cvss_v3_code>
        <rdfs:comment xml:lang="en">The Remediation Level of a vulnerability is an important factor for prioritization. The typical vulnerability is unpatched when initially published. Workarounds or hotfixes may offer interim remediation until an official patch or upgrade is issued. Each of these respective stages adjusts the temporal score downwards, reflecting the decreasing urgency as remediation becomes final. The less official and permanent a fix, the higher the vulnerability score.</rdfs:comment>
        <rdfs:isDefinedBy rdf:datatype="http://www.w3.org/2001/XMLSchema#anyURI">https://www.first.org/cvss/specification-document#3-2-Remediation-Level-RL</rdfs:isDefinedBy>
        <rdfs:isDefinedBy xml:lang="en">https://www.first.org/cvss/v2/guide#2-2-2-Remediation-Level-RL</rdfs:isDefinedBy>
        <rdfs:label xml:lang="en">Remediation Level</rdfs:label>
    </owl:Class>
    


    <!-- http://ontologies.ti-semantics.com/score#CVSSv3ReportConfidence -->

    <owl:Class rdf:about="http://ontologies.ti-semantics.com/score#CVSSv3ReportConfidence">
        <rdfs:subClassOf rdf:resource="http://ontologies.ti-semantics.com/score#CVSSv3Metric"/>
        <rdfs:subClassOf rdf:resource="http://ontologies.ti-semantics.com/score#TemporalMetric"/>
        <cvss_v3_code xml:lang="en">RC</cvss_v3_code>
        <rdfs:comment xml:lang="en">This metric measures the degree of confidence in the existence of the vulnerability and the credibility of the known technical details. Sometimes only the existence of vulnerabilities are publicized, but without specific details. For example, an impact may be recognized as undesirable, but the root cause may not be known. The vulnerability may later be corroborated by research which suggests where the vulnerability may lie, though the research may not be certain. Finally, a vulnerability may be confirmed through acknowledgement by the author or vendor of the affected technology. The urgency of a vulnerability is higher when a vulnerability is known to exist with certainty. This metric also suggests the level of technical knowledge available to would-be attackers. The more a vulnerability is validated by the vendor or other reputable sources, the higher the score.</rdfs:comment>
        <rdfs:isDefinedBy rdf:datatype="http://www.w3.org/2001/XMLSchema#anyURI">https://www.first.org/cvss/specification-document#3-3-Report-Confidence-RC</rdfs:isDefinedBy>
        <rdfs:label xml:lang="en">Report Confidence</rdfs:label>
    </owl:Class>
    


    <!-- http://ontologies.ti-semantics.com/score#CVSSv3RequiredUserInteraction -->

    <owl:Class rdf:about="http://ontologies.ti-semantics.com/score#CVSSv3RequiredUserInteraction">
        <rdfs:subClassOf rdf:resource="http://ontologies.ti-semantics.com/score#CVSSv3UserInteraction"/>
    </owl:Class>
    


    <!-- http://ontologies.ti-semantics.com/score#CVSSv3Scope -->

    <owl:Class rdf:about="http://ontologies.ti-semantics.com/score#CVSSv3Scope">
        <rdfs:subClassOf rdf:resource="http://ontologies.ti-semantics.com/score#CVSSv3Metric"/>
        <cvss_v3_code>S</cvss_v3_code>
        <rdfs:comment xml:lang="en">An important property captured by CVSS v3.0 is the ability for a vulnerability in one software component to impact resources beyond its means, or privileges. This consequence is represented by the metric Authorization Scope, or simply Scope.

Formally, Scope refers to the collection of privileges defined by a computing authority (e.g. an application, an operating system, or a sandbox environment) when granting access to computing resources (e.g. files, CPU, memory, etc). These privileges are assigned based on some method of identification and authorization. In some cases, the authorization may be simple or loosely controlled based upon predefined rules or standards. For example, in the case of Ethernet traffic sent to a network switch, the switch accepts traffic that arrives on its ports and is an authority that controls the traffic flow to other switch ports.

When the vulnerability of a software component governed by one authorization scope is able to affect resources governed by another authorization scope, a Scope change has occurred.
Intuitively, one may think of a scope change as breaking out of a sandbox, and an example would be a vulnerability in a virtual machine that enables an attacker to delete files on the host OS (perhaps even its own VM). In this example, there are two separate authorization authorities: one that defines and enforces privileges for the virtual machine and its users, and one that defines and enforces privileges for the host system within which the virtual machine runs.

A scope change would not occur, for example, with a vulnerability in Microsoft Word that allows an attacker to compromise all system files of the host OS, because the same authority enforces privileges of the user’s instance of Word, and the host’s system files.</rdfs:comment>
        <rdfs:isDefinedBy rdf:datatype="http://www.w3.org/2001/XMLSchema#anyURI">https://www.first.org/cvss/specification-document#2-2-Scope-S</rdfs:isDefinedBy>
        <rdfs:label xml:lang="en">Scope</rdfs:label>
    </owl:Class>
    


    <!-- http://ontologies.ti-semantics.com/score#CVSSv3TemporalMetricGroup -->

    <owl:Class rdf:about="http://ontologies.ti-semantics.com/score#CVSSv3TemporalMetricGroup">
        <rdfs:subClassOf rdf:resource="http://ontologies.ti-semantics.com/score#CVSSv3MetricGroup"/>
    </owl:Class>
    


    <!-- http://ontologies.ti-semantics.com/score#CVSSv3TemporaryFixRemediation -->

    <owl:Class rdf:about="http://ontologies.ti-semantics.com/score#CVSSv3TemporaryFixRemediation">
        <rdfs:subClassOf rdf:resource="http://ontologies.ti-semantics.com/score#CVSSv3RemediationLevel"/>
    </owl:Class>
    


    <!-- http://ontologies.ti-semantics.com/score#CVSSv3UnavailableRemediation -->

    <owl:Class rdf:about="http://ontologies.ti-semantics.com/score#CVSSv3UnavailableRemediation">
        <rdfs:subClassOf rdf:resource="http://ontologies.ti-semantics.com/score#CVSSv3RemediationLevel"/>
    </owl:Class>
    


    <!-- http://ontologies.ti-semantics.com/score#CVSSv3UnchangedScope -->

    <owl:Class rdf:about="http://ontologies.ti-semantics.com/score#CVSSv3UnchangedScope">
        <rdfs:subClassOf rdf:resource="http://ontologies.ti-semantics.com/score#CVSSv3Scope"/>
    </owl:Class>
    


    <!-- http://ontologies.ti-semantics.com/score#CVSSv3UnknownReportConfidence -->

    <owl:Class rdf:about="http://ontologies.ti-semantics.com/score#CVSSv3UnknownReportConfidence">
        <rdfs:subClassOf rdf:resource="http://ontologies.ti-semantics.com/score#CVSSv3ReportConfidence"/>
    </owl:Class>
    


    <!-- http://ontologies.ti-semantics.com/score#CVSSv3UnprovenExploitCodeMaturity -->

    <owl:Class rdf:about="http://ontologies.ti-semantics.com/score#CVSSv3UnprovenExploitCodeMaturity">
        <rdfs:subClassOf rdf:resource="http://ontologies.ti-semantics.com/score#CVSSv3ExploitCodeMaturity"/>
    </owl:Class>
    


    <!-- http://ontologies.ti-semantics.com/score#CVSSv3UserInteraction -->

    <owl:Class rdf:about="http://ontologies.ti-semantics.com/score#CVSSv3UserInteraction">
        <rdfs:subClassOf rdf:resource="http://ontologies.ti-semantics.com/score#CVSSv3Metric"/>
        <rdfs:subClassOf rdf:resource="http://ontologies.ti-semantics.com/score#ExploitabilityMetric"/>
        <cvss_v3_code>UI</cvss_v3_code>
        <rdfs:comment xml:lang="en">This metric captures the requirement for a user, other than the attacker, to participate in the successful compromise of the vulnerable component. This metric determines whether the vulnerability can be exploited solely at the will of the attacker, or whether a separate user (or user-initiated process) must participate in some manner. This metric value is greatest when no user interaction is required.</rdfs:comment>
        <rdfs:isDefinedBy rdf:datatype="http://www.w3.org/2001/XMLSchema#anyURI">https://www.first.org/cvss/specification-document#2-1-4-User-Interaction-UI</rdfs:isDefinedBy>
        <rdfs:label xml:lang="en">User Interaction</rdfs:label>
    </owl:Class>
    


    <!-- http://ontologies.ti-semantics.com/score#CVSSv3WorkaroundRemediation -->

    <owl:Class rdf:about="http://ontologies.ti-semantics.com/score#CVSSv3WorkaroundRemediation">
        <rdfs:subClassOf rdf:resource="http://ontologies.ti-semantics.com/score#CVSSv3RemediationLevel"/>
    </owl:Class>
    


    <!-- http://ontologies.ti-semantics.com/score#EnvironmentalMetric -->

    <owl:Class rdf:about="http://ontologies.ti-semantics.com/score#EnvironmentalMetric">
        <rdfs:subClassOf rdf:resource="http://ontologies.ti-semantics.com/score#Metric"/>
        <rdfs:comment rdf:datatype="http://www.w3.org/2001/XMLSchema#string">Defines the characteristics of a vulnerability that are relevant and unique to a particular user&apos;s environment.</rdfs:comment>
        <rdfs:comment xml:lang="en">These metrics enable the analyst to customize the CVSS score depending on the importance of the affected IT asset to a user’s organization, measured in terms of complementary/alternative security controls in place, Confidentiality, Integrity, and Availability. The metrics are the modified equivalent of base metrics and are assigned metrics value based on the component placement in organization infrastructure.</rdfs:comment>
        <rdfs:isDefinedBy rdf:datatype="http://www.w3.org/2001/XMLSchema#anyURI">https://www.first.org/cvss/cvss-v30-specification-v1.7.pdf</rdfs:isDefinedBy>
        <rdfs:label>CVSS Environmental Metrics</rdfs:label>
    </owl:Class>
    <owl:Axiom>
        <owl:annotatedSource rdf:resource="http://ontologies.ti-semantics.com/score#EnvironmentalMetric"/>
        <owl:annotatedProperty rdf:resource="http://www.w3.org/2000/01/rdf-schema#comment"/>
        <owl:annotatedTarget rdf:datatype="http://www.w3.org/2001/XMLSchema#string">Defines the characteristics of a vulnerability that are relevant and unique to a particular user&apos;s environment.</owl:annotatedTarget>
        <rdfs:comment>Previous text</rdfs:comment>
    </owl:Axiom>
    


    <!-- http://ontologies.ti-semantics.com/score#ExploitabilityMetric -->

    <owl:Class rdf:about="http://ontologies.ti-semantics.com/score#ExploitabilityMetric">
        <rdfs:subClassOf rdf:resource="http://ontologies.ti-semantics.com/score#Metric"/>
        <rdfs:isDefinedBy rdf:datatype="http://www.w3.org/2001/XMLSchema#anyURI">https://www.first.org/cvss/cvss-v30-specification-v1.7.pdf</rdfs:isDefinedBy>
    </owl:Class>
    


    <!-- http://ontologies.ti-semantics.com/score#ImpactMetric -->

    <owl:Class rdf:about="http://ontologies.ti-semantics.com/score#ImpactMetric">
        <rdfs:subClassOf rdf:resource="http://ontologies.ti-semantics.com/score#Metric"/>
        <rdfs:comment xml:lang="en">The Impact metrics refer to the properties of the impacted component. Whether a successfully exploited vulnerability affects one or more components, the impact metrics are scored according to the component that suffers the worst outcome that is most directly and predictably associated with a successful attack. That is, analysts should constrain impacts to a reasonable, final outcome which they are confident an attacker is able to achieve.

If a scope change has not occurred, the Impact metrics should reflect the confidentiality, integrity, and availability (CIA) impact to the vulnerable component. However, if a scope change has occurred, then the Impact metrics should reflect the CIA impact to either the vulnerable component, or the impacted component, whichever suffers the most severe outcome.</rdfs:comment>
        <rdfs:isDefinedBy rdf:datatype="http://www.w3.org/2001/XMLSchema#anyURI">https://www.first.org/cvss/cvss-v30-specification-v1.7.pdf</rdfs:isDefinedBy>
    </owl:Class>
    


    <!-- http://ontologies.ti-semantics.com/score#Metric -->

    <owl:Class rdf:about="http://ontologies.ti-semantics.com/score#Metric">
        <rdfs:comment xml:lang="en">A standard of measure of a degree to which a software system or process possesses some property.</rdfs:comment>
        <rdfs:seeAlso rdf:datatype="http://www.w3.org/2001/XMLSchema#anyURI">https://www.wikidata.org/wiki/Special:EntityData/Q657339</rdfs:seeAlso>
    </owl:Class>
    


    <!-- http://ontologies.ti-semantics.com/score#MetricGroup -->

    <owl:Class rdf:about="http://ontologies.ti-semantics.com/score#MetricGroup"/>
    


    <!-- http://ontologies.ti-semantics.com/score#SecurityRequirement -->

    <owl:Class rdf:about="http://ontologies.ti-semantics.com/score#SecurityRequirement">
        <rdfs:subClassOf rdf:resource="http://ontologies.ti-semantics.com/score#CVSSv2Metric"/>
        <rdfs:subClassOf rdf:resource="http://ontologies.ti-semantics.com/score#CVSSv3Metric"/>
        <rdfs:subClassOf rdf:resource="http://ontologies.ti-semantics.com/score#EnvironmentalMetric"/>
        <rdfs:comment xml:lang="en">These metrics enable the analyst to customize the CVSS score depending on the importance of the affected IT asset to a user’s organization, measured in terms of Confidentiality, Integrity, and Availability. That is, if an IT asset supports a business function for which Availability is most important, the analyst can assign a greater value to Availability relative to Confidentiality and Integrity. Each security requirement has three possible values: Low, Medium, or High.
The full effect on the environmental score is determined by the corresponding Modified Base Impact metrics. That is, these metrics modify the environmental score by reweighting the Modified Confidentiality, Integrity, and Availability impact metrics. For example, the Modified
Confidentiality impact (MC) metric has increased weight if the Confidentiality Requirement (CR) is High. Likewise, the Modified Confidentiality impact metric has decreased weight if the Confidentiality Requirement is Low. The Modified Confidentiality impact metric weighting is neutral if the Confidentiality Requirement is Medium. This same process is applied to the Integrity and Availability requirements.
Note that the Confidentiality Requirement will not affect the Environmental score if the (Modified Base) confidentiality impact is set to None. Also, increasing the Confidentiality Requirement from Medium to High will not change the Environmental score when the (Modified Base) impact metrics are set to High. This is because the modified impact sub score (part of the Modified Base score that calculates impact) is already at a maximum value of 10.</rdfs:comment>
        <rdfs:isDefinedBy rdf:datatype="http://www.w3.org/2001/XMLSchema#anyURI">https://www.first.org/cvss/specification-document#4-1-Security-Requirements-CR-IR-AR</rdfs:isDefinedBy>
        <rdfs:isDefinedBy xml:lang="en">https://www.first.org/cvss/v2/guide#2-3-3-Security-Requirements-CR-IR-AR</rdfs:isDefinedBy>
    </owl:Class>
    


    <!-- http://ontologies.ti-semantics.com/score#TemporalMetric -->

    <owl:Class rdf:about="http://ontologies.ti-semantics.com/score#TemporalMetric">
        <rdfs:subClassOf rdf:resource="http://ontologies.ti-semantics.com/score#Metric"/>
        <rdfs:comment rdf:datatype="http://www.w3.org/2001/XMLSchema#string">Defines the characteristics of a vulnerability that change over time but not among user environments.</rdfs:comment>
        <rdfs:isDefinedBy rdf:datatype="http://www.w3.org/2001/XMLSchema#anyURI">https://www.first.org/cvss/specification-document#3-Temporal-Metrics</rdfs:isDefinedBy>
        <rdfs:isDefinedBy xml:lang="en">https://www.first.org/cvss/v2/guide#2-2-Temporal-Metrics</rdfs:isDefinedBy>
        <rdfs:label>CVSS Temporal Metrics</rdfs:label>
    </owl:Class>
    


    <!-- 
    ///////////////////////////////////////////////////////////////////////////////////////
    //
    // Individuals
    //
    ///////////////////////////////////////////////////////////////////////////////////////
     -->

    


    <!-- http://ontologies.ti-semantics.com/score#CVSSv2AdjacentAccessVector -->

    <owl:NamedIndividual rdf:about="http://ontologies.ti-semantics.com/score#CVSSv2AdjacentAccessVector">
        <rdf:type rdf:resource="http://ontologies.ti-semantics.com/score#CVSSv2AdjacentAccessVector"/>
        <cvss_v2_score rdf:datatype="http://www.w3.org/2001/XMLSchema#decimal">0.646</cvss_v2_score>
    </owl:NamedIndividual>
    


    <!-- http://ontologies.ti-semantics.com/score#CVSSv2CompleteAvailabilityImpact -->

    <owl:NamedIndividual rdf:about="http://ontologies.ti-semantics.com/score#CVSSv2CompleteAvailabilityImpact">
        <rdf:type rdf:resource="http://ontologies.ti-semantics.com/score#CVSSv2CompleteAvailabilityImpact"/>
        <greaterScoreThan rdf:resource="http://ontologies.ti-semantics.com/score#CVSSv2PartialAvailabilityImpact"/>
        <cvss_v2_score rdf:datatype="http://www.w3.org/2001/XMLSchema#decimal">0.660</cvss_v2_score>
    </owl:NamedIndividual>
    


    <!-- http://ontologies.ti-semantics.com/score#CVSSv2CompleteConfidentialityImpact -->

    <owl:NamedIndividual rdf:about="http://ontologies.ti-semantics.com/score#CVSSv2CompleteConfidentialityImpact">
        <rdf:type rdf:resource="http://ontologies.ti-semantics.com/score#CVSSv2CompleteConfidentialityImpact"/>
        <greaterScoreThan rdf:resource="http://ontologies.ti-semantics.com/score#CVSSv2CompleteConfidentialityImpact"/>
        <cvss_v2_score rdf:datatype="http://www.w3.org/2001/XMLSchema#decimal">0.660</cvss_v2_score>
    </owl:NamedIndividual>
    


    <!-- http://ontologies.ti-semantics.com/score#CVSSv2CompleteIntegrityImpact -->

    <owl:NamedIndividual rdf:about="http://ontologies.ti-semantics.com/score#CVSSv2CompleteIntegrityImpact">
        <rdf:type rdf:resource="http://ontologies.ti-semantics.com/score#CVSSv2CompleteIntegrityImpact"/>
        <greaterScoreThan rdf:resource="http://ontologies.ti-semantics.com/score#CVSSv2PartialIntegrityImpact"/>
        <cvss_v2_score rdf:datatype="http://www.w3.org/2001/XMLSchema#decimal">0.660</cvss_v2_score>
    </owl:NamedIndividual>
    


    <!-- http://ontologies.ti-semantics.com/score#CVSSv2ConfirmedReportConfidence -->

    <owl:NamedIndividual rdf:about="http://ontologies.ti-semantics.com/score#CVSSv2ConfirmedReportConfidence">
        <rdf:type rdf:resource="http://ontologies.ti-semantics.com/score#CVSSv2ConfirmedReportConfidence"/>
        <greaterScoreThan rdf:resource="http://ontologies.ti-semantics.com/score#CVSSv2UncorroboratedReportConfidence"/>
    </owl:NamedIndividual>
    


    <!-- http://ontologies.ti-semantics.com/score#CVSSv2FunctionalExploitability -->

    <owl:NamedIndividual rdf:about="http://ontologies.ti-semantics.com/score#CVSSv2FunctionalExploitability">
        <rdf:type rdf:resource="http://ontologies.ti-semantics.com/score#CVSSv2FunctionalExploitability"/>
        <greaterScoreThan rdf:resource="http://ontologies.ti-semantics.com/score#CVSSv2ProofOfConceptExploitability"/>
        <cvss_v2_score rdf:datatype="http://www.w3.org/2001/XMLSchema#decimal">0.95</cvss_v2_score>
    </owl:NamedIndividual>
    


    <!-- http://ontologies.ti-semantics.com/score#CVSSv2HighAccessComplexity -->

    <owl:NamedIndividual rdf:about="http://ontologies.ti-semantics.com/score#CVSSv2HighAccessComplexity">
        <rdf:type rdf:resource="http://ontologies.ti-semantics.com/score#CVSSv2HighAccessComplexity"/>
        <cvss_v3_score rdf:datatype="http://www.w3.org/2001/XMLSchema#decimal">0.44</cvss_v3_score>
    </owl:NamedIndividual>
    


    <!-- http://ontologies.ti-semantics.com/score#CVSSv2HighAvailabilityRequirement -->

    <owl:NamedIndividual rdf:about="http://ontologies.ti-semantics.com/score#CVSSv2HighAvailabilityRequirement">
        <rdf:type rdf:resource="http://ontologies.ti-semantics.com/score#CVSSv2HighAvailabilityRequirement"/>
        <greaterScoreThan rdf:resource="http://ontologies.ti-semantics.com/score#CVSSv2MediumAvailabilityRequirement"/>
        <cvss_v2_score rdf:datatype="http://www.w3.org/2001/XMLSchema#decimal">1.51</cvss_v2_score>
    </owl:NamedIndividual>
    


    <!-- http://ontologies.ti-semantics.com/score#CVSSv2HighCollateralDamagePotential -->

    <owl:NamedIndividual rdf:about="http://ontologies.ti-semantics.com/score#CVSSv2HighCollateralDamagePotential">
        <rdf:type rdf:resource="http://ontologies.ti-semantics.com/score#CVSSv2HighCollateralDamagePotential"/>
        <greaterScoreThan rdf:resource="http://ontologies.ti-semantics.com/score#CVSSv2MediumHighCollateralDamagePotential"/>
        <cvss_v2_score rdf:datatype="http://www.w3.org/2001/XMLSchema#decimal">0.5</cvss_v2_score>
    </owl:NamedIndividual>
    


    <!-- http://ontologies.ti-semantics.com/score#CVSSv2HighConfidentialityRequirement -->

    <owl:NamedIndividual rdf:about="http://ontologies.ti-semantics.com/score#CVSSv2HighConfidentialityRequirement">
        <rdf:type rdf:resource="http://ontologies.ti-semantics.com/score#CVSSv2HighConfidentialityRequirement"/>
        <greaterScoreThan rdf:resource="http://ontologies.ti-semantics.com/score#CVSSv2MediumConfidentialityRequirement"/>
        <cvss_v2_score rdf:datatype="http://www.w3.org/2001/XMLSchema#decimal">1.51</cvss_v2_score>
    </owl:NamedIndividual>
    


    <!-- http://ontologies.ti-semantics.com/score#CVSSv2HighExploitability -->

    <owl:NamedIndividual rdf:about="http://ontologies.ti-semantics.com/score#CVSSv2HighExploitability">
        <rdf:type rdf:resource="http://ontologies.ti-semantics.com/score#CVSSv2HighExploitability"/>
        <greaterScoreThan rdf:resource="http://ontologies.ti-semantics.com/score#CVSSv2FunctionalExploitability"/>
        <cvss_v2_score rdf:datatype="http://www.w3.org/2001/XMLSchema#decimal">1</cvss_v2_score>
    </owl:NamedIndividual>
    


    <!-- http://ontologies.ti-semantics.com/score#CVSSv2HighIntegrityRequirement -->

    <owl:NamedIndividual rdf:about="http://ontologies.ti-semantics.com/score#CVSSv2HighIntegrityRequirement">
        <rdf:type rdf:resource="http://ontologies.ti-semantics.com/score#CVSSv2HighIntegrityRequirement"/>
        <greaterScoreThan rdf:resource="http://ontologies.ti-semantics.com/score#CVSSv2MediumIntegrityRequirement"/>
        <cvss_v2_score rdf:datatype="http://www.w3.org/2001/XMLSchema#decimal">1.51</cvss_v2_score>
    </owl:NamedIndividual>
    


    <!-- http://ontologies.ti-semantics.com/score#CVSSv2HighTargetCount -->

    <owl:NamedIndividual rdf:about="http://ontologies.ti-semantics.com/score#CVSSv2HighTargetCount">
        <rdf:type rdf:resource="http://ontologies.ti-semantics.com/score#CVSSv2HighTargetCount"/>
        <greaterScoreThan rdf:resource="http://ontologies.ti-semantics.com/score#CVSSv2MediumTargetCount"/>
        <cvss_v2_score rdf:datatype="http://www.w3.org/2001/XMLSchema#decimal">1.0</cvss_v2_score>
    </owl:NamedIndividual>
    


    <!-- http://ontologies.ti-semantics.com/score#CVSSv2LocalAccessVector -->

    <owl:NamedIndividual rdf:about="http://ontologies.ti-semantics.com/score#CVSSv2LocalAccessVector">
        <rdf:type rdf:resource="http://ontologies.ti-semantics.com/score#CVSSv2LocalAccessVector"/>
        <cvss_v2_score rdf:datatype="http://www.w3.org/2001/XMLSchema#decimal">0.395</cvss_v2_score>
    </owl:NamedIndividual>
    


    <!-- http://ontologies.ti-semantics.com/score#CVSSv2LowAccessComplexity -->

    <owl:NamedIndividual rdf:about="http://ontologies.ti-semantics.com/score#CVSSv2LowAccessComplexity">
        <rdf:type rdf:resource="http://ontologies.ti-semantics.com/score#CVSSv2LowAccessComplexity"/>
        <cvss_v3_score rdf:datatype="http://www.w3.org/2001/XMLSchema#decimal">0.77</cvss_v3_score>
    </owl:NamedIndividual>
    


    <!-- http://ontologies.ti-semantics.com/score#CVSSv2LowAvailabilityRequirement -->

    <owl:NamedIndividual rdf:about="http://ontologies.ti-semantics.com/score#CVSSv2LowAvailabilityRequirement">
        <rdf:type rdf:resource="http://ontologies.ti-semantics.com/score#CVSSv2LowAvailabilityRequirement"/>
        <cvss_v2_score rdf:datatype="http://www.w3.org/2001/XMLSchema#decimal">0.5</cvss_v2_score>
    </owl:NamedIndividual>
    


    <!-- http://ontologies.ti-semantics.com/score#CVSSv2LowCollateralDamagePotential -->

    <owl:NamedIndividual rdf:about="http://ontologies.ti-semantics.com/score#CVSSv2LowCollateralDamagePotential">
        <rdf:type rdf:resource="http://ontologies.ti-semantics.com/score#CVSSv2LowCollateralDamagePotential"/>
        <greaterScoreThan rdf:resource="http://ontologies.ti-semantics.com/score#CVSSv2NoCollateralDamagePotential"/>
        <cvss_v2_score rdf:datatype="http://www.w3.org/2001/XMLSchema#decimal">0.1</cvss_v2_score>
    </owl:NamedIndividual>
    


    <!-- http://ontologies.ti-semantics.com/score#CVSSv2LowConfidentialityRequirement -->

    <owl:NamedIndividual rdf:about="http://ontologies.ti-semantics.com/score#CVSSv2LowConfidentialityRequirement">
        <rdf:type rdf:resource="http://ontologies.ti-semantics.com/score#CVSSv2LowConfidentialityRequirement"/>
        <cvss_v2_score rdf:datatype="http://www.w3.org/2001/XMLSchema#decimal">0.5</cvss_v2_score>
    </owl:NamedIndividual>
    


    <!-- http://ontologies.ti-semantics.com/score#CVSSv2LowIntegrityRequirement -->

    <owl:NamedIndividual rdf:about="http://ontologies.ti-semantics.com/score#CVSSv2LowIntegrityRequirement">
        <rdf:type rdf:resource="http://ontologies.ti-semantics.com/score#CVSSv2LowIntegrityRequirement"/>
        <cvss_v2_score rdf:datatype="http://www.w3.org/2001/XMLSchema#decimal">0.5</cvss_v2_score>
    </owl:NamedIndividual>
    


    <!-- http://ontologies.ti-semantics.com/score#CVSSv2LowMediumCollateralDamagePotential -->

    <owl:NamedIndividual rdf:about="http://ontologies.ti-semantics.com/score#CVSSv2LowMediumCollateralDamagePotential">
        <rdf:type rdf:resource="http://ontologies.ti-semantics.com/score#CVSSv2LowMediumCollateralDamagePotential"/>
        <greaterScoreThan rdf:resource="http://ontologies.ti-semantics.com/score#CVSSv2LowCollateralDamagePotential"/>
        <cvss_v2_score rdf:datatype="http://www.w3.org/2001/XMLSchema#decimal">0.3</cvss_v2_score>
    </owl:NamedIndividual>
    


    <!-- http://ontologies.ti-semantics.com/score#CVSSv2LowTargetCount -->

    <owl:NamedIndividual rdf:about="http://ontologies.ti-semantics.com/score#CVSSv2LowTargetCount">
        <rdf:type rdf:resource="http://ontologies.ti-semantics.com/score#CVSSv2LowTargetCount"/>
        <greaterScoreThan rdf:resource="http://ontologies.ti-semantics.com/score#CVSSv2NilTargetCount"/>
        <cvss_v2_score rdf:datatype="http://www.w3.org/2001/XMLSchema#decimal">0.25</cvss_v2_score>
    </owl:NamedIndividual>
    


    <!-- http://ontologies.ti-semantics.com/score#CVSSv2MediumAvailabilityRequirement -->

    <owl:NamedIndividual rdf:about="http://ontologies.ti-semantics.com/score#CVSSv2MediumAvailabilityRequirement">
        <rdf:type rdf:resource="http://ontologies.ti-semantics.com/score#CVSSv2MediumAvailabilityRequirement"/>
        <greaterScoreThan rdf:resource="http://ontologies.ti-semantics.com/score#CVSSv2LowAvailabilityRequirement"/>
        <cvss_v2_score rdf:datatype="http://www.w3.org/2001/XMLSchema#decimal">1</cvss_v2_score>
    </owl:NamedIndividual>
    


    <!-- http://ontologies.ti-semantics.com/score#CVSSv2MediumConfidentialityRequirement -->

    <owl:NamedIndividual rdf:about="http://ontologies.ti-semantics.com/score#CVSSv2MediumConfidentialityRequirement">
        <rdf:type rdf:resource="http://ontologies.ti-semantics.com/score#CVSSv2MediumConfidentialityRequirement"/>
        <greaterScoreThan rdf:resource="http://ontologies.ti-semantics.com/score#CVSSv2LowConfidentialityRequirement"/>
        <cvss_v2_score rdf:datatype="http://www.w3.org/2001/XMLSchema#decimal">1</cvss_v2_score>
    </owl:NamedIndividual>
    


    <!-- http://ontologies.ti-semantics.com/score#CVSSv2MediumHighCollateralDamagePotential -->

    <owl:NamedIndividual rdf:about="http://ontologies.ti-semantics.com/score#CVSSv2MediumHighCollateralDamagePotential">
        <rdf:type rdf:resource="http://ontologies.ti-semantics.com/score#CVSSv2MediumHighCollateralDamagePotential"/>
        <greaterScoreThan rdf:resource="http://ontologies.ti-semantics.com/score#CVSSv2LowMediumCollateralDamagePotential"/>
        <cvss_v2_score rdf:datatype="http://www.w3.org/2001/XMLSchema#decimal">0.4</cvss_v2_score>
    </owl:NamedIndividual>
    


    <!-- http://ontologies.ti-semantics.com/score#CVSSv2MediumIntegrityRequirement -->

    <owl:NamedIndividual rdf:about="http://ontologies.ti-semantics.com/score#CVSSv2MediumIntegrityRequirement">
        <rdf:type rdf:resource="http://ontologies.ti-semantics.com/score#CVSSv2MediumIntegrityRequirement"/>
        <greaterScoreThan rdf:resource="http://ontologies.ti-semantics.com/score#CVSSv2LowIntegrityRequirement"/>
        <cvss_v2_score rdf:datatype="http://www.w3.org/2001/XMLSchema#decimal">1</cvss_v2_score>
    </owl:NamedIndividual>
    


    <!-- http://ontologies.ti-semantics.com/score#CVSSv2MediumTargetCount -->

    <owl:NamedIndividual rdf:about="http://ontologies.ti-semantics.com/score#CVSSv2MediumTargetCount">
        <rdf:type rdf:resource="http://ontologies.ti-semantics.com/score#CVSSv2MediumTargetCount"/>
        <greaterScoreThan rdf:resource="http://ontologies.ti-semantics.com/score#CVSSv2LowTargetCount"/>
        <cvss_v2_score rdf:datatype="http://www.w3.org/2001/XMLSchema#decimal">0.75</cvss_v2_score>
    </owl:NamedIndividual>
    


    <!-- http://ontologies.ti-semantics.com/score#CVSSv2MultipleAuthentications -->

    <owl:NamedIndividual rdf:about="http://ontologies.ti-semantics.com/score#CVSSv2MultipleAuthentications">
        <rdf:type rdf:resource="http://ontologies.ti-semantics.com/score#CVSSv2MultipleAuthentications"/>
        <cvss_v2_score rdf:datatype="http://www.w3.org/2001/XMLSchema#decimal">0.45</cvss_v2_score>
    </owl:NamedIndividual>
    


    <!-- http://ontologies.ti-semantics.com/score#CVSSv2NetworkAccessVector -->

    <owl:NamedIndividual rdf:about="http://ontologies.ti-semantics.com/score#CVSSv2NetworkAccessVector">
        <rdf:type rdf:resource="http://ontologies.ti-semantics.com/score#CVSSv2NetworkAccessVector"/>
        <cvss_v2_score rdf:datatype="http://www.w3.org/2001/XMLSchema#decimal">1.0</cvss_v2_score>
    </owl:NamedIndividual>
    


    <!-- http://ontologies.ti-semantics.com/score#CVSSv2NilTargetCount -->

    <owl:NamedIndividual rdf:about="http://ontologies.ti-semantics.com/score#CVSSv2NilTargetCount">
        <rdf:type rdf:resource="http://ontologies.ti-semantics.com/score#CVSSv2NilTargetCount"/>
        <cvss_v2_score rdf:datatype="http://www.w3.org/2001/XMLSchema#decimal">0</cvss_v2_score>
    </owl:NamedIndividual>
    


    <!-- http://ontologies.ti-semantics.com/score#CVSSv2NoAuthentication -->

    <owl:NamedIndividual rdf:about="http://ontologies.ti-semantics.com/score#CVSSv2NoAuthentication">
        <rdf:type rdf:resource="http://ontologies.ti-semantics.com/score#CVSSv2NoAuthentication"/>
        <greaterScoreThan rdf:resource="http://ontologies.ti-semantics.com/score#CVSSv2SingleAuthentication"/>
        <cvss_v2_score rdf:datatype="http://www.w3.org/2001/XMLSchema#decimal">0.704</cvss_v2_score>
    </owl:NamedIndividual>
    


    <!-- http://ontologies.ti-semantics.com/score#CVSSv2NoAvailabilityImpact -->

    <owl:NamedIndividual rdf:about="http://ontologies.ti-semantics.com/score#CVSSv2NoAvailabilityImpact">
        <rdf:type rdf:resource="http://ontologies.ti-semantics.com/score#CVSSv2NoAvailabilityImpact"/>
    </owl:NamedIndividual>
    


    <!-- http://ontologies.ti-semantics.com/score#CVSSv2NoCollateralDamagePotential -->

    <owl:NamedIndividual rdf:about="http://ontologies.ti-semantics.com/score#CVSSv2NoCollateralDamagePotential">
        <rdf:type rdf:resource="http://ontologies.ti-semantics.com/score#CVSSv2NoCollateralDamagePotential"/>
        <cvss_v2_score rdf:datatype="http://www.w3.org/2001/XMLSchema#decimal">0</cvss_v2_score>
    </owl:NamedIndividual>
    


    <!-- http://ontologies.ti-semantics.com/score#CVSSv2NoConfidentialityImpact -->

    <owl:NamedIndividual rdf:about="http://ontologies.ti-semantics.com/score#CVSSv2NoConfidentialityImpact">
        <rdf:type rdf:resource="http://ontologies.ti-semantics.com/score#CVSSv2NoConfidentialityImpact"/>
        <cvss_v2_score rdf:datatype="http://www.w3.org/2001/XMLSchema#decimal">0</cvss_v2_score>
    </owl:NamedIndividual>
    


    <!-- http://ontologies.ti-semantics.com/score#CVSSv2NoIntegrityImpact -->

    <owl:NamedIndividual rdf:about="http://ontologies.ti-semantics.com/score#CVSSv2NoIntegrityImpact">
        <rdf:type rdf:resource="http://ontologies.ti-semantics.com/score#CVSSv2NoIntegrityImpact"/>
    </owl:NamedIndividual>
    


    <!-- http://ontologies.ti-semantics.com/score#CVSSv2NotDefinedAvailabilityRequirement -->

    <owl:NamedIndividual rdf:about="http://ontologies.ti-semantics.com/score#CVSSv2NotDefinedAvailabilityRequirement">
        <rdf:type rdf:resource="http://ontologies.ti-semantics.com/score#CVSSv2NotDefinedAvailabilityRequirement"/>
        <cvss_v2_score rdf:datatype="http://www.w3.org/2001/XMLSchema#decimal">1</cvss_v2_score>
    </owl:NamedIndividual>
    


    <!-- http://ontologies.ti-semantics.com/score#CVSSv2NotDefinedCollateralDamagePotential -->

    <owl:NamedIndividual rdf:about="http://ontologies.ti-semantics.com/score#CVSSv2NotDefinedCollateralDamagePotential">
        <rdf:type rdf:resource="http://ontologies.ti-semantics.com/score#CVSSv2NotDefinedCollateralDamagePotential"/>
        <cvss_v2_score rdf:datatype="http://www.w3.org/2001/XMLSchema#decimal">0</cvss_v2_score>
    </owl:NamedIndividual>
    


    <!-- http://ontologies.ti-semantics.com/score#CVSSv2NotDefinedConfidentialityRequirement -->

    <owl:NamedIndividual rdf:about="http://ontologies.ti-semantics.com/score#CVSSv2NotDefinedConfidentialityRequirement">
        <rdf:type rdf:resource="http://ontologies.ti-semantics.com/score#CVSSv2NotDefinedConfidentialityRequirement"/>
        <cvss_v2_score rdf:datatype="http://www.w3.org/2001/XMLSchema#decimal">1</cvss_v2_score>
    </owl:NamedIndividual>
    


    <!-- http://ontologies.ti-semantics.com/score#CVSSv2NotDefinedExploitability -->

    <owl:NamedIndividual rdf:about="http://ontologies.ti-semantics.com/score#CVSSv2NotDefinedExploitability">
        <rdf:type rdf:resource="http://ontologies.ti-semantics.com/score#CVSSv2NotDefinedExploitability"/>
        <cvss_v2_score rdf:datatype="http://www.w3.org/2001/XMLSchema#decimal">1</cvss_v2_score>
    </owl:NamedIndividual>
    


    <!-- http://ontologies.ti-semantics.com/score#CVSSv2NotDefinedIntegrityRequirement -->

    <owl:NamedIndividual rdf:about="http://ontologies.ti-semantics.com/score#CVSSv2NotDefinedIntegrityRequirement">
        <rdf:type rdf:resource="http://ontologies.ti-semantics.com/score#CVSSv2NotDefinedIntegrityRequirement"/>
        <cvss_v2_score rdf:datatype="http://www.w3.org/2001/XMLSchema#decimal">1</cvss_v2_score>
    </owl:NamedIndividual>
    


    <!-- http://ontologies.ti-semantics.com/score#CVSSv2NotDefinedRemediation -->

    <owl:NamedIndividual rdf:about="http://ontologies.ti-semantics.com/score#CVSSv2NotDefinedRemediation">
        <rdf:type rdf:resource="http://ontologies.ti-semantics.com/score#CVSSv2NotDefinedRemediation"/>
        <cvss_v2_score rdf:datatype="http://www.w3.org/2001/XMLSchema#decimal">1</cvss_v2_score>
    </owl:NamedIndividual>
    


    <!-- http://ontologies.ti-semantics.com/score#CVSSv2NotDefinedTargetCount -->

    <owl:NamedIndividual rdf:about="http://ontologies.ti-semantics.com/score#CVSSv2NotDefinedTargetCount">
        <rdf:type rdf:resource="http://ontologies.ti-semantics.com/score#CVSSv2NotDefinedTargetCount"/>
        <cvss_v2_score rdf:datatype="http://www.w3.org/2001/XMLSchema#decimal">1</cvss_v2_score>
    </owl:NamedIndividual>
    


    <!-- http://ontologies.ti-semantics.com/score#CVSSv2OfficialFixRemediation -->

    <owl:NamedIndividual rdf:about="http://ontologies.ti-semantics.com/score#CVSSv2OfficialFixRemediation">
        <rdf:type rdf:resource="http://ontologies.ti-semantics.com/score#CVSSv2OfficialFixRemediation"/>
        <cvss_v2_score rdf:datatype="http://www.w3.org/2001/XMLSchema#decimal">0.87</cvss_v2_score>
    </owl:NamedIndividual>
    


    <!-- http://ontologies.ti-semantics.com/score#CVSSv2PartialAvailabilityImpact -->

    <owl:NamedIndividual rdf:about="http://ontologies.ti-semantics.com/score#CVSSv2PartialAvailabilityImpact">
        <rdf:type rdf:resource="http://ontologies.ti-semantics.com/score#CVSSv2PartialAvailabilityImpact"/>
        <greaterScoreThan rdf:resource="http://ontologies.ti-semantics.com/score#CVSSv2NoAvailabilityImpact"/>
        <cvss_v2_score rdf:datatype="http://www.w3.org/2001/XMLSchema#decimal">0.275</cvss_v2_score>
    </owl:NamedIndividual>
    


    <!-- http://ontologies.ti-semantics.com/score#CVSSv2PartialConfidentialityImpact -->

    <owl:NamedIndividual rdf:about="http://ontologies.ti-semantics.com/score#CVSSv2PartialConfidentialityImpact">
        <rdf:type rdf:resource="http://ontologies.ti-semantics.com/score#CVSSv2PartialConfidentialityImpact"/>
        <greaterScoreThan rdf:resource="http://ontologies.ti-semantics.com/score#CVSSv2NoConfidentialityImpact"/>
        <cvss_v2_score rdf:datatype="http://www.w3.org/2001/XMLSchema#decimal">0.275</cvss_v2_score>
    </owl:NamedIndividual>
    


    <!-- http://ontologies.ti-semantics.com/score#CVSSv2PartialIntegrityImpact -->

    <owl:NamedIndividual rdf:about="http://ontologies.ti-semantics.com/score#CVSSv2PartialIntegrityImpact">
        <rdf:type rdf:resource="http://ontologies.ti-semantics.com/score#CVSSv2PartialIntegrityImpact"/>
        <greaterScoreThan rdf:resource="http://ontologies.ti-semantics.com/score#CVSSv2NoIntegrityImpact"/>
        <cvss_v2_score rdf:datatype="http://www.w3.org/2001/XMLSchema#decimal">0.275</cvss_v2_score>
    </owl:NamedIndividual>
    


    <!-- http://ontologies.ti-semantics.com/score#CVSSv2ProofOfConceptExploitability -->

    <owl:NamedIndividual rdf:about="http://ontologies.ti-semantics.com/score#CVSSv2ProofOfConceptExploitability">
        <rdf:type rdf:resource="http://ontologies.ti-semantics.com/score#CVSSv2ProofOfConceptExploitability"/>
        <greaterScoreThan rdf:resource="http://ontologies.ti-semantics.com/score#CVSSv2UnprovenExploitability"/>
        <cvss_v2_score rdf:datatype="http://www.w3.org/2001/XMLSchema#decimal">0.9</cvss_v2_score>
    </owl:NamedIndividual>
    


    <!-- http://ontologies.ti-semantics.com/score#CVSSv2SingleAuthentication -->

    <owl:NamedIndividual rdf:about="http://ontologies.ti-semantics.com/score#CVSSv2SingleAuthentication">
        <rdf:type rdf:resource="http://ontologies.ti-semantics.com/score#CVSSv2SingleAuthentication"/>
        <greaterScoreThan rdf:resource="http://ontologies.ti-semantics.com/score#CVSSv2MultipleAuthentications"/>
        <cvss_v2_score rdf:datatype="http://www.w3.org/2001/XMLSchema#decimal">0.56</cvss_v2_score>
    </owl:NamedIndividual>
    


    <!-- http://ontologies.ti-semantics.com/score#CVSSv2TemporaryFixRemediation -->

    <owl:NamedIndividual rdf:about="http://ontologies.ti-semantics.com/score#CVSSv2TemporaryFixRemediation">
        <rdf:type rdf:resource="http://ontologies.ti-semantics.com/score#CVSSv2TemporaryFixRemediation"/>
        <greaterScoreThan rdf:resource="http://ontologies.ti-semantics.com/score#CVSSv2OfficialFixRemediation"/>
        <cvss_v2_score rdf:datatype="http://www.w3.org/2001/XMLSchema#decimal">0.9</cvss_v2_score>
    </owl:NamedIndividual>
    


    <!-- http://ontologies.ti-semantics.com/score#CVSSv2UnavailableRemediation -->

    <owl:NamedIndividual rdf:about="http://ontologies.ti-semantics.com/score#CVSSv2UnavailableRemediation">
        <rdf:type rdf:resource="http://ontologies.ti-semantics.com/score#CVSSv2UnavailableRemediation"/>
        <greaterScoreThan rdf:resource="http://ontologies.ti-semantics.com/score#CVSSv2WorkaroundRemediation"/>
        <cvss_v2_score rdf:datatype="http://www.w3.org/2001/XMLSchema#decimal">1</cvss_v2_score>
    </owl:NamedIndividual>
    


    <!-- http://ontologies.ti-semantics.com/score#CVSSv2UnconfirmedReportConfidence -->

    <owl:NamedIndividual rdf:about="http://ontologies.ti-semantics.com/score#CVSSv2UnconfirmedReportConfidence">
        <rdf:type rdf:resource="http://ontologies.ti-semantics.com/score#CVSSv2UnconfirmedReportConfidence"/>
    </owl:NamedIndividual>
    


    <!-- http://ontologies.ti-semantics.com/score#CVSSv2UncorroboratedReportConfidence -->

    <owl:NamedIndividual rdf:about="http://ontologies.ti-semantics.com/score#CVSSv2UncorroboratedReportConfidence">
        <rdf:type rdf:resource="http://ontologies.ti-semantics.com/score#CVSSv2UncorroboratedReportConfidence"/>
        <greaterScoreThan rdf:resource="http://ontologies.ti-semantics.com/score#CVSSv2UnconfirmedReportConfidence"/>
    </owl:NamedIndividual>
    


    <!-- http://ontologies.ti-semantics.com/score#CVSSv2UnprovenExploitability -->

    <owl:NamedIndividual rdf:about="http://ontologies.ti-semantics.com/score#CVSSv2UnprovenExploitability">
        <rdf:type rdf:resource="http://ontologies.ti-semantics.com/score#CVSSv2UnprovenExploitability"/>
        <cvss_v2_score rdf:datatype="http://www.w3.org/2001/XMLSchema#decimal">0.85</cvss_v2_score>
    </owl:NamedIndividual>
    


    <!-- http://ontologies.ti-semantics.com/score#CVSSv2WorkaroundRemediation -->

    <owl:NamedIndividual rdf:about="http://ontologies.ti-semantics.com/score#CVSSv2WorkaroundRemediation">
        <rdf:type rdf:resource="http://ontologies.ti-semantics.com/score#CVSSv2WorkaroundRemediation"/>
        <greaterScoreThan rdf:resource="http://ontologies.ti-semantics.com/score#CVSSv2TemporaryFixRemediation"/>
        <cvss_v2_score rdf:datatype="http://www.w3.org/2001/XMLSchema#decimal">0.95</cvss_v2_score>
    </owl:NamedIndividual>
    


    <!-- http://ontologies.ti-semantics.com/score#CVSSv3AdjacentAttackVector -->

    <owl:NamedIndividual rdf:about="http://ontologies.ti-semantics.com/score#CVSSv3AdjacentAttackVector">
        <rdf:type rdf:resource="http://ontologies.ti-semantics.com/score#CVSSv3AdjacentAttackVector"/>
        <greaterScoreThan rdf:resource="http://ontologies.ti-semantics.com/score#CVSSv3LocalAttackVector"/>
        <cvss_v3_score rdf:datatype="http://www.w3.org/2001/XMLSchema#decimal">0.62</cvss_v3_score>
    </owl:NamedIndividual>
    


    <!-- http://ontologies.ti-semantics.com/score#CVSSv3ChangedScope -->

    <owl:NamedIndividual rdf:about="http://ontologies.ti-semantics.com/score#CVSSv3ChangedScope">
        <rdf:type rdf:resource="http://ontologies.ti-semantics.com/score#CVSSv3ChangedScope"/>
    </owl:NamedIndividual>
    


    <!-- http://ontologies.ti-semantics.com/score#CVSSv3ConfirmedReportConfidence -->

    <owl:NamedIndividual rdf:about="http://ontologies.ti-semantics.com/score#CVSSv3ConfirmedReportConfidence">
        <rdf:type rdf:resource="http://ontologies.ti-semantics.com/score#CVSSv3ConfirmedReportConfidence"/>
        <greaterScoreThan rdf:resource="http://ontologies.ti-semantics.com/score#CVSSv3ReasonableReportConfidence"/>
        <cvss_v3_score rdf:datatype="http://www.w3.org/2001/XMLSchema#decimal">1</cvss_v3_score>
    </owl:NamedIndividual>
    


    <!-- http://ontologies.ti-semantics.com/score#CVSSv3FunctionalExploitCodeMaturity -->

    <owl:NamedIndividual rdf:about="http://ontologies.ti-semantics.com/score#CVSSv3FunctionalExploitCodeMaturity">
        <rdf:type rdf:resource="http://ontologies.ti-semantics.com/score#CVSSv3FunctionalExploitCodeMaturity"/>
        <greaterScoreThan rdf:resource="http://ontologies.ti-semantics.com/score#CVSSv3ProofOfConceptExploitCodeMaturity"/>
        <cvss_v3_score rdf:datatype="http://www.w3.org/2001/XMLSchema#decimal">0.97</cvss_v3_score>
    </owl:NamedIndividual>
    


    <!-- http://ontologies.ti-semantics.com/score#CVSSv3HighAttackComplexity -->

    <owl:NamedIndividual rdf:about="http://ontologies.ti-semantics.com/score#CVSSv3HighAttackComplexity">
        <rdf:type rdf:resource="http://ontologies.ti-semantics.com/score#CVSSv3HighAttackComplexity"/>
        <cvss_v3_score rdf:datatype="http://www.w3.org/2001/XMLSchema#decimal">0.44</cvss_v3_score>
    </owl:NamedIndividual>
    


    <!-- http://ontologies.ti-semantics.com/score#CVSSv3HighAvailabilityImpact -->

    <owl:NamedIndividual rdf:about="http://ontologies.ti-semantics.com/score#CVSSv3HighAvailabilityImpact">
        <rdf:type rdf:resource="http://ontologies.ti-semantics.com/score#CVSSv3HighAvailabilityImpact"/>
        <greaterScoreThan rdf:resource="http://ontologies.ti-semantics.com/score#CVSSv3LowAvailabilityImpact"/>
        <cvss_v3_score rdf:datatype="http://www.w3.org/2001/XMLSchema#decimal">0.56</cvss_v3_score>
    </owl:NamedIndividual>
    


    <!-- http://ontologies.ti-semantics.com/score#CVSSv3HighAvailabilityRequirement -->

    <owl:NamedIndividual rdf:about="http://ontologies.ti-semantics.com/score#CVSSv3HighAvailabilityRequirement">
        <rdf:type rdf:resource="http://ontologies.ti-semantics.com/score#CVSSv3HighAvailabilityRequirement"/>
        <greaterScoreThan rdf:resource="http://ontologies.ti-semantics.com/score#CVSSv3MediumAvailabilityRequirement"/>
        <cvss_v2_score rdf:datatype="http://www.w3.org/2001/XMLSchema#decimal">1.51</cvss_v2_score>
    </owl:NamedIndividual>
    


    <!-- http://ontologies.ti-semantics.com/score#CVSSv3HighConfidentialityImpact -->

    <owl:NamedIndividual rdf:about="http://ontologies.ti-semantics.com/score#CVSSv3HighConfidentialityImpact">
        <rdf:type rdf:resource="http://ontologies.ti-semantics.com/score#CVSSv3HighConfidentialityImpact"/>
        <greaterScoreThan rdf:resource="http://ontologies.ti-semantics.com/score#CVSSv3LowConfidentialityImpact"/>
        <cvss_v3_score rdf:datatype="http://www.w3.org/2001/XMLSchema#decimal">0.56</cvss_v3_score>
    </owl:NamedIndividual>
    


    <!-- http://ontologies.ti-semantics.com/score#CVSSv3HighExploitCodeMaturity -->

    <owl:NamedIndividual rdf:about="http://ontologies.ti-semantics.com/score#CVSSv3HighExploitCodeMaturity">
        <rdf:type rdf:resource="http://ontologies.ti-semantics.com/score#CVSSv3HighExploitCodeMaturity"/>
        <greaterScoreThan rdf:resource="http://ontologies.ti-semantics.com/score#CVSSv3FunctionalExploitCodeMaturity"/>
        <cvss_v3_score rdf:datatype="http://www.w3.org/2001/XMLSchema#decimal">1</cvss_v3_score>
    </owl:NamedIndividual>
    


    <!-- http://ontologies.ti-semantics.com/score#CVSSv3HighIntegrityImpact -->

    <owl:NamedIndividual rdf:about="http://ontologies.ti-semantics.com/score#CVSSv3HighIntegrityImpact">
        <rdf:type rdf:resource="http://ontologies.ti-semantics.com/score#CVSSv3HighIntegrityImpact"/>
        <greaterScoreThan rdf:resource="http://ontologies.ti-semantics.com/score#CVSSv3LowIntegrityImpact"/>
        <cvss_v3_score rdf:datatype="http://www.w3.org/2001/XMLSchema#decimal">0.56</cvss_v3_score>
    </owl:NamedIndividual>
    


    <!-- http://ontologies.ti-semantics.com/score#CVSSv3HighPrivilegesRequired -->

    <owl:NamedIndividual rdf:about="http://ontologies.ti-semantics.com/score#CVSSv3HighPrivilegesRequired">
        <rdf:type rdf:resource="http://ontologies.ti-semantics.com/score#CVSSv3HighPrivilegesRequired"/>
        <cvss_v3_score rdf:datatype="http://www.w3.org/2001/XMLSchema#decimal">0.27</cvss_v3_score>
    </owl:NamedIndividual>
    


    <!-- http://ontologies.ti-semantics.com/score#CVSSv3LocalAttackVector -->

    <owl:NamedIndividual rdf:about="http://ontologies.ti-semantics.com/score#CVSSv3LocalAttackVector">
        <rdf:type rdf:resource="http://ontologies.ti-semantics.com/score#CVSSv3LocalAttackVector"/>
        <greaterScoreThan rdf:resource="http://ontologies.ti-semantics.com/score#CVSSv3PhysicalAttackVector"/>
        <cvss_v3_score rdf:datatype="http://www.w3.org/2001/XMLSchema#decimal">0.55</cvss_v3_score>
    </owl:NamedIndividual>
    


    <!-- http://ontologies.ti-semantics.com/score#CVSSv3LowAttackComplexity -->

    <owl:NamedIndividual rdf:about="http://ontologies.ti-semantics.com/score#CVSSv3LowAttackComplexity">
        <rdf:type rdf:resource="http://ontologies.ti-semantics.com/score#CVSSv3LowAttackComplexity"/>
        <cvss_v3_score rdf:datatype="http://www.w3.org/2001/XMLSchema#decimal">0.77</cvss_v3_score>
    </owl:NamedIndividual>
    


    <!-- http://ontologies.ti-semantics.com/score#CVSSv3LowAvailabilityImpact -->

    <owl:NamedIndividual rdf:about="http://ontologies.ti-semantics.com/score#CVSSv3LowAvailabilityImpact">
        <rdf:type rdf:resource="http://ontologies.ti-semantics.com/score#CVSSv3LowAvailabilityImpact"/>
        <greaterScoreThan rdf:resource="http://ontologies.ti-semantics.com/score#CVSSv3NoAvailabilityImpact"/>
        <cvss_v3_score rdf:datatype="http://www.w3.org/2001/XMLSchema#decimal">0.22</cvss_v3_score>
    </owl:NamedIndividual>
    


    <!-- http://ontologies.ti-semantics.com/score#CVSSv3LowAvailabilityRequirement -->

    <owl:NamedIndividual rdf:about="http://ontologies.ti-semantics.com/score#CVSSv3LowAvailabilityRequirement">
        <rdf:type rdf:resource="http://ontologies.ti-semantics.com/score#CVSSv3LowAvailabilityRequirement"/>
        <cvss_v2_score rdf:datatype="http://www.w3.org/2001/XMLSchema#decimal">0.5</cvss_v2_score>
    </owl:NamedIndividual>
    


    <!-- http://ontologies.ti-semantics.com/score#CVSSv3LowConfidentialityImpact -->

    <owl:NamedIndividual rdf:about="http://ontologies.ti-semantics.com/score#CVSSv3LowConfidentialityImpact">
        <rdf:type rdf:resource="http://ontologies.ti-semantics.com/score#CVSSv3LowConfidentialityImpact"/>
        <greaterScoreThan rdf:resource="http://ontologies.ti-semantics.com/score#CVSSv3NoConfidentialityImpact"/>
        <cvss_v3_score rdf:datatype="http://www.w3.org/2001/XMLSchema#decimal">0.22</cvss_v3_score>
    </owl:NamedIndividual>
    


    <!-- http://ontologies.ti-semantics.com/score#CVSSv3LowIntegrityImpact -->

    <owl:NamedIndividual rdf:about="http://ontologies.ti-semantics.com/score#CVSSv3LowIntegrityImpact">
        <rdf:type rdf:resource="http://ontologies.ti-semantics.com/score#CVSSv3LowIntegrityImpact"/>
        <greaterScoreThan rdf:resource="http://ontologies.ti-semantics.com/score#CVSSv3NoIntegrityImpact"/>
        <cvss_v3_score rdf:datatype="http://www.w3.org/2001/XMLSchema#decimal">0.22</cvss_v3_score>
    </owl:NamedIndividual>
    


    <!-- http://ontologies.ti-semantics.com/score#CVSSv3LowPrivilegesRequired -->

    <owl:NamedIndividual rdf:about="http://ontologies.ti-semantics.com/score#CVSSv3LowPrivilegesRequired">
        <rdf:type rdf:resource="http://ontologies.ti-semantics.com/score#CVSSv3LowPrivilegesRequired"/>
        <greaterScoreThan rdf:resource="http://ontologies.ti-semantics.com/score#CVSSv3HighPrivilegesRequired"/>
        <cvss_v3_score rdf:datatype="http://www.w3.org/2001/XMLSchema#decimal">0.62</cvss_v3_score>
    </owl:NamedIndividual>
    


    <!-- http://ontologies.ti-semantics.com/score#CVSSv3MediumAvailabilityRequirement -->

    <owl:NamedIndividual rdf:about="http://ontologies.ti-semantics.com/score#CVSSv3MediumAvailabilityRequirement">
        <rdf:type rdf:resource="http://ontologies.ti-semantics.com/score#CVSSv3MediumAvailabilityRequirement"/>
        <greaterScoreThan rdf:resource="http://ontologies.ti-semantics.com/score#CVSSv3LowAvailabilityRequirement"/>
        <cvss_v2_score rdf:datatype="http://www.w3.org/2001/XMLSchema#decimal">1</cvss_v2_score>
    </owl:NamedIndividual>
    


    <!-- http://ontologies.ti-semantics.com/score#CVSSv3NetworkAttackVector -->

    <owl:NamedIndividual rdf:about="http://ontologies.ti-semantics.com/score#CVSSv3NetworkAttackVector">
        <rdf:type rdf:resource="http://ontologies.ti-semantics.com/score#CVSSv3NetworkAttackVector"/>
        <greaterScoreThan rdf:resource="http://ontologies.ti-semantics.com/score#CVSSv3AdjacentAttackVector"/>
        <cvss_v3_score rdf:datatype="http://www.w3.org/2001/XMLSchema#decimal">0.85</cvss_v3_score>
    </owl:NamedIndividual>
    


    <!-- http://ontologies.ti-semantics.com/score#CVSSv3NoAvailabilityImpact -->

    <owl:NamedIndividual rdf:about="http://ontologies.ti-semantics.com/score#CVSSv3NoAvailabilityImpact">
        <rdf:type rdf:resource="http://ontologies.ti-semantics.com/score#CVSSv3NoAvailabilityImpact"/>
        <cvss_v2_score rdf:datatype="http://www.w3.org/2001/XMLSchema#decimal">0</cvss_v2_score>
        <cvss_v3_score rdf:datatype="http://www.w3.org/2001/XMLSchema#decimal">0</cvss_v3_score>
    </owl:NamedIndividual>
    


    <!-- http://ontologies.ti-semantics.com/score#CVSSv3NoConfidentialityImpact -->

    <owl:NamedIndividual rdf:about="http://ontologies.ti-semantics.com/score#CVSSv3NoConfidentialityImpact">
        <rdf:type rdf:resource="http://ontologies.ti-semantics.com/score#CVSSv3NoConfidentialityImpact"/>
        <cvss_v3_score rdf:datatype="http://www.w3.org/2001/XMLSchema#decimal">0</cvss_v3_score>
    </owl:NamedIndividual>
    


    <!-- http://ontologies.ti-semantics.com/score#CVSSv3NoIntegrityImpact -->

    <owl:NamedIndividual rdf:about="http://ontologies.ti-semantics.com/score#CVSSv3NoIntegrityImpact">
        <rdf:type rdf:resource="http://ontologies.ti-semantics.com/score#CVSSv3NoIntegrityImpact"/>
        <cvss_v2_score rdf:datatype="http://www.w3.org/2001/XMLSchema#decimal">0</cvss_v2_score>
        <cvss_v3_score rdf:datatype="http://www.w3.org/2001/XMLSchema#decimal">0</cvss_v3_score>
    </owl:NamedIndividual>
    


    <!-- http://ontologies.ti-semantics.com/score#CVSSv3NoPrivilegesRequired -->

    <owl:NamedIndividual rdf:about="http://ontologies.ti-semantics.com/score#CVSSv3NoPrivilegesRequired">
        <rdf:type rdf:resource="http://ontologies.ti-semantics.com/score#CVSSv3NoPrivilegesRequired"/>
        <greaterScoreThan rdf:resource="http://ontologies.ti-semantics.com/score#CVSSv3LowPrivilegesRequired"/>
        <cvss_v3_score rdf:datatype="http://www.w3.org/2001/XMLSchema#decimal">0.85</cvss_v3_score>
    </owl:NamedIndividual>
    


    <!-- http://ontologies.ti-semantics.com/score#CVSSv3NoUserInteraction -->

    <owl:NamedIndividual rdf:about="http://ontologies.ti-semantics.com/score#CVSSv3NoUserInteraction">
        <rdf:type rdf:resource="http://ontologies.ti-semantics.com/score#CVSSv3NoUserInteraction"/>
        <greaterScoreThan rdf:resource="http://ontologies.ti-semantics.com/score#CVSSv3RequiredUserInteraction"/>
        <cvss_v3_score rdf:datatype="http://www.w3.org/2001/XMLSchema#decimal">0.85</cvss_v3_score>
    </owl:NamedIndividual>
    


    <!-- http://ontologies.ti-semantics.com/score#CVSSv3NotDefinedAvailabilityRequirement -->

    <owl:NamedIndividual rdf:about="http://ontologies.ti-semantics.com/score#CVSSv3NotDefinedAvailabilityRequirement">
        <rdf:type rdf:resource="http://ontologies.ti-semantics.com/score#CVSSv3NotDefinedAvailabilityRequirement"/>
        <cvss_v2_score rdf:datatype="http://www.w3.org/2001/XMLSchema#decimal">1</cvss_v2_score>
    </owl:NamedIndividual>
    


    <!-- http://ontologies.ti-semantics.com/score#CVSSv3NotDefinedExploitCodeMaturity -->

    <owl:NamedIndividual rdf:about="http://ontologies.ti-semantics.com/score#CVSSv3NotDefinedExploitCodeMaturity">
        <rdf:type rdf:resource="http://ontologies.ti-semantics.com/score#CVSSv3NotDefinedExploitCodeMaturity"/>
        <cvss_v3_score rdf:datatype="http://www.w3.org/2001/XMLSchema#decimal">1</cvss_v3_score>
    </owl:NamedIndividual>
    


    <!-- http://ontologies.ti-semantics.com/score#CVSSv3NotDefinedRemediation -->

    <owl:NamedIndividual rdf:about="http://ontologies.ti-semantics.com/score#CVSSv3NotDefinedRemediation">
        <rdf:type rdf:resource="http://ontologies.ti-semantics.com/score#CVSSv3NotDefinedRemediation"/>
    </owl:NamedIndividual>
    


    <!-- http://ontologies.ti-semantics.com/score#CVSSv3NotDefinedReportConfidence -->

    <owl:NamedIndividual rdf:about="http://ontologies.ti-semantics.com/score#CVSSv3NotDefinedReportConfidence">
        <rdf:type rdf:resource="http://ontologies.ti-semantics.com/score#CVSSv3NotDefinedReportConfidence"/>
    </owl:NamedIndividual>
    


    <!-- http://ontologies.ti-semantics.com/score#CVSSv3OfficialFixRemediation -->

    <owl:NamedIndividual rdf:about="http://ontologies.ti-semantics.com/score#CVSSv3OfficialFixRemediation">
        <rdf:type rdf:resource="http://ontologies.ti-semantics.com/score#CVSSv3OfficialFixRemediation"/>
        <cvss_v3_score rdf:datatype="http://www.w3.org/2001/XMLSchema#decimal">0.95</cvss_v3_score>
    </owl:NamedIndividual>
    


    <!-- http://ontologies.ti-semantics.com/score#CVSSv3PhysicalAttackVector -->

    <owl:NamedIndividual rdf:about="http://ontologies.ti-semantics.com/score#CVSSv3PhysicalAttackVector">
        <rdf:type rdf:resource="http://ontologies.ti-semantics.com/score#CVSSv3PhysicalAttackVector"/>
        <cvss_v3_score rdf:datatype="http://www.w3.org/2001/XMLSchema#decimal">0.2</cvss_v3_score>
    </owl:NamedIndividual>
    


    <!-- http://ontologies.ti-semantics.com/score#CVSSv3ProofOfConceptExploitCodeMaturity -->

    <owl:NamedIndividual rdf:about="http://ontologies.ti-semantics.com/score#CVSSv3ProofOfConceptExploitCodeMaturity">
        <rdf:type rdf:resource="http://ontologies.ti-semantics.com/score#CVSSv3ProofOfConceptExploitCodeMaturity"/>
        <greaterScoreThan rdf:resource="http://ontologies.ti-semantics.com/score#CVSSv3UnprovenExploitCodeMaturity"/>
        <cvss_v3_score rdf:datatype="http://www.w3.org/2001/XMLSchema#decimal">0.94</cvss_v3_score>
    </owl:NamedIndividual>
    


    <!-- http://ontologies.ti-semantics.com/score#CVSSv3ReasonableReportConfidence -->

    <owl:NamedIndividual rdf:about="http://ontologies.ti-semantics.com/score#CVSSv3ReasonableReportConfidence">
        <rdf:type rdf:resource="http://ontologies.ti-semantics.com/score#CVSSv3ReasonableReportConfidence"/>
        <greaterScoreThan rdf:resource="http://ontologies.ti-semantics.com/score#CVSSv3UnknownReportConfidence"/>
        <cvss_v3_score rdf:datatype="http://www.w3.org/2001/XMLSchema#decimal">0.96</cvss_v3_score>
    </owl:NamedIndividual>
    


    <!-- http://ontologies.ti-semantics.com/score#CVSSv3RequiredUserInteraction -->

    <owl:NamedIndividual rdf:about="http://ontologies.ti-semantics.com/score#CVSSv3RequiredUserInteraction">
        <rdf:type rdf:resource="http://ontologies.ti-semantics.com/score#CVSSv3RequiredUserInteraction"/>
        <cvss_v2_score rdf:datatype="http://www.w3.org/2001/XMLSchema#decimal">0.62</cvss_v2_score>
        <cvss_v3_score rdf:datatype="http://www.w3.org/2001/XMLSchema#decimal">0.62</cvss_v3_score>
    </owl:NamedIndividual>
    


    <!-- http://ontologies.ti-semantics.com/score#CVSSv3TemporaryFixRemediation -->

    <owl:NamedIndividual rdf:about="http://ontologies.ti-semantics.com/score#CVSSv3TemporaryFixRemediation">
        <rdf:type rdf:resource="http://ontologies.ti-semantics.com/score#CVSSv3TemporaryFixRemediation"/>
        <greaterScoreThan rdf:resource="http://ontologies.ti-semantics.com/score#CVSSv3OfficialFixRemediation"/>
        <cvss_v3_score rdf:datatype="http://www.w3.org/2001/XMLSchema#decimal">0.96</cvss_v3_score>
    </owl:NamedIndividual>
    


    <!-- http://ontologies.ti-semantics.com/score#CVSSv3UnavailableRemediation -->

    <owl:NamedIndividual rdf:about="http://ontologies.ti-semantics.com/score#CVSSv3UnavailableRemediation">
        <rdf:type rdf:resource="http://ontologies.ti-semantics.com/score#CVSSv3RemediationLevel"/>
        <rdf:type rdf:resource="http://ontologies.ti-semantics.com/score#CVSSv3UnavailableRemediation"/>
        <greaterScoreThan rdf:resource="http://ontologies.ti-semantics.com/score#CVSSv3WorkaroundRemediation"/>
        <cvss_v3_score rdf:datatype="http://www.w3.org/2001/XMLSchema#decimal">1</cvss_v3_score>
    </owl:NamedIndividual>
    


    <!-- http://ontologies.ti-semantics.com/score#CVSSv3UnchangedScope -->

    <owl:NamedIndividual rdf:about="http://ontologies.ti-semantics.com/score#CVSSv3UnchangedScope">
        <rdf:type rdf:resource="http://ontologies.ti-semantics.com/score#CVSSv3UnchangedScope"/>
        <greaterScoreThan rdf:resource="http://ontologies.ti-semantics.com/score#CVSSv3ChangedScope"/>
    </owl:NamedIndividual>
    


    <!-- http://ontologies.ti-semantics.com/score#CVSSv3UnknownReportConfidence -->

    <owl:NamedIndividual rdf:about="http://ontologies.ti-semantics.com/score#CVSSv3UnknownReportConfidence">
        <rdf:type rdf:resource="http://ontologies.ti-semantics.com/score#CVSSv3UnknownReportConfidence"/>
        <cvss_v3_score rdf:datatype="http://www.w3.org/2001/XMLSchema#decimal">0.92</cvss_v3_score>
    </owl:NamedIndividual>
    


    <!-- http://ontologies.ti-semantics.com/score#CVSSv3UnprovenExploitCodeMaturity -->

    <owl:NamedIndividual rdf:about="http://ontologies.ti-semantics.com/score#CVSSv3UnprovenExploitCodeMaturity">
        <rdf:type rdf:resource="http://ontologies.ti-semantics.com/score#CVSSv3UnprovenExploitCodeMaturity"/>
        <cvss_v3_score rdf:datatype="http://www.w3.org/2001/XMLSchema#decimal">0.91</cvss_v3_score>
    </owl:NamedIndividual>
    


    <!-- http://ontologies.ti-semantics.com/score#CVSSv3WorkaroundRemediation -->

    <owl:NamedIndividual rdf:about="http://ontologies.ti-semantics.com/score#CVSSv3WorkaroundRemediation">
        <rdf:type rdf:resource="http://ontologies.ti-semantics.com/score#CVSSv3WorkaroundRemediation"/>
        <greaterScoreThan rdf:resource="http://ontologies.ti-semantics.com/score#CVSSv3TemporaryFixRemediation"/>
        <cvss_v3_score rdf:datatype="http://www.w3.org/2001/XMLSchema#decimal">0.97</cvss_v3_score>
    </owl:NamedIndividual>
    


    <!-- 
    ///////////////////////////////////////////////////////////////////////////////////////
    //
    // Annotations
    //
    ///////////////////////////////////////////////////////////////////////////////////////
     -->

    <rdf:Description rdf:about="http://ontologies.ti-semantics.com/score#CVSSv2AdjacentAccessVector">
        <rdfs:label xml:lang="en">Adjacent</rdfs:label>
        <rdfs:comment xml:lang="en">A vulnerability exploitable with adjacent network access requires the attacker to have access to either the broadcast or collision domain of the vulnerable software.  Examples of local networks include local IP subnet, Bluetooth, IEEE 802.11, and local Ethernet segment.</rdfs:comment>
        <rdfs:isDefinedBy rdf:datatype="http://www.w3.org/2001/XMLSchema#anyURI">https://www.first.org/cvss/v2/guide</rdfs:isDefinedBy>
        <cvss_v2_code>A</cvss_v2_code>
    </rdf:Description>
    <rdf:Description rdf:about="http://ontologies.ti-semantics.com/score#CVSSv2CompleteAvailabilityImpact">
        <cvss_v2_code>C</cvss_v2_code>
        <rdfs:label xml:lang="en">Complete</rdfs:label>
        <rdfs:isDefinedBy rdf:datatype="http://www.w3.org/2001/XMLSchema#anyURI">https://www.first.org/cvss/v2/guide</rdfs:isDefinedBy>
        <rdfs:comment xml:lang="en">There is a total shutdown of the affected resource. The attacker can render the resource completely unavailable.</rdfs:comment>
    </rdf:Description>
    <rdf:Description rdf:about="http://ontologies.ti-semantics.com/score#CVSSv2CompleteConfidentialityImpact">
        <rdfs:isDefinedBy rdf:datatype="http://www.w3.org/2001/XMLSchema#anyURI">https://www.first.org/cvss/v2/guide#2-1-4-Confidentiality-Impact-C</rdfs:isDefinedBy>
        <rdfs:label xml:lang="en">Complete</rdfs:label>
        <cvss_v2_code>C</cvss_v2_code>
        <rdfs:comment xml:lang="en">There is total information disclosure, resulting in all system files being revealed. The attacker is able to read all of the system&apos;s data (memory, files, etc.)</rdfs:comment>
    </rdf:Description>
    <rdf:Description rdf:about="http://ontologies.ti-semantics.com/score#CVSSv2CompleteIntegrityImpact">
        <cvss_v2_code>C</cvss_v2_code>
        <rdfs:label xml:lang="en">Complete</rdfs:label>
        <rdfs:isDefinedBy rdf:datatype="http://www.w3.org/2001/XMLSchema#anyURI">https://www.first.org/cvss/v2/guide#2-1-5-Integrity-Impact-I</rdfs:isDefinedBy>
        <rdfs:comment xml:lang="en">There is a total compromise of system integrity. There is a complete loss of system protection, resulting in the entire system being compromised. The attacker is able to modify any files on the target system.</rdfs:comment>
    </rdf:Description>
    <rdf:Description rdf:about="http://ontologies.ti-semantics.com/score#CVSSv2ConfirmedReportConfidence">
        <rdfs:label xml:lang="en">Confirmed</rdfs:label>
        <rdfs:comment xml:lang="en">The vulnerability has been acknowledged by the vendor or author of the affected technology. The vulnerability may also be Confirmed when its existence is confirmed from an external event such as publication of functional or proof-of-concept exploit code or widespread exploitation.</rdfs:comment>
        <rdfs:isDefinedBy rdf:datatype="http://www.w3.org/2001/XMLSchema#anyURI">https://www.first.org/cvss/v2/guide#2-2-3-Report-Confidence-RC</rdfs:isDefinedBy>
        <cvss_v2_code>C</cvss_v2_code>
    </rdf:Description>
    <rdf:Description rdf:about="http://ontologies.ti-semantics.com/score#CVSSv2FunctionalExploitability">
        <rdfs:isDefinedBy rdf:datatype="http://www.w3.org/2001/XMLSchema#anyURI">https://www.first.org/cvss/v2/guide#2-2-1-Exploitability-E</rdfs:isDefinedBy>
        <rdfs:label xml:lang="en">Functional</rdfs:label>
        <rdfs:comment xml:lang="en">Functional exploit code is available. The code works in most situations where the vulnerability exists.</rdfs:comment>
        <cvss_v2_code>F</cvss_v2_code>
    </rdf:Description>
    <rdf:Description rdf:about="http://ontologies.ti-semantics.com/score#CVSSv2HighAccessComplexity">
        <rdfs:label xml:lang="en">High</rdfs:label>
        <cvss_v2_code xml:lang="en">H</cvss_v2_code>
        <rdfs:comment xml:lang="en">Specialized access conditions exist. For example:
- In most configurations, the attacking party must already have elevated privileges or spoof additional systems in addition to the attacking system (e.g., DNS hijacking).
- The attack depends on social engineering methods that would be easily detected by knowledgeable people. For example, the victim must perform several suspicious or atypical actions.
- The vulnerable configuration is seen very rarely in practice.
- If a race condition exists, the window is very narrow.</rdfs:comment>
        <rdfs:isDefinedBy xml:lang="en">https://www.first.org/cvss/v2/guide#2-1-2-Access-Complexity-AC</rdfs:isDefinedBy>
    </rdf:Description>
    <rdf:Description rdf:about="http://ontologies.ti-semantics.com/score#CVSSv2HighAvailabilityRequirement">
        <rdfs:comment xml:lang="en">Loss of Availability is likely to have a catastrophic adverse effect on the organization or individuals associated with the organization (e.g., employees, customers).</rdfs:comment>
        <cvss_v2_code xml:lang="en">H</cvss_v2_code>
        <rdfs:isDefinedBy xml:lang="en">https://www.first.org/cvss/v2/guide#2-3-3-Security-Requirements-CR-IR-AR</rdfs:isDefinedBy>
    </rdf:Description>
    <rdf:Description rdf:about="http://ontologies.ti-semantics.com/score#CVSSv2HighCollateralDamagePotential">
        <rdfs:comment xml:lang="en">A successful exploit of this vulnerability may result in catastrophic physical or property damage and loss. Or, there may be a catastrophic loss of revenue or productivity.</rdfs:comment>
        <rdfs:isDefinedBy rdf:datatype="http://www.w3.org/2001/XMLSchema#anyURI">https://www.first.org/cvss/v2/guide#2-3-1-Collateral-Damage-Potential-CDP</rdfs:isDefinedBy>
        <cvss_v2_code>H</cvss_v2_code>
        <rdfs:label xml:lang="en">High</rdfs:label>
    </rdf:Description>
    <rdf:Description rdf:about="http://ontologies.ti-semantics.com/score#CVSSv2HighConfidentialityRequirement">
        <cvss_v2_code xml:lang="en">H</cvss_v2_code>
        <rdfs:comment xml:lang="en">Loss of Confidentiality is likely to have a catastrophic adverse effect on the organization or individuals associated with the organization (e.g., employees, customers).</rdfs:comment>
        <rdfs:isDefinedBy xml:lang="en">https://www.first.org/cvss/v2/guide#2-3-3-Security-Requirements-CR-IR-AR</rdfs:isDefinedBy>
    </rdf:Description>
    <rdf:Description rdf:about="http://ontologies.ti-semantics.com/score#CVSSv2HighExploitability">
        <rdfs:isDefinedBy rdf:datatype="http://www.w3.org/2001/XMLSchema#anyURI">https://www.first.org/cvss/v2/guide#2-2-1-Exploitability-E</rdfs:isDefinedBy>
        <rdfs:comment xml:lang="en">Either the vulnerability is exploitable by functional mobile autonomous code, or no exploit is required (manual trigger) and details are widely available. The code works in every situation, or is actively being delivered via a mobile autonomous agent (such as a worm or virus).</rdfs:comment>
        <cvss_v2_code>H</cvss_v2_code>
        <rdfs:label xml:lang="en">High</rdfs:label>
    </rdf:Description>
    <rdf:Description rdf:about="http://ontologies.ti-semantics.com/score#CVSSv2HighIntegrityRequirement">
        <cvss_v2_code xml:lang="en">H</cvss_v2_code>
        <rdfs:comment xml:lang="en">Loss of Integrity is likely to have a catastrophic adverse effect on the organization or individuals associated with the organization (e.g., employees, customers).</rdfs:comment>
        <rdfs:isDefinedBy xml:lang="en">https://www.first.org/cvss/v2/guide#2-3-3-Security-Requirements-CR-IR-AR</rdfs:isDefinedBy>
    </rdf:Description>
    <rdf:Description rdf:about="http://ontologies.ti-semantics.com/score#CVSSv2HighTargetCount">
        <cvss_v2_code>H</cvss_v2_code>
        <rdfs:label xml:lang="en">High</rdfs:label>
        <rdfs:comment xml:lang="en">Targets exist inside the environment on a considerable scale. Between 76% - 100% of the total environment is considered at risk.</rdfs:comment>
        <rdfs:isDefinedBy rdf:datatype="http://www.w3.org/2001/XMLSchema#anyURI">https://www.first.org/cvss/v2/guide#2-3-2-Target-Distribution-TD</rdfs:isDefinedBy>
    </rdf:Description>
    <rdf:Description rdf:about="http://ontologies.ti-semantics.com/score#CVSSv2LocalAccessVector">
        <cvss_v2_code>L</cvss_v2_code>
        <rdfs:comment xml:lang="en">A vulnerability exploitable with only local access requires the attacker to have either physical access to the vulnerable system or a local (shell) account. Examples of locally exploitable vulnerabilities are peripheral attacks such as Firewire/USB DMA attacks, and local privilege escalations (e.g., sudo).</rdfs:comment>
        <rdfs:isDefinedBy rdf:datatype="http://www.w3.org/2001/XMLSchema#anyURI">https://www.first.org/cvss/v2/guide</rdfs:isDefinedBy>
        <rdfs:label xml:lang="en">Local</rdfs:label>
    </rdf:Description>
    <rdf:Description rdf:about="http://ontologies.ti-semantics.com/score#CVSSv2LowAccessComplexity">
        <rdfs:isDefinedBy xml:lang="en">https://www.first.org/cvss/v2/guide#2-1-2-Access-Complexity-AC</rdfs:isDefinedBy>
        <rdfs:comment xml:lang="en">Specialized access conditions or extenuating circumstances do not exist. The following are examples:
- The affected product typically requires access to a wide range of systems and users, possibly anonymous and untrusted (e.g., Internet-facing web or mail server).
- The affected configuration is default or ubiquitous.
- The attack can be performed manually and requires little skill or additional information gathering.
- The race condition is a lazy one (i.e., it is technically a race but easily winnable).</rdfs:comment>
        <rdfs:label xml:lang="en">Low</rdfs:label>
        <cvss_v2_code>L</cvss_v2_code>
    </rdf:Description>
    <rdf:Description rdf:about="http://ontologies.ti-semantics.com/score#CVSSv2LowAvailabilityRequirement">
        <rdfs:isDefinedBy xml:lang="en">https://www.first.org/cvss/v2/guide#2-3-3-Security-Requirements-CR-IR-AR</rdfs:isDefinedBy>
        <cvss_v2_code xml:lang="en">L</cvss_v2_code>
        <rdfs:comment xml:lang="en">Loss of Availability is likely to have only a limited adverse effect on the organization or individuals associated with the organization (e.g., employees, customers).</rdfs:comment>
    </rdf:Description>
    <rdf:Description rdf:about="http://ontologies.ti-semantics.com/score#CVSSv2LowCollateralDamagePotential">
        <cvss_v2_code>L</cvss_v2_code>
        <rdfs:comment xml:lang="en">A successful exploit of this vulnerability may result in slight physical or property damage. Or, there may be a slight loss of revenue or productivity to the organization.</rdfs:comment>
        <rdfs:label xml:lang="en">Low</rdfs:label>
        <rdfs:isDefinedBy rdf:datatype="http://www.w3.org/2001/XMLSchema#anyURI">https://www.first.org/cvss/v2/guide#2-3-1-Collateral-Damage-Potential-CDP</rdfs:isDefinedBy>
    </rdf:Description>
    <rdf:Description rdf:about="http://ontologies.ti-semantics.com/score#CVSSv2LowConfidentialityRequirement">
        <cvss_v2_code xml:lang="en">L</cvss_v2_code>
        <rdfs:isDefinedBy xml:lang="en">https://www.first.org/cvss/v2/guide#2-3-3-Security-Requirements-CR-IR-AR</rdfs:isDefinedBy>
        <rdfs:comment xml:lang="en">Loss of Confidentiality is likely to have only a limited adverse effect on the organization or individuals associated with the organization (e.g., employees, customers).</rdfs:comment>
    </rdf:Description>
    <rdf:Description rdf:about="http://ontologies.ti-semantics.com/score#CVSSv2LowIntegrityRequirement">
        <rdfs:comment xml:lang="en">Loss of Integrity is likely to have only a limited adverse effect on the organization or individuals associated with the organization (e.g., employees, customers).</rdfs:comment>
        <cvss_v2_code xml:lang="en">L</cvss_v2_code>
        <rdfs:isDefinedBy xml:lang="en">https://www.first.org/cvss/v2/guide#2-3-3-Security-Requirements-CR-IR-AR</rdfs:isDefinedBy>
    </rdf:Description>
    <rdf:Description rdf:about="http://ontologies.ti-semantics.com/score#CVSSv2LowMediumCollateralDamagePotential">
        <cvss_v2_code>LM</cvss_v2_code>
        <rdfs:label xml:lang="en">Low-Medium</rdfs:label>
        <rdfs:comment xml:lang="en">A successful exploit of this vulnerability may result in moderate physical or property damage. Or, there may be a moderate loss of revenue or productivity to the organization.</rdfs:comment>
        <rdfs:isDefinedBy rdf:datatype="http://www.w3.org/2001/XMLSchema#anyURI">https://www.first.org/cvss/v2/guide#2-3-1-Collateral-Damage-Potential-CDP</rdfs:isDefinedBy>
    </rdf:Description>
    <rdf:Description rdf:about="http://ontologies.ti-semantics.com/score#CVSSv2LowTargetCount">
        <rdfs:isDefinedBy rdf:datatype="http://www.w3.org/2001/XMLSchema#anyURI">https://www.first.org/cvss/v2/guide#2-3-2-Target-Distribution-TD</rdfs:isDefinedBy>
        <rdfs:label xml:lang="en">Low</rdfs:label>
        <cvss_v2_code>L</cvss_v2_code>
        <rdfs:comment xml:lang="en">Targets exist inside the environment, but on a small scale. Between 1% - 25% of the total environment is at risk.</rdfs:comment>
    </rdf:Description>
    <rdf:Description rdf:about="http://ontologies.ti-semantics.com/score#CVSSv2MediumAvailabilityRequirement">
        <cvss_v2_code xml:lang="en">M</cvss_v2_code>
        <rdfs:isDefinedBy xml:lang="en">https://www.first.org/cvss/v2/guide#2-3-3-Security-Requirements-CR-IR-AR</rdfs:isDefinedBy>
        <rdfs:comment xml:lang="en">Loss of Availability is likely to have a serious adverse effect on the organization or individuals associated with the organization (e.g., employees, customers).</rdfs:comment>
    </rdf:Description>
    <rdf:Description rdf:about="http://ontologies.ti-semantics.com/score#CVSSv2MediumConfidentialityRequirement">
        <cvss_v2_code xml:lang="en">M</cvss_v2_code>
        <rdfs:isDefinedBy xml:lang="en">https://www.first.org/cvss/v2/guide#2-3-3-Security-Requirements-CR-IR-AR</rdfs:isDefinedBy>
        <rdfs:comment xml:lang="en">Loss of Confidentiality is likely to have a serious adverse effect on the organization or individuals associated with the organization (e.g., employees, customers).</rdfs:comment>
    </rdf:Description>
    <rdf:Description rdf:about="http://ontologies.ti-semantics.com/score#CVSSv2MediumHighCollateralDamagePotential">
        <cvss_v2_code>MH</cvss_v2_code>
        <rdfs:comment xml:lang="en">A successful exploit of this vulnerability may result in significant physical or property damage or loss. Or, there may be a significant loss of revenue or productivity.</rdfs:comment>
        <rdfs:isDefinedBy rdf:datatype="http://www.w3.org/2001/XMLSchema#anyURI">https://www.first.org/cvss/v2/guide#2-3-1-Collateral-Damage-Potential-CDP</rdfs:isDefinedBy>
        <rdfs:label xml:lang="en">Medium-High</rdfs:label>
    </rdf:Description>
    <rdf:Description rdf:about="http://ontologies.ti-semantics.com/score#CVSSv2MediumIntegrityRequirement">
        <cvss_v2_code xml:lang="en">M</cvss_v2_code>
        <rdfs:comment xml:lang="en">Loss of Integrity is likely to have a serious adverse effect on the organization or individuals associated with the organization (e.g., employees, customers).</rdfs:comment>
        <rdfs:isDefinedBy xml:lang="en">https://www.first.org/cvss/v2/guide#2-3-3-Security-Requirements-CR-IR-AR</rdfs:isDefinedBy>
    </rdf:Description>
    <rdf:Description rdf:about="http://ontologies.ti-semantics.com/score#CVSSv2MediumTargetCount">
        <rdfs:isDefinedBy rdf:datatype="http://www.w3.org/2001/XMLSchema#anyURI">https://www.first.org/cvss/v2/guide#2-3-2-Target-Distribution-TD</rdfs:isDefinedBy>
        <rdfs:label xml:lang="en">Medium</rdfs:label>
        <rdfs:comment xml:lang="en">Targets exist inside the environment, but on a medium scale. Between 26% - 75% of the total environment is at risk.</rdfs:comment>
        <cvss_v2_code>M</cvss_v2_code>
    </rdf:Description>
    <rdf:Description rdf:about="http://ontologies.ti-semantics.com/score#CVSSv2MultipleAuthentications">
        <cvss_v2_code>M</cvss_v2_code>
        <rdfs:label xml:lang="en">Multiple</rdfs:label>
        <rdfs:isDefinedBy rdf:datatype="http://www.w3.org/2001/XMLSchema#anyURI">https://www.first.org/cvss/v2/guide#2-1-3-Authentication-Au</rdfs:isDefinedBy>
        <rdfs:comment xml:lang="en">Exploiting the vulnerability requires that the attacker authenticate two or more times, even if the same credentials are used each time. An example is an attacker authenticating to an operating system in addition to providing credentials to access an application hosted on that system.</rdfs:comment>
    </rdf:Description>
    <rdf:Description rdf:about="http://ontologies.ti-semantics.com/score#CVSSv2NetworkAccessVector">
        <rdfs:comment xml:lang="en">A vulnerability exploitable with network access means the vulnerable software is bound to the network stack and the attacker does not require local network access or local access. Such a vulnerability is often termed &quot;remotely exploitable&quot;. An example of a network attack is an RPC buffer overflow.</rdfs:comment>
        <cvss_v2_code>N</cvss_v2_code>
        <rdfs:label xml:lang="en">Network</rdfs:label>
        <rdfs:isDefinedBy rdf:datatype="http://www.w3.org/2001/XMLSchema#anyURI">https://www.first.org/cvss/v2/guide</rdfs:isDefinedBy>
    </rdf:Description>
    <rdf:Description rdf:about="http://ontologies.ti-semantics.com/score#CVSSv2NilTargetCount">
        <cvss_v2_code>N</cvss_v2_code>
        <rdfs:isDefinedBy rdf:datatype="http://www.w3.org/2001/XMLSchema#anyURI">https://www.first.org/cvss/v2/guide#2-3-2-Target-Distribution-TD</rdfs:isDefinedBy>
        <rdfs:comment xml:lang="en">No target systems exist, or targets are so highly specialized that they only exist in a laboratory setting. Effectively 0% of the environment is at risk.</rdfs:comment>
        <rdfs:label xml:lang="en">None</rdfs:label>
    </rdf:Description>
    <rdf:Description rdf:about="http://ontologies.ti-semantics.com/score#CVSSv2NoAuthentication">
        <rdfs:isDefinedBy rdf:datatype="http://www.w3.org/2001/XMLSchema#anyURI">https://www.first.org/cvss/v2/guide#2-1-3-Authentication-Au</rdfs:isDefinedBy>
        <rdfs:comment xml:lang="en">Authentication is not required to exploit the vulnerability.</rdfs:comment>
        <rdfs:comment xml:lang="en">None</rdfs:comment>
        <cvss_v2_code>N</cvss_v2_code>
    </rdf:Description>
    <rdf:Description rdf:about="http://ontologies.ti-semantics.com/score#CVSSv2NoAvailabilityImpact">
        <rdfs:comment xml:lang="en">There is no impact to the availability of the system.</rdfs:comment>
        <rdfs:label xml:lang="en">None</rdfs:label>
        <cvss_v2_code>N</cvss_v2_code>
        <rdfs:isDefinedBy rdf:datatype="http://www.w3.org/2001/XMLSchema#anyURI">https://www.first.org/cvss/v2/guide</rdfs:isDefinedBy>
    </rdf:Description>
    <rdf:Description rdf:about="http://ontologies.ti-semantics.com/score#CVSSv2NoCollateralDamagePotential">
        <rdfs:isDefinedBy rdf:datatype="http://www.w3.org/2001/XMLSchema#anyURI">https://www.first.org/cvss/v2/guide#2-3-1-Collateral-Damage-Potential-CDP</rdfs:isDefinedBy>
        <rdfs:label xml:lang="en">None</rdfs:label>
        <cvss_v2_code>N</cvss_v2_code>
        <rdfs:comment xml:lang="en">There is no potential for loss of life, physical assets, productivity or revenue.</rdfs:comment>
    </rdf:Description>
    <rdf:Description rdf:about="http://ontologies.ti-semantics.com/score#CVSSv2NoConfidentialityImpact">
        <cvss_v2_code xml:lang="en">N</cvss_v2_code>
        <rdfs:isDefinedBy rdf:datatype="http://www.w3.org/2001/XMLSchema#anyURI">https://www.first.org/cvss/v2/guide#2-1-4-Confidentiality-Impact-C</rdfs:isDefinedBy>
        <rdfs:comment xml:lang="en">There is no impact to the confidentiality of the system.</rdfs:comment>
        <rdfs:label xml:lang="en">None</rdfs:label>
    </rdf:Description>
    <rdf:Description rdf:about="http://ontologies.ti-semantics.com/score#CVSSv2NoIntegrityImpact">
        <rdfs:label xml:lang="en">None</rdfs:label>
        <rdfs:isDefinedBy rdf:datatype="http://www.w3.org/2001/XMLSchema#anyURI">https://www.first.org/cvss/v2/guide#2-1-5-Integrity-Impact-I</rdfs:isDefinedBy>
        <cvss_v3_code xml:lang="en">N</cvss_v3_code>
        <rdfs:comment xml:lang="en">There is no impact to the integrity of the system.</rdfs:comment>
    </rdf:Description>
    <owl:Axiom>
        <owl:annotatedSource rdf:resource="http://ontologies.ti-semantics.com/score#CVSSv2NoIntegrityImpact"/>
        <owl:annotatedProperty rdf:resource="http://www.w3.org/2000/01/rdf-schema#comment"/>
        <owl:annotatedTarget xml:lang="en">There is no impact to the integrity of the system.</owl:annotatedTarget>
        <rdfs:isDefinedBy rdf:datatype="http://www.w3.org/2001/XMLSchema#anyURI">https://www.first.org/cvss/v2/guide#2-1-5-Integrity-Impact-I</rdfs:isDefinedBy>
    </owl:Axiom>
    <rdf:Description rdf:about="http://ontologies.ti-semantics.com/score#CVSSv2NotDefinedAvailabilityRequirement">
        <rdfs:comment xml:lang="en">Assigning this value to the metric will not influence the score. It is a signal to the equation to skip this metric.</rdfs:comment>
        <cvss_v2_code xml:lang="en">ND</cvss_v2_code>
        <rdfs:isDefinedBy xml:lang="en">https://www.first.org/cvss/v2/guide#2-3-3-Security-Requirements-CR-IR-AR</rdfs:isDefinedBy>
    </rdf:Description>
    <rdf:Description rdf:about="http://ontologies.ti-semantics.com/score#CVSSv2NotDefinedCollateralDamagePotential">
        <rdfs:comment xml:lang="en">Assigning this value to the metric will not influence the score. It is a signal to the equation to skip this metric.</rdfs:comment>
        <cvss_v2_code>ND</cvss_v2_code>
        <rdfs:isDefinedBy rdf:datatype="http://www.w3.org/2001/XMLSchema#anyURI">https://www.first.org/cvss/v2/guide#2-3-1-Collateral-Damage-Potential-CDP</rdfs:isDefinedBy>
        <rdfs:label xml:lang="en">Not Defined</rdfs:label>
    </rdf:Description>
    <rdf:Description rdf:about="http://ontologies.ti-semantics.com/score#CVSSv2NotDefinedConfidentialityRequirement">
        <rdfs:isDefinedBy xml:lang="en">https://www.first.org/cvss/v2/guide#2-3-3-Security-Requirements-CR-IR-AR</rdfs:isDefinedBy>
        <cvss_v2_code xml:lang="en">ND</cvss_v2_code>
        <rdfs:comment xml:lang="en">Assigning this value to the metric will not influence the score. It is a signal to the equation to skip this metric.</rdfs:comment>
    </rdf:Description>
    <rdf:Description rdf:about="http://ontologies.ti-semantics.com/score#CVSSv2NotDefinedExploitability">
        <cvss_v2_code>ND</cvss_v2_code>
        <rdfs:comment xml:lang="en">Assigning this value to the metric will not influence the score. It is a signal to the equation to skip this metric.</rdfs:comment>
        <rdfs:comment xml:lang="en">Not Defined</rdfs:comment>
        <rdfs:isDefinedBy rdf:datatype="http://www.w3.org/2001/XMLSchema#anyURI">https://www.first.org/cvss/v2/guide#2-2-1-Exploitability-E</rdfs:isDefinedBy>
    </rdf:Description>
    <rdf:Description rdf:about="http://ontologies.ti-semantics.com/score#CVSSv2NotDefinedIntegrityRequirement">
        <rdfs:comment xml:lang="en">Assigning this value to the metric will not influence the score. It is a signal to the equation to skip this metric.</rdfs:comment>
        <cvss_v2_code xml:lang="en">ND</cvss_v2_code>
        <rdfs:isDefinedBy xml:lang="en">https://www.first.org/cvss/v2/guide#2-3-3-Security-Requirements-CR-IR-AR</rdfs:isDefinedBy>
    </rdf:Description>
    <rdf:Description rdf:about="http://ontologies.ti-semantics.com/score#CVSSv2NotDefinedRemediation">
        <rdfs:isDefinedBy xml:lang="en">https://www.first.org/cvss/v2/guide#2-2-2-Remediation-Level-RL</rdfs:isDefinedBy>
        <rdfs:comment xml:lang="en">Assigning this value to the metric will not influence the score. It is a signal to a scoring equation to skip this metric.</rdfs:comment>
        <rdfs:label xml:lang="en">Not Defined</rdfs:label>
        <cvss_v2_code>X</cvss_v2_code>
    </rdf:Description>
    <rdf:Description rdf:about="http://ontologies.ti-semantics.com/score#CVSSv2NotDefinedTargetCount">
        <rdfs:isDefinedBy rdf:datatype="http://www.w3.org/2001/XMLSchema#anyURI">https://www.first.org/cvss/v2/guide#2-3-2-Target-Distribution-TD</rdfs:isDefinedBy>
        <rdfs:label xml:lang="en">Not Defined</rdfs:label>
        <cvss_v2_code>ND</cvss_v2_code>
        <rdfs:comment xml:lang="en">Assigning this value to the metric will not influence the score. It is a signal to the equation to skip this metric.</rdfs:comment>
    </rdf:Description>
    <rdf:Description rdf:about="http://ontologies.ti-semantics.com/score#CVSSv2OfficialFixRemediation">
        <rdfs:label xml:lang="en">Official Fix</rdfs:label>
        <rdfs:comment xml:lang="en">A complete vendor solution is available. Either the vendor has issued an official patch, or an upgrade is available.</rdfs:comment>
        <rdfs:isDefinedBy xml:lang="en">https://www.first.org/cvss/v2/guide#2-2-2-Remediation-Level-RL</rdfs:isDefinedBy>
        <cvss_v2_code>O</cvss_v2_code>
    </rdf:Description>
    <rdf:Description rdf:about="http://ontologies.ti-semantics.com/score#CVSSv2PartialAvailabilityImpact">
        <rdfs:comment xml:lang="en">There is reduced performance or interruptions in resource availability. An example is a network-based flood attack that permits a limited number of successful connections to an Internet service.</rdfs:comment>
        <cvss_v2_code>P</cvss_v2_code>
        <rdfs:isDefinedBy rdf:datatype="http://www.w3.org/2001/XMLSchema#anyURI">https://www.first.org/cvss/v2/guide</rdfs:isDefinedBy>
        <rdfs:label xml:lang="en">Partial</rdfs:label>
    </rdf:Description>
    <rdf:Description rdf:about="http://ontologies.ti-semantics.com/score#CVSSv2PartialConfidentialityImpact">
        <rdfs:isDefinedBy xml:lang="en">https://www.first.org/cvss/v2/guide#2-1-4-Confidentiality-Impact-C</rdfs:isDefinedBy>
        <rdfs:comment xml:lang="en">There is considerable informational disclosure. Access to some system files is possible, but the attacker does not have control over what is obtained, or the scope of the loss is constrained. An example is a vulnerability that divulges only certain tables in a database.</rdfs:comment>
    </rdf:Description>
    <rdf:Description rdf:about="http://ontologies.ti-semantics.com/score#CVSSv2PartialIntegrityImpact">
        <rdfs:comment xml:lang="en">Modification of some system files or information is possible, but the attacker does not have control over what can be modified, or the scope of what the attacker can affect is limited. For example, system or application files may be overwritten or modified, but either the attacker has no control over which files are affected or the attacker can modify files within only a limited context or scope.</rdfs:comment>
        <rdfs:label xml:lang="en">Partial</rdfs:label>
        <cvss_v2_code>P</cvss_v2_code>
        <rdfs:isDefinedBy rdf:datatype="http://www.w3.org/2001/XMLSchema#anyURI">https://www.first.org/cvss/v2/guide#2-1-5-Integrity-Impact-I</rdfs:isDefinedBy>
    </rdf:Description>
    <rdf:Description rdf:about="http://ontologies.ti-semantics.com/score#CVSSv2ProofOfConceptExploitability">
        <rdfs:comment xml:lang="en">Proof-of-concept exploit code or an attack demonstration that is not practical for most systems is available. The code or technique is not functional in all situations and may require substantial modification by a skilled attacker.</rdfs:comment>
        <rdfs:label xml:lang="en">Proof-of-Concept</rdfs:label>
        <cvss_v2_code>POC</cvss_v2_code>
        <rdfs:isDefinedBy rdf:datatype="http://www.w3.org/2001/XMLSchema#anyURI">https://www.first.org/cvss/v2/guide#2-2-1-Exploitability-E</rdfs:isDefinedBy>
    </rdf:Description>
    <rdf:Description rdf:about="http://ontologies.ti-semantics.com/score#CVSSv2SingleAuthentication">
        <rdfs:comment xml:lang="en">The vulnerability requires an attacker to be logged into the system (such as at a command line or via a desktop session or web interface).</rdfs:comment>
        <rdfs:label xml:lang="en">Single</rdfs:label>
        <rdfs:isDefinedBy rdf:datatype="http://www.w3.org/2001/XMLSchema#anyURI">https://www.first.org/cvss/v2/guide#2-1-3-Authentication-Au</rdfs:isDefinedBy>
        <cvss_v2_code>S</cvss_v2_code>
    </rdf:Description>
    <rdf:Description rdf:about="http://ontologies.ti-semantics.com/score#CVSSv2TemporaryFixRemediation">
        <cvss_v2_code>T</cvss_v2_code>
        <rdfs:comment xml:lang="en">There is an official but temporary fix available. This includes instances where the vendor issues a temporary hotfix, tool, or workaround.</rdfs:comment>
        <rdfs:label xml:lang="en">Temporary Fix</rdfs:label>
        <rdfs:isDefinedBy xml:lang="en">https://www.first.org/cvss/v2/guide#2-2-2-Remediation-Level-RL</rdfs:isDefinedBy>
    </rdf:Description>
    <rdf:Description rdf:about="http://ontologies.ti-semantics.com/score#CVSSv2UnavailableRemediation">
        <rdfs:comment xml:lang="en">There is either no solution available or it is impossible to apply.</rdfs:comment>
        <rdfs:label xml:lang="en">Unavailable</rdfs:label>
        <rdfs:isDefinedBy xml:lang="en">https://www.first.org/cvss/v2/guide#2-2-2-Remediation-Level-RL</rdfs:isDefinedBy>
        <cvss_v2_code>U</cvss_v2_code>
    </rdf:Description>
    <rdf:Description rdf:about="http://ontologies.ti-semantics.com/score#CVSSv2UnconfirmedReportConfidence">
        <rdfs:isDefinedBy rdf:datatype="http://www.w3.org/2001/XMLSchema#anyURI">https://www.first.org/cvss/v2/guide#2-2-3-Report-Confidence-RC</rdfs:isDefinedBy>
        <rdfs:comment xml:lang="en">There is a single unconfirmed source or possibly multiple conflicting reports. There is little confidence in the validity of the reports. An example is a rumor that surfaces from the hacker underground.</rdfs:comment>
        <cvss_v2_code>UC</cvss_v2_code>
        <rdfs:label xml:lang="en">Unconfirmed</rdfs:label>
    </rdf:Description>
    <rdf:Description rdf:about="http://ontologies.ti-semantics.com/score#CVSSv2UncorroboratedReportConfidence">
        <rdfs:comment xml:lang="en">There are multiple non-official sources, possibly including independent security companies or research organizations. At this point there may be conflicting technical details or some other lingering ambiguity.</rdfs:comment>
        <cvss_v2_code>UR</cvss_v2_code>
        <rdfs:label xml:lang="en">Uncorroborated</rdfs:label>
        <rdfs:isDefinedBy rdf:datatype="http://www.w3.org/2001/XMLSchema#anyURI">https://www.first.org/cvss/v2/guide#2-2-3-Report-Confidence-RC</rdfs:isDefinedBy>
    </rdf:Description>
    <rdf:Description rdf:about="http://ontologies.ti-semantics.com/score#CVSSv2UnprovenExploitability">
        <cvss_v2_code>U</cvss_v2_code>
        <rdfs:label xml:lang="en">Unproven</rdfs:label>
        <rdfs:isDefinedBy rdf:datatype="http://www.w3.org/2001/XMLSchema#anyURI">https://www.first.org/cvss/v2/guide#2-2-1-Exploitability-E</rdfs:isDefinedBy>
        <rdfs:comment xml:lang="en">No exploit code is available, or an exploit is entirely theoretical.</rdfs:comment>
    </rdf:Description>
    <rdf:Description rdf:about="http://ontologies.ti-semantics.com/score#CVSSv2WorkaroundRemediation">
        <rdfs:comment xml:lang="en">There is an unofficial, non-vendor solution available. In some cases, users of the affected technology will create a patch of their own or provide steps to work around or otherwise mitigate the vulnerability.</rdfs:comment>
        <cvss_v2_code>W</cvss_v2_code>
        <rdfs:isDefinedBy xml:lang="en">https://www.first.org/cvss/v2/guide#2-2-2-Remediation-Level-RL</rdfs:isDefinedBy>
        <rdfs:label xml:lang="en">Workaround</rdfs:label>
    </rdf:Description>
    <rdf:Description rdf:about="http://ontologies.ti-semantics.com/score#CVSSv3AdjacentAttackVector">
        <cvss_v3_code xml:lang="en">A</cvss_v3_code>
        <rdfs:label xml:lang="en">Adjacent</rdfs:label>
        <rdfs:comment xml:lang="en">A vulnerability exploitable with adjacent network access means the vulnerable component is bound to the network stack, however the attack is limited to the same shared physical (e.g. Bluetooth, IEEE 802.11), or logical (e.g. local IP subnet) network, and cannot be performed across an OSI layer 3 boundary (e.g. a router). An example of an Adjacent attack would be an ARP (IPv4) or neighbor discovery (IPv6) flood leading to a denial of service on the local LAN segment. See also CVE-2013-6014.</rdfs:comment>
        <rdfs:isDefinedBy xml:lang="en">https://www.first.org/cvss/specification-document#2-1-1-Attack-Vector-AV</rdfs:isDefinedBy>
    </rdf:Description>
    <rdf:Description rdf:about="http://ontologies.ti-semantics.com/score#CVSSv3ChangedScope">
        <cvss_v3_code xml:lang="en">C</cvss_v3_code>
        <rdfs:isDefinedBy xml:lang="en">https://www.first.org/cvss/specification-document#2-2-Scope-S</rdfs:isDefinedBy>
        <rdfs:comment xml:lang="en">An exploited vulnerability can affect resources beyond the authorization privileges intended by the vulnerable component. In this case the vulnerable component and the impacted component are different.</rdfs:comment>
        <rdfs:label xml:lang="en">Changed</rdfs:label>
    </rdf:Description>
    <rdf:Description rdf:about="http://ontologies.ti-semantics.com/score#CVSSv3ConfirmedReportConfidence">
        <rdfs:label xml:lang="en">Confirmed</rdfs:label>
        <rdfs:comment xml:lang="en">Detailed reports exist, or functional reproduction is possible (functional exploits may provide this). Source code is available to independently verify the assertions of the research, or the author or vendor of the affected code has confirmed the presence of the vulnerability.</rdfs:comment>
        <rdfs:isDefinedBy xml:lang="en">https://www.first.org/cvss/specification-document#3-3-Report-Confidence-RC</rdfs:isDefinedBy>
        <cvss_v3_code>C</cvss_v3_code>
    </rdf:Description>
    <rdf:Description rdf:about="http://ontologies.ti-semantics.com/score#CVSSv3FunctionalExploitCodeMaturity">
        <cvss_v3_code xml:lang="en">F</cvss_v3_code>
        <rdfs:isDefinedBy rdf:datatype="http://www.w3.org/2001/XMLSchema#anyURI">https://www.first.org/cvss/specification-document#3-1-Exploit-Code-Maturity-E</rdfs:isDefinedBy>
        <rdfs:comment xml:lang="en">Functional exploit code is available. The code works in most situations where the vulnerability exists.</rdfs:comment>
    </rdf:Description>
    <rdf:Description rdf:about="http://ontologies.ti-semantics.com/score#CVSSv3HighAttackComplexity">
        <rdfs:comment xml:lang="en">A successful attack depends on conditions beyond the attacker&apos;s control. That is, a successful attack cannot be accomplished at will, but requires the attacker to invest in some measurable amount of effort in preparation or execution against the vulnerable component before a successful attack can be expected. For example, a successful attack may depend on an attacker overcoming any of the following conditions:

- The attacker must conduct target-specific reconnaissance. For example, on target configuration settings, sequence numbers, shared secrets, etc.

- The attacker must prepare the target environment to improve exploit reliability. For example, repeated exploitation to win a race condition, or overcoming advanced exploit mitigation techniques.

- The attacker must inject herself into the logical network path between the target and the resource requested by the victim in order to read and/or modify network communications (e.g. man in the middle attack).</rdfs:comment>
        <cvss_v3_code>H</cvss_v3_code>
        <rdfs:label xml:lang="en">High</rdfs:label>
        <rdfs:isDefinedBy xml:lang="en">https://www.first.org/cvss/specification-document#2-1-2-Attack-Complexity-AC</rdfs:isDefinedBy>
    </rdf:Description>
    <rdf:Description rdf:about="http://ontologies.ti-semantics.com/score#CVSSv3HighAvailabilityImpact">
        <rdfs:comment xml:lang="en">There is total loss of availability, resulting in the attacker being able to fully deny access to resources in the impacted component; this loss is either sustained (while the attacker continues to deliver the attack) or persistent (the condition persists even after the attack has completed). Alternatively, the attacker has the ability to deny some availability, but the loss of availability presents a direct, serious consequence to the impacted component (e.g., the attacker cannot disrupt existing connections, but can prevent new connections; the attacker can repeatedly exploit a vulnerability that, in each instance of a successful attack, leaks a only small amount of memory, but after repeated exploitation causes a service to become completely unavailable).</rdfs:comment>
        <cvss_v3_code>H</cvss_v3_code>
        <rdfs:label xml:lang="en">High</rdfs:label>
    </rdf:Description>
    <rdf:Description rdf:about="http://ontologies.ti-semantics.com/score#CVSSv3HighAvailabilityRequirement">
        <rdfs:comment xml:lang="en">Loss of Availability is likely to have a catastrophic adverse effect on the organization or individuals associated with the organization (e.g., employees, customers).</rdfs:comment>
        <cvss_v3_code xml:lang="en">H</cvss_v3_code>
        <rdfs:isDefinedBy rdf:datatype="http://www.w3.org/2001/XMLSchema#anyURI">https://www.first.org/cvss/specification-document#4-1-Security-Requirements-CR-IR-AR</rdfs:isDefinedBy>
    </rdf:Description>
    <rdf:Description rdf:about="http://ontologies.ti-semantics.com/score#CVSSv3HighConfidentialityImpact">
        <rdfs:label xml:lang="en">High</rdfs:label>
        <rdfs:comment xml:lang="en">There is total loss of confidentiality, resulting in all resources within the
 impacted component being divulged to the attacker. Alternatively, access to only some restricted information is obtained, but the disclosed information presents a direct, serious impact. For example, an attacker steals the administrator&apos;s password, or private encryption keys of a web server.</rdfs:comment>
        <cvss_v3_code xml:lang="en">H</cvss_v3_code>
    </rdf:Description>
    <rdf:Description rdf:about="http://ontologies.ti-semantics.com/score#CVSSv3HighExploitCodeMaturity">
        <cvss_v3_code xml:lang="en">H</cvss_v3_code>
        <rdfs:isDefinedBy rdf:datatype="http://www.w3.org/2001/XMLSchema#anyURI">https://www.first.org/cvss/specification-document#3-1-Exploit-Code-Maturity-E</rdfs:isDefinedBy>
        <rdfs:comment xml:lang="en">Functional autonomous code exists, or no exploit is required (manual trigger) and details are widely available. Exploit code works in every situation, or is actively being delivered via an autonomous agent (such as a worm or virus). Network-connected systems are likely to encounter scanning or exploitation attempts. Exploit development has reached the level of reliable, widely-available, easy-to-use automated tools.</rdfs:comment>
    </rdf:Description>
    <rdf:Description rdf:about="http://ontologies.ti-semantics.com/score#CVSSv3HighIntegrityImpact">
        <rdfs:label xml:lang="en">High</rdfs:label>
        <rdfs:isDefinedBy xml:lang="en">https://www.first.org/cvss/specification-document#2-3-2-Integrity-Impact-I</rdfs:isDefinedBy>
        <rdfs:comment xml:lang="en">There is a total loss of integrity, or a complete loss of protection. For example, the attacker is able to modify any/all files protected by the impacted component. Alternatively, only some files can be modified, but malicious modification would present a direct, serious consequence to the impacted component.</rdfs:comment>
        <cvss_v3_code>H</cvss_v3_code>
    </rdf:Description>
    <rdf:Description rdf:about="http://ontologies.ti-semantics.com/score#CVSSv3HighPrivilegesRequired">
        <cvss_v3_code>H</cvss_v3_code>
        <rdfs:label xml:lang="en">High</rdfs:label>
        <rdfs:comment xml:lang="en">The attacker is authorized with (i.e. requires) privileges that provide significant (e.g. administrative) control over the vulnerable component that could affect component-wide settings and files.</rdfs:comment>
        <rdfs:isDefinedBy xml:lang="en">https://www.first.org/cvss/specification-document#2-1-3-Privileges-Required-PR</rdfs:isDefinedBy>
    </rdf:Description>
    <rdf:Description rdf:about="http://ontologies.ti-semantics.com/score#CVSSv3LocalAttackVector">
        <rdfs:label xml:lang="en">Local</rdfs:label>
        <rdfs:comment xml:lang="en">A vulnerability exploitable with Local access means that the vulnerable component is not bound to the network stack, and the attacker’s path is via read/write/execute capabilities. In some cases, the attacker may be logged in locally in order to exploit the vulnerability, otherwise, she may rely on User Interaction to execute a malicious file.</rdfs:comment>
        <rdfs:isDefinedBy xml:lang="en">https://www.first.org/cvss/specification-document#2-1-1-Attack-Vector-AV</rdfs:isDefinedBy>
        <cvss_v3_code xml:lang="en">L</cvss_v3_code>
    </rdf:Description>
    <rdf:Description rdf:about="http://ontologies.ti-semantics.com/score#CVSSv3LowAttackComplexity">
        <rdfs:comment xml:lang="en">Specialized access conditions or extenuating circumstances do not exist. An attacker can expect repeatable success against the vulnerable component.</rdfs:comment>
        <cvss_v3_code>L</cvss_v3_code>
        <rdfs:isDefinedBy xml:lang="en">https://www.first.org/cvss/specification-document#2-1-2-Attack-Complexity-AC</rdfs:isDefinedBy>
        <rdfs:label xml:lang="en">Low</rdfs:label>
    </rdf:Description>
    <rdf:Description rdf:about="http://ontologies.ti-semantics.com/score#CVSSv3LowAvailabilityImpact">
        <rdfs:label xml:lang="en">Low</rdfs:label>
        <rdfs:comment xml:lang="en">There is reduced performance or interruptions in resource availability. Even if repeated exploitation of the vulnerability is possible, the attacker does not have the ability to completely deny service to legitimate users. The resources in the impacted component are either partially available all of the time, or fully available only some of the time, but overall there is no direct, serious consequence to the impacted component.</rdfs:comment>
        <cvss_v3_code>L</cvss_v3_code>
    </rdf:Description>
    <rdf:Description rdf:about="http://ontologies.ti-semantics.com/score#CVSSv3LowAvailabilityRequirement">
        <rdfs:comment xml:lang="en">Loss of Availability is likely to have only a limited adverse effect on the organization or individuals associated with the organization (e.g., employees, customers).</rdfs:comment>
        <rdfs:isDefinedBy rdf:datatype="http://www.w3.org/2001/XMLSchema#anyURI">https://www.first.org/cvss/specification-document#4-1-Security-Requirements-CR-IR-AR</rdfs:isDefinedBy>
        <cvss_v3_code xml:lang="en">L</cvss_v3_code>
    </rdf:Description>
    <rdf:Description rdf:about="http://ontologies.ti-semantics.com/score#CVSSv3LowConfidentialityImpact">
        <cvss_v3_code xml:lang="en">L</cvss_v3_code>
        <rdfs:comment xml:lang="en">There is some loss of confidentiality. Access to some restricted information is obtained, but the attacker does not have control over what information is obtained, or the amount or kind of loss is constrained. The information disclosure does not cause a direct, serious loss to the impacted component.</rdfs:comment>
        <rdfs:label xml:lang="en">Low</rdfs:label>
    </rdf:Description>
    <rdf:Description rdf:about="http://ontologies.ti-semantics.com/score#CVSSv3LowIntegrityImpact">
        <cvss_v3_code>L</cvss_v3_code>
        <rdfs:isDefinedBy xml:lang="en">https://www.first.org/cvss/specification-document#2-3-2-Integrity-Impact-I</rdfs:isDefinedBy>
        <rdfs:comment xml:lang="en">Modification of data is possible, but the attacker does not have control over the consequence of a modification, or the amount of modification is constrained. The data modification does not have a direct, serious impact on the impacted component.</rdfs:comment>
        <rdfs:label xml:lang="en">Low</rdfs:label>
    </rdf:Description>
    <rdf:Description rdf:about="http://ontologies.ti-semantics.com/score#CVSSv3LowPrivilegesRequired">
        <rdfs:comment xml:lang="en">The attacker is authorized with (i.e. requires) privileges that provide basic user capabilities that could normally affect only settings and files owned by a user. Alternatively, an attacker with Low privileges may have the ability to cause an impact only to non-sensitive resources.</rdfs:comment>
        <rdfs:label xml:lang="en">Low</rdfs:label>
        <cvss_v3_code>L</cvss_v3_code>
        <rdfs:isDefinedBy xml:lang="en">https://www.first.org/cvss/specification-document#2-1-3-Privileges-Required-PR</rdfs:isDefinedBy>
    </rdf:Description>
    <rdf:Description rdf:about="http://ontologies.ti-semantics.com/score#CVSSv3MediumAvailabilityRequirement">
        <rdfs:comment xml:lang="en">Loss of Availability is likely to have a serious adverse effect on the organization or individuals associated with the organization (e.g., employees, customers).</rdfs:comment>
        <cvss_v3_code xml:lang="en">M</cvss_v3_code>
        <rdfs:isDefinedBy rdf:datatype="http://www.w3.org/2001/XMLSchema#anyURI">https://www.first.org/cvss/specification-document#4-1-Security-Requirements-CR-IR-AR</rdfs:isDefinedBy>
    </rdf:Description>
    <rdf:Description rdf:about="http://ontologies.ti-semantics.com/score#CVSSv3NetworkAttackVector">
        <rdfs:comment xml:lang="en">A vulnerability exploitable with network access means the vulnerable component is bound to the network stack and the attacker&apos;s path is through OSI layer 3 (the network layer). Such a vulnerability is often termed “remotely exploitable” and can be thought of as an attack being exploitable one or more network hops away (e.g. across layer 3 boundaries from routers). An example of a network attack is an attacker causing a denial of service (DoS) by sending a specially crafted TCP packet from across the public Internet (e.g. CVE-2004-0230).</rdfs:comment>
        <rdfs:isDefinedBy xml:lang="en">https://www.first.org/cvss/specification-document#2-1-1-Attack-Vector-AV</rdfs:isDefinedBy>
        <rdfs:label xml:lang="en">Network</rdfs:label>
        <cvss_v3_code xml:lang="en">N</cvss_v3_code>
    </rdf:Description>
    <rdf:Description rdf:about="http://ontologies.ti-semantics.com/score#CVSSv3NoAvailabilityImpact">
        <rdfs:label xml:lang="en">None</rdfs:label>
        <cvss_v3_code>N</cvss_v3_code>
        <rdfs:isDefinedBy rdf:datatype="http://www.w3.org/2001/XMLSchema#anyURI">https://www.first.org/cvss/v2/guide</rdfs:isDefinedBy>
        <rdfs:comment xml:lang="en">There is no impact to availability within the impacted component.</rdfs:comment>
    </rdf:Description>
    <rdf:Description rdf:about="http://ontologies.ti-semantics.com/score#CVSSv3NoConfidentialityImpact">
        <cvss_v2_code xml:lang="en">N</cvss_v2_code>
        <rdfs:label xml:lang="en">None</rdfs:label>
        <rdfs:comment xml:lang="en">There is no loss of confidentiality within the impacted component.</rdfs:comment>
    </rdf:Description>
    <rdf:Description rdf:about="http://ontologies.ti-semantics.com/score#CVSSv3NoIntegrityImpact">
        <rdfs:isDefinedBy xml:lang="en">https://www.first.org/cvss/specification-document#2-3-2-Integrity-Impact-I</rdfs:isDefinedBy>
        <rdfs:label xml:lang="en">None</rdfs:label>
        <rdfs:comment xml:lang="en">There is no loss of integrity within the impacted component.</rdfs:comment>
        <rdfs:isDefinedBy rdf:datatype="http://www.w3.org/2001/XMLSchema#anyURI">https://www.first.org/cvss/v2/guide#2-1-5-Integrity-Impact-I</rdfs:isDefinedBy>
        <cvss_v3_code xml:lang="en">N</cvss_v3_code>
        <rdfs:comment xml:lang="en">There is no impact to the integrity of the system.</rdfs:comment>
    </rdf:Description>
    <owl:Axiom>
        <owl:annotatedSource rdf:resource="http://ontologies.ti-semantics.com/score#CVSSv3NoIntegrityImpact"/>
        <owl:annotatedProperty rdf:resource="http://www.w3.org/2000/01/rdf-schema#comment"/>
        <owl:annotatedTarget xml:lang="en">There is no loss of integrity within the impacted component.</owl:annotatedTarget>
        <rdfs:isDefinedBy rdf:datatype="http://www.w3.org/2001/XMLSchema#anyURI">https://www.first.org/cvss/specification-document#2-3-2-Integrity-Impact-I</rdfs:isDefinedBy>
    </owl:Axiom>
    <owl:Axiom>
        <owl:annotatedSource rdf:resource="http://ontologies.ti-semantics.com/score#CVSSv3NoIntegrityImpact"/>
        <owl:annotatedProperty rdf:resource="http://www.w3.org/2000/01/rdf-schema#comment"/>
        <owl:annotatedTarget xml:lang="en">There is no impact to the integrity of the system.</owl:annotatedTarget>
        <rdfs:isDefinedBy rdf:datatype="http://www.w3.org/2001/XMLSchema#anyURI">https://www.first.org/cvss/specification-document#2-3-2-Integrity-Impact-I</rdfs:isDefinedBy>
    </owl:Axiom>
    <rdf:Description rdf:about="http://ontologies.ti-semantics.com/score#CVSSv3NoPrivilegesRequired">
        <cvss_v3_code xml:lang="en">N</cvss_v3_code>
        <rdfs:isDefinedBy xml:lang="en">https://www.first.org/cvss/specification-document#2-1-3-Privileges-Required-PR</rdfs:isDefinedBy>
        <rdfs:label xml:lang="en">None</rdfs:label>
        <rdfs:comment xml:lang="en">The attacker is unauthorized prior to attack, and therefore does not require any access to settings or files to carry out an attack.</rdfs:comment>
    </rdf:Description>
    <rdf:Description rdf:about="http://ontologies.ti-semantics.com/score#CVSSv3NoUserInteraction">
        <rdfs:isDefinedBy rdf:datatype="http://www.w3.org/2001/XMLSchema#anyURI">https://www.first.org/cvss/specification-document#2-1-4-User-Interaction-UI</rdfs:isDefinedBy>
        <cvss_v3_code xml:lang="en">N</cvss_v3_code>
        <rdfs:label xml:lang="en">None</rdfs:label>
        <rdfs:comment xml:lang="en">The vulnerable system can be exploited without interaction from any user.</rdfs:comment>
    </rdf:Description>
    <rdf:Description rdf:about="http://ontologies.ti-semantics.com/score#CVSSv3NotDefinedAvailabilityRequirement">
        <cvss_v3_code xml:lang="en">X</cvss_v3_code>
        <rdfs:isDefinedBy rdf:datatype="http://www.w3.org/2001/XMLSchema#anyURI">https://www.first.org/cvss/specification-document#4-1-Security-Requirements-CR-IR-AR</rdfs:isDefinedBy>
        <rdfs:comment xml:lang="en">Assigning this value to the metric will not influence the score. It is a signal to the equation to skip this metric.</rdfs:comment>
    </rdf:Description>
    <rdf:Description rdf:about="http://ontologies.ti-semantics.com/score#CVSSv3NotDefinedExploitCodeMaturity">
        <rdfs:comment xml:lang="en">Assigning this value to the metric will not influence the score. It is a signal to a scoring equation to skip this metric.</rdfs:comment>
        <rdfs:isDefinedBy rdf:datatype="http://www.w3.org/2001/XMLSchema#anyURI">https://www.first.org/cvss/specification-document#3-1-Exploit-Code-Maturity-E</rdfs:isDefinedBy>
        <cvss_v3_code xml:lang="en">X</cvss_v3_code>
    </rdf:Description>
    <rdf:Description rdf:about="http://ontologies.ti-semantics.com/score#CVSSv3NotDefinedRemediation">
        <rdfs:label xml:lang="en">Not Defined</rdfs:label>
        <rdfs:comment xml:lang="en">Assigning this value to the metric will not influence the score. It is a signal to a scoring equation to skip this metric.</rdfs:comment>
        <cvss_v3_code>X</cvss_v3_code>
        <rdfs:isDefinedBy xml:lang="en">https://www.first.org/cvss/specification-document#3-2-Remediation-Level-RL</rdfs:isDefinedBy>
    </rdf:Description>
    <rdf:Description rdf:about="http://ontologies.ti-semantics.com/score#CVSSv3NotDefinedReportConfidence">
        <rdfs:isDefinedBy xml:lang="en">https://www.first.org/cvss/specification-document#3-3-Report-Confidence-RC</rdfs:isDefinedBy>
        <rdfs:comment xml:lang="en">Assigning this value to the metric will not influence the score. It is a signal to a scoring equation to skip this metric.</rdfs:comment>
        <cvss_v3_code>X</cvss_v3_code>
        <rdfs:label xml:lang="en">Not Defined</rdfs:label>
    </rdf:Description>
    <rdf:Description rdf:about="http://ontologies.ti-semantics.com/score#CVSSv3OfficialFixRemediation">
        <cvss_v3_code>O</cvss_v3_code>
        <rdfs:comment xml:lang="en">A complete vendor solution is available. Either the vendor has issued an official patch, or an upgrade is available.</rdfs:comment>
        <rdfs:isDefinedBy xml:lang="en">https://www.first.org/cvss/specification-document#3-2-Remediation-Level-RL</rdfs:isDefinedBy>
        <rdfs:label xml:lang="en">Official Fix</rdfs:label>
    </rdf:Description>
    <rdf:Description rdf:about="http://ontologies.ti-semantics.com/score#CVSSv3PhysicalAttackVector">
        <rdfs:comment xml:lang="en">A vulnerability exploitable with Physical access requires the attacker to  physically touch or manipulate the vulnerable component. Physical interaction may be brief (e.g. evil maid attack) or persistent. An example of such an attack is a cold boot attack which allows an attacker to access to disk encryption keys after gaining physical access to the system, or peripheral attacks such as Firewire/USB Direct Memory Access attacks.</rdfs:comment>
        <rdfs:label xml:lang="en">Physical</rdfs:label>
        <rdfs:isDefinedBy xml:lang="en">https://www.first.org/cvss/specification-document#2-1-1-Attack-Vector-AV</rdfs:isDefinedBy>
        <cvss_v3_code xml:lang="en">P</cvss_v3_code>
    </rdf:Description>
    <rdf:Description rdf:about="http://ontologies.ti-semantics.com/score#CVSSv3ProofOfConceptExploitCodeMaturity">
        <cvss_v3_code xml:lang="en">P</cvss_v3_code>
        <rdfs:isDefinedBy rdf:datatype="http://www.w3.org/2001/XMLSchema#anyURI">https://www.first.org/cvss/specification-document#3-1-Exploit-Code-Maturity-E</rdfs:isDefinedBy>
        <rdfs:comment xml:lang="en">Proof-of-concept exploit code is available, or an attack demonstration is not practical for most systems. The code or technique is not functional in all situations and may require substantial modification by a skilled attacker.</rdfs:comment>
    </rdf:Description>
    <rdf:Description rdf:about="http://ontologies.ti-semantics.com/score#CVSSv3ReasonableReportConfidence">
        <rdfs:isDefinedBy xml:lang="en">https://www.first.org/cvss/specification-document#3-3-Report-Confidence-RC</rdfs:isDefinedBy>
        <cvss_v3_code>R</cvss_v3_code>
        <rdfs:label xml:lang="en">Reasonable</rdfs:label>
        <rdfs:comment xml:lang="en">Significant details are published, but researchers either do not have full confidence in the root cause, or do not have access to source code to fully confirm all of the interactions that may lead to the result. Reasonable confidence exists, however, that the bug is reproducible and at least one impact is able to be verified (proof-of-concept exploits may provide this). An example is a detailed write-up of research into a vulnerability with an explanation (possibly obfuscated or “left as an exercise to the reader”) that gives assurances on how to reproduce the results.</rdfs:comment>
    </rdf:Description>
    <rdf:Description rdf:about="http://ontologies.ti-semantics.com/score#CVSSv3RequiredUserInteraction">
        <cvss_v3_code xml:lang="en">R</cvss_v3_code>
        <rdfs:label xml:lang="en">Required</rdfs:label>
        <rdfs:comment xml:lang="en">Successful exploitation of this vulnerability requires a user to take some action before the vulnerability can be exploited. For example, a successful exploit may only be possible during the installation of an application by a system administrator.</rdfs:comment>
        <rdfs:isDefinedBy rdf:datatype="http://www.w3.org/2001/XMLSchema#anyURI">https://www.first.org/cvss/specification-document#2-1-4-User-Interaction-UI</rdfs:isDefinedBy>
    </rdf:Description>
    <rdf:Description rdf:about="http://ontologies.ti-semantics.com/score#CVSSv3TemporaryFixRemediation">
        <rdfs:isDefinedBy xml:lang="en">https://www.first.org/cvss/specification-document#3-2-Remediation-Level-RL</rdfs:isDefinedBy>
        <cvss_v3_code>T</cvss_v3_code>
        <rdfs:comment xml:lang="en">There is an official but temporary fix available. This includes instances where the vendor issues a temporary hotfix, tool, or workaround.</rdfs:comment>
        <rdfs:label xml:lang="en">Temporary Fix</rdfs:label>
    </rdf:Description>
    <rdf:Description rdf:about="http://ontologies.ti-semantics.com/score#CVSSv3UnavailableRemediation">
        <cvss_v3_code>U</cvss_v3_code>
        <rdfs:comment xml:lang="en">There is either no solution available or it is impossible to apply.</rdfs:comment>
        <rdfs:isDefinedBy xml:lang="en">https://www.first.org/cvss/specification-document#3-2-Remediation-Level-RL</rdfs:isDefinedBy>
        <rdfs:label xml:lang="en">Unavailable</rdfs:label>
    </rdf:Description>
    <rdf:Description rdf:about="http://ontologies.ti-semantics.com/score#CVSSv3UnchangedScope">
        <rdfs:isDefinedBy rdf:datatype="http://www.w3.org/2001/XMLSchema#anyURI">https://www.first.org/cvss/specification-document#2-2-Scope-S</rdfs:isDefinedBy>
        <cvss_v3_code xml:lang="en">U</cvss_v3_code>
        <rdfs:comment xml:lang="en">An exploited vulnerability can only affect resources managed by the same authority. In this case the vulnerable component and the impacted component are the same.</rdfs:comment>
        <rdfs:label xml:lang="en">Unchanged</rdfs:label>
    </rdf:Description>
    <rdf:Description rdf:about="http://ontologies.ti-semantics.com/score#CVSSv3UnknownReportConfidence">
        <rdfs:isDefinedBy xml:lang="en">https://www.first.org/cvss/specification-document#3-3-Report-Confidence-RC</rdfs:isDefinedBy>
        <cvss_v3_code>U</cvss_v3_code>
        <rdfs:comment>There are reports of impacts that indicate a vulnerability is present. The reports indicate that the cause of the vulnerability is unknown, or reports may differ on the cause or impacts of the vulnerability. Reporters are uncertain of the true nature of the vulnerability, and there is little confidence in the validity of the reports or whether a static Base score can be applied given the differences described. An example is a bug report which notes that an intermittent but non-reproducible crash occurs, with evidence of memory corruption suggesting that denial of service, or possible more serious impacts, may result.</rdfs:comment>
        <rdfs:label xml:lang="en">Unknown</rdfs:label>
    </rdf:Description>
    <rdf:Description rdf:about="http://ontologies.ti-semantics.com/score#CVSSv3UnprovenExploitCodeMaturity">
        <rdfs:isDefinedBy rdf:datatype="http://www.w3.org/2001/XMLSchema#anyURI">https://www.first.org/cvss/specification-document#3-1-Exploit-Code-Maturity-E</rdfs:isDefinedBy>
        <cvss_v3_code xml:lang="en">U</cvss_v3_code>
        <rdfs:comment xml:lang="en">No exploit code is available, or an exploit is theoretical.</rdfs:comment>
    </rdf:Description>
    <rdf:Description rdf:about="http://ontologies.ti-semantics.com/score#CVSSv3WorkaroundRemediation">
        <rdfs:comment xml:lang="en">There is an unofficial, non-vendor solution available. In some cases, users of the affected technology will create a patch of their own or provide steps to work around or otherwise mitigate the vulnerability.</rdfs:comment>
        <cvss_v3_code>W</cvss_v3_code>
        <rdfs:isDefinedBy xml:lang="en">https://www.first.org/cvss/specification-document#3-2-Remediation-Level-RL</rdfs:isDefinedBy>
        <rdfs:label xml:lang="en">Workaround</rdfs:label>
    </rdf:Description>
</rdf:RDF>



<!-- Generated by the OWL API (version 4.5.7.2018-12-02T02:23:35Z) https://github.com/owlcs/owlapi -->

