<?xml version="1.0"?>
<rdf:RDF xmlns="http://ontologies.ti-semantics.com/vulnerability#"
     xml:base="http://ontologies.ti-semantics.com/vulnerability"
     xmlns:owl="http://www.w3.org/2002/07/owl#"
     xmlns:rdf="http://www.w3.org/1999/02/22-rdf-syntax-ns#"
     xmlns:uvo="http://ontologies.ti-semantics.com/uvo#"
     xmlns:xml="http://www.w3.org/XML/1998/namespace"
     xmlns:xsd="http://www.w3.org/2001/XMLSchema#"
     xmlns:core="http://ontologies.ti-semantics.com/core#"
     xmlns:rdfs="http://www.w3.org/2000/01/rdf-schema#"
     xmlns:core1="https://mswimmer.github.io/utim/core#"
     xmlns:terms="http://purl.org/dc/terms/"
     xmlns:vulnerability="http://ontologies.ti-semantics.com/vulnerability#">
    <owl:Ontology rdf:about="http://ontologies.ti-semantics.com/vulnerability">
        <owl:versionIRI rdf:resource="http://ontologies.ti-semantics.com/vulnerability-1.0.2"/>
        <owl:imports rdf:resource="http://ontologies.ti-semantics.com/core-1.0.0"/>
        <owl:imports rdf:resource="http://ontologies.ti-semantics.com/weakness-v1.0.2"/>
        <terms:license rdf:datatype="http://www.w3.org/2001/XMLSchema#anyURI">http://creativecommons.org/licenses/by-sa/4.0/</terms:license>
        <rdfs:comment xml:lang="en">This is an ontology for describing vulnerabilities in software and systems. The intent of this ontology is to allow reasoning over threat data.</rdfs:comment>
        <rdfs:label xml:lang="en">Vulnerability Ontology</rdfs:label>
    </owl:Ontology>
    


    <!-- 
    ///////////////////////////////////////////////////////////////////////////////////////
    //
    // Annotation properties
    //
    ///////////////////////////////////////////////////////////////////////////////////////
     -->

    


    <!-- http://ontologies.ti-semantics.com/core#xpath -->

    <owl:AnnotationProperty rdf:about="http://ontologies.ti-semantics.com/core#xpath"/>
    


    <!-- http://ontologies.ti-semantics.com/vulnerability#summary -->

    <owl:AnnotationProperty rdf:about="http://ontologies.ti-semantics.com/vulnerability#summary">
        <rdfs:range rdf:resource="http://www.w3.org/2001/XMLSchema#string"/>
        <rdfs:domain rdf:resource="http://ontologies.ti-semantics.com/vulnerability#Entry"/>
    </owl:AnnotationProperty>
    


    <!-- http://purl.org/dc/terms/license -->

    <owl:AnnotationProperty rdf:about="http://purl.org/dc/terms/license"/>
    


    <!-- 
    ///////////////////////////////////////////////////////////////////////////////////////
    //
    // Object Properties
    //
    ///////////////////////////////////////////////////////////////////////////////////////
     -->

    


    <!-- http://ontologies.ti-semantics.com/vulnerability#reference -->

    <owl:ObjectProperty rdf:about="http://ontologies.ti-semantics.com/vulnerability#reference">
        <rdfs:subPropertyOf rdf:resource="http://ontologies.ti-semantics.com/core#reference"/>
        <rdfs:domain rdf:resource="http://ontologies.ti-semantics.com/core#Vulnerability"/>
        <rdfs:range rdf:resource="http://ontologies.ti-semantics.com/vulnerability#Reference"/>
        <core:xpath>references</core:xpath>
        <rdfs:comment xml:lang="en">This related a vulnerability to a reference of some type.</rdfs:comment>
        <rdfs:label xml:lang="en">reference</rdfs:label>
    </owl:ObjectProperty>
    


    <!-- http://ontologies.ti-semantics.com/vulnerability#scanner -->

    <owl:ObjectProperty rdf:about="http://ontologies.ti-semantics.com/vulnerability#scanner">
        <core:xpath>//vuln:scanner</core:xpath>
        <rdfs:comment>Range is toolConfigurationType in the schema</rdfs:comment>
    </owl:ObjectProperty>
    


    <!-- http://ontologies.ti-semantics.com/vulnerability#score -->

    <owl:ObjectProperty rdf:about="http://ontologies.ti-semantics.com/vulnerability#score">
        <rdf:type rdf:resource="http://www.w3.org/2002/07/owl#FunctionalProperty"/>
        <rdfs:domain rdf:resource="http://ontologies.ti-semantics.com/core#Vulnerability"/>
        <rdfs:range rdf:resource="http://ontologies.ti-semantics.com/core#Metric"/>
        <core:xpath>//vuln:cvss</core:xpath>
        <rdfs:comment xml:lang="en">Specify the score individual that defines the security related metrics of this vulnerability.</rdfs:comment>
        <rdfs:label xml:lang="en">score</rdfs:label>
    </owl:ObjectProperty>
    


    <!-- http://ontologies.ti-semantics.com/vulnerability#vulnerability -->

    <owl:ObjectProperty rdf:about="http://ontologies.ti-semantics.com/vulnerability#vulnerability">
        <rdfs:domain rdf:resource="http://ontologies.ti-semantics.com/vulnerability#VulnerabilityCatalog"/>
        <rdfs:range rdf:resource="http://ontologies.ti-semantics.com/core#Vulnerability"/>
        <rdfs:comment xml:lang="en">Relates a vulnerability instance to a catalog of vulnerabilities.</rdfs:comment>
        <rdfs:label xml:lang="en">vulnerability</rdfs:label>
    </owl:ObjectProperty>
    


    <!-- http://ontologies.ti-semantics.com/vulnerability#vulnerablePlatform -->

    <owl:ObjectProperty rdf:about="http://ontologies.ti-semantics.com/vulnerability#vulnerablePlatform">
        <rdfs:domain rdf:resource="http://ontologies.ti-semantics.com/core#Vulnerability"/>
        <rdfs:range rdf:resource="http://ontologies.ti-semantics.com/core#Platform"/>
        <rdfs:comment xml:lang="en">Which platform or products are vulnerable to this vulnerability.</rdfs:comment>
        <rdfs:label xml:lang="en">vulnerable platform</rdfs:label>
    </owl:ObjectProperty>
    


    <!-- http://ontologies.ti-semantics.com/vulnerability#weakness -->

    <owl:ObjectProperty rdf:about="http://ontologies.ti-semantics.com/vulnerability#weakness">
        <rdfs:domain rdf:resource="http://ontologies.ti-semantics.com/core#Vulnerability"/>
        <rdfs:range rdf:resource="http://ontologies.ti-semantics.com/core#Weakness"/>
        <rdfs:comment xml:lang="en">This specifies the weakness that the vulnerability is related to.</rdfs:comment>
        <rdfs:label xml:lang="en">related weakness</rdfs:label>
    </owl:ObjectProperty>
    


    <!-- 
    ///////////////////////////////////////////////////////////////////////////////////////
    //
    // Data properties
    //
    ///////////////////////////////////////////////////////////////////////////////////////
     -->

    


    <!-- http://ontologies.ti-semantics.com/vulnerability#id -->

    <owl:DatatypeProperty rdf:about="http://ontologies.ti-semantics.com/vulnerability#id">
        <rdfs:subPropertyOf rdf:resource="http://ontologies.ti-semantics.com/core#id"/>
        <rdfs:domain rdf:resource="http://ontologies.ti-semantics.com/core#Vulnerability"/>
        <rdfs:range rdf:resource="http://www.w3.org/2001/XMLSchema#token"/>
        <rdfs:comment xml:lang="en">An Identifier of a vulnerability as a token literal. For instance, CVE-2019-0002 for a CVE.</rdfs:comment>
        <rdfs:label xml:lang="en">vulnerability id</rdfs:label>
    </owl:DatatypeProperty>
    


    <!-- http://ontologies.ti-semantics.com/vulnerability#modified -->

    <owl:DatatypeProperty rdf:about="http://ontologies.ti-semantics.com/vulnerability#modified">
        <rdfs:domain rdf:resource="http://ontologies.ti-semantics.com/core#Vulnerability"/>
        <rdfs:range rdf:resource="http://www.w3.org/2001/XMLSchema#date"/>
        <rdfs:range rdf:resource="http://www.w3.org/2001/XMLSchema#dateTime"/>
        <core:xpath>//last-modified-datetime</core:xpath>
        <rdfs:comment xml:lang="en">Last time this entry was modified. This can be either a date or a dateTime.</rdfs:comment>
        <rdfs:label xml:lang="en">modified</rdfs:label>
    </owl:DatatypeProperty>
    


    <!-- http://ontologies.ti-semantics.com/vulnerability#published -->

    <owl:DatatypeProperty rdf:about="http://ontologies.ti-semantics.com/vulnerability#published">
        <rdfs:domain rdf:resource="http://ontologies.ti-semantics.com/core#Vulnerability"/>
        <rdfs:range rdf:resource="http://www.w3.org/2001/XMLSchema#date"/>
        <rdfs:range rdf:resource="http://www.w3.org/2001/XMLSchema#dateTime"/>
        <core:xpath>published-datetime</core:xpath>
        <rdfs:comment xml:lang="en">The time this entry was published. This can be either a date or a dateTime.</rdfs:comment>
    </owl:DatatypeProperty>
    


    <!-- http://ontologies.ti-semantics.com/vulnerability#referenceDeprecated -->

    <owl:DatatypeProperty rdf:about="http://ontologies.ti-semantics.com/vulnerability#referenceDeprecated">
        <rdfs:domain rdf:resource="http://ontologies.ti-semantics.com/core#Vulnerability"/>
        <rdfs:range rdf:resource="http://www.w3.org/2001/XMLSchema#boolean"/>
        <rdfs:comment xml:lang="en">If true, the reference is deprecated. If false, it&apos;s not. If it&apos;s skipped, we don&apos;t know.</rdfs:comment>
        <rdfs:label xml:lang="en">deprecated</rdfs:label>
    </owl:DatatypeProperty>
    


    <!-- http://ontologies.ti-semantics.com/vulnerability#referenceSource -->

    <owl:DatatypeProperty rdf:about="http://ontologies.ti-semantics.com/vulnerability#referenceSource">
        <rdfs:domain rdf:resource="http://ontologies.ti-semantics.com/vulnerability#Reference"/>
        <rdfs:range rdf:resource="http://www.w3.org/2001/XMLSchema#token"/>
        <rdfs:comment xml:lang="en">This is a token that represents the source of the reference. Values look like: BID, SECTRACK, CONFIRM, etc.</rdfs:comment>
        <rdfs:label xml:lang="en">reference source</rdfs:label>
    </owl:DatatypeProperty>
    


    <!-- http://ontologies.ti-semantics.com/vulnerability#referenceTitle -->

    <owl:DatatypeProperty rdf:about="http://ontologies.ti-semantics.com/vulnerability#referenceTitle">
        <rdfs:domain rdf:resource="http://ontologies.ti-semantics.com/vulnerability#Reference"/>
        <rdfs:range rdf:resource="http://www.w3.org/2000/01/rdf-schema#Literal"/>
        <rdfs:comment xml:lang="en">A human readable title for this reference.</rdfs:comment>
        <rdfs:label xml:lang="en">reference title</rdfs:label>
    </owl:DatatypeProperty>
    


    <!-- http://ontologies.ti-semantics.com/vulnerability#referenceURL -->

    <owl:DatatypeProperty rdf:about="http://ontologies.ti-semantics.com/vulnerability#referenceURL">
        <rdfs:domain rdf:resource="http://ontologies.ti-semantics.com/vulnerability#Reference"/>
        <rdfs:range rdf:resource="http://www.w3.org/2001/XMLSchema#anyURI"/>
        <rdfs:comment xml:lang="en">The URL the reference points to. This should be a human readable WWW resource. If the resource is RDF, it would be better to use rdfs:seeAlso.</rdfs:comment>
        <rdfs:label xml:lang="en">reference URL</rdfs:label>
    </owl:DatatypeProperty>
    


    <!-- 
    ///////////////////////////////////////////////////////////////////////////////////////
    //
    // Classes
    //
    ///////////////////////////////////////////////////////////////////////////////////////
     -->

    


    <!-- http://ontologies.ti-semantics.com/core#Catalog -->

    <owl:Class rdf:about="http://ontologies.ti-semantics.com/core#Catalog"/>
    


    <!-- http://ontologies.ti-semantics.com/core#Software -->

    <owl:Class rdf:about="http://ontologies.ti-semantics.com/core#Software"/>
    


    <!-- http://ontologies.ti-semantics.com/vulnerability#CVECatalog -->

    <owl:Class rdf:about="http://ontologies.ti-semantics.com/vulnerability#CVECatalog">
        <rdfs:subClassOf rdf:resource="http://ontologies.ti-semantics.com/vulnerability#VulnerabilityCatalog"/>
        <core:xpath>/cve</core:xpath>
        <rdfs:comment xml:lang="en">The Mitre Common Vulnerability Enumeration (CVE) list. The entries in this catalog are CVE entries as provided by Mitre.</rdfs:comment>
    </owl:Class>
    


    <!-- http://ontologies.ti-semantics.com/vulnerability#CVEVulnerability -->

    <owl:Class rdf:about="http://ontologies.ti-semantics.com/vulnerability#CVEVulnerability">
        <rdfs:subClassOf rdf:resource="http://ontologies.ti-semantics.com/vulnerability#PublishedVulnerability"/>
        <core:xpath>/cve/item</core:xpath>
        <rdfs:comment xml:lang="en">A CVE entry curated and published by the Mitre organization.</rdfs:comment>
    </owl:Class>
    


    <!-- http://ontologies.ti-semantics.com/vulnerability#CandidateVulnerability -->

    <owl:Class rdf:about="http://ontologies.ti-semantics.com/vulnerability#CandidateVulnerability">
        <rdfs:subClassOf rdf:resource="http://ontologies.ti-semantics.com/core#Vulnerability"/>
        <rdfs:comment xml:lang="en">The entry describes a candidate vulnerability.</rdfs:comment>
    </owl:Class>
    


    <!-- http://ontologies.ti-semantics.com/vulnerability#NVD12Catalog -->

    <owl:Class rdf:about="http://ontologies.ti-semantics.com/vulnerability#NVD12Catalog">
        <rdfs:subClassOf rdf:resource="http://ontologies.ti-semantics.com/vulnerability#VulnerabilityCatalog"/>
        <core:xpath>/nvd</core:xpath>
        <rdfs:comment xml:lang="en">The NIST National Vulnerability Database catalog of vulnerabilities. The entries in this catalog is defined by the structure of the National Vulnerability Database XML feed files version: 1.2. The elements and attribute in this document are described by xsd:annotation tags.</rdfs:comment>
    </owl:Class>
    


    <!-- http://ontologies.ti-semantics.com/vulnerability#NVD12Vulnerability -->

    <owl:Class rdf:about="http://ontologies.ti-semantics.com/vulnerability#NVD12Vulnerability">
        <rdfs:subClassOf rdf:resource="http://ontologies.ti-semantics.com/vulnerability#PublishedVulnerability"/>
        <core:xpath>/nvd/entry</core:xpath>
        <rdfs:comment xml:lang="en">A CVE entry curated and published by the National Vulnerability Database project.</rdfs:comment>
    </owl:Class>
    


    <!-- http://ontologies.ti-semantics.com/vulnerability#NVD20Catalog -->

    <owl:Class rdf:about="http://ontologies.ti-semantics.com/vulnerability#NVD20Catalog">
        <rdfs:subClassOf rdf:resource="http://ontologies.ti-semantics.com/vulnerability#VulnerabilityCatalog"/>
    </owl:Class>
    


    <!-- http://ontologies.ti-semantics.com/vulnerability#NVD20Vulnerability -->

    <owl:Class rdf:about="http://ontologies.ti-semantics.com/vulnerability#NVD20Vulnerability">
        <rdfs:subClassOf rdf:resource="http://ontologies.ti-semantics.com/vulnerability#PublishedVulnerability"/>
    </owl:Class>
    


    <!-- http://ontologies.ti-semantics.com/vulnerability#PatchReference -->

    <owl:Class rdf:about="http://ontologies.ti-semantics.com/vulnerability#PatchReference">
        <rdfs:subClassOf rdf:resource="http://ontologies.ti-semantics.com/vulnerability#Reference"/>
        <rdfs:comment xml:lang="en">This type of referenence comes in form of a patch, usually, but not always, from the vendor of the platform/product. This raises the confidence in this vulnerability greatly.</rdfs:comment>
        <rdfs:label>PATCH</rdfs:label>
    </owl:Class>
    


    <!-- http://ontologies.ti-semantics.com/vulnerability#PublishedVulnerability -->

    <owl:Class rdf:about="http://ontologies.ti-semantics.com/vulnerability#PublishedVulnerability">
        <rdfs:subClassOf rdf:resource="http://ontologies.ti-semantics.com/core#Vulnerability"/>
        <rdfs:comment xml:lang="en">This vulnerability has been officially published by some authority.</rdfs:comment>
        <rdfs:label xml:lang="en">Published Vulnerability</rdfs:label>
    </owl:Class>
    


    <!-- http://ontologies.ti-semantics.com/vulnerability#Reference -->

    <owl:Class rdf:about="http://ontologies.ti-semantics.com/vulnerability#Reference">
        <rdfs:subClassOf rdf:resource="http://ontologies.ti-semantics.com/core#Reference"/>
        <rdfs:subClassOf>
            <owl:Restriction>
                <owl:onProperty rdf:resource="http://ontologies.ti-semantics.com/vulnerability#referenceURL"/>
                <owl:qualifiedCardinality rdf:datatype="http://www.w3.org/2001/XMLSchema#nonNegativeInteger">1</owl:qualifiedCardinality>
                <owl:onDataRange rdf:resource="http://www.w3.org/2001/XMLSchema#anyURI"/>
            </owl:Restriction>
        </rdfs:subClassOf>
        <rdfs:comment xml:lang="en">This is a reference from a vulnerabilty to some external entity that may contain further information (in human readable form) about that vulnerability. This can be further refined in subclasses, but this is the catchall when we don&apos;t know much more about the sort of reference.</rdfs:comment>
        <rdfs:label xml:lang="en">Reference</rdfs:label>
    </owl:Class>
    


    <!-- http://ontologies.ti-semantics.com/vulnerability#VendorAdvisoryReference -->

    <owl:Class rdf:about="http://ontologies.ti-semantics.com/vulnerability#VendorAdvisoryReference">
        <rdfs:subClassOf rdf:resource="http://ontologies.ti-semantics.com/vulnerability#Reference"/>
        <rdfs:comment xml:lang="en">This type of reference comes from the vendor of the affected platform/product as an advisory. This adds much to the weight that this vulnerability is real.</rdfs:comment>
        <rdfs:label>VENDOR_ADVISORY</rdfs:label>
    </owl:Class>
    


    <!-- http://ontologies.ti-semantics.com/vulnerability#VulnerabilityCatalog -->

    <owl:Class rdf:about="http://ontologies.ti-semantics.com/vulnerability#VulnerabilityCatalog">
        <rdfs:subClassOf rdf:resource="http://ontologies.ti-semantics.com/core#Catalog"/>
    </owl:Class>
    


    <!-- 
    ///////////////////////////////////////////////////////////////////////////////////////
    //
    // Individuals
    //
    ///////////////////////////////////////////////////////////////////////////////////////
     -->

    


    <!-- http://ontologies.ti-semantics.com/vulnerability#configuration_change -->

    <owl:NamedIndividual rdf:about="http://ontologies.ti-semantics.com/vulnerability#configuration_change"/>
    


    <!-- http://ontologies.ti-semantics.com/vulnerability#external_mitigation -->

    <owl:NamedIndividual rdf:about="http://ontologies.ti-semantics.com/vulnerability#external_mitigation"/>
    


    <!-- http://ontologies.ti-semantics.com/vulnerability#patch -->

    <owl:NamedIndividual rdf:about="http://ontologies.ti-semantics.com/vulnerability#patch"/>
    


    <!-- http://ontologies.ti-semantics.com/vulnerability#policy_change -->

    <owl:NamedIndividual rdf:about="http://ontologies.ti-semantics.com/vulnerability#policy_change"/>
    


    <!-- http://ontologies.ti-semantics.com/vulnerability#software_update -->

    <owl:NamedIndividual rdf:about="http://ontologies.ti-semantics.com/vulnerability#software_update"/>
</rdf:RDF>



<!-- Generated by the OWL API (version 4.5.7.2018-12-02T02:23:35Z) https://github.com/owlcs/owlapi -->

